BASE   <http://www.cidoc-crm.org/cidoc-crm/>
PREFIX rdf: <http://www.w3.org/1999/02/22-rdf-syntax-ns#>
PREFIX rdfs: <http://www.w3.org/2000/01/rdf-schema#>
PREFIX owl: <http://www.w3.org/2002/07/owl#>
PREFIX xsd: <http://www.w3.org/2001/XMLSchema#>

<>      rdf:type         owl:Ontology;
        owl:versionInfo  "RDFs Implementation (February 2024) of CIDOC-CRM 7.1.3"@en;
        rdfs:comment     "CIDOC CRM v7.1.3 implemented in RDFS\n\nThis is the implementation approved by the 58th CRM-SIG meeting (March 2024)\nas the current RDFS version for the CIDOC CRM namespace.\nNote that this is NOT a definition of the CIDOC CRM, but a CIDOC CRM compatible implementation\nof an RDF Schema derived from the authoritative release of the CIDOC CRM v7.1.3 on February 2024\nhttps://cidoc-crm.org/Version/version-7.1.3 by an automated algorithm. It is intended for an\nassumed majority of uses. Depending on the application, users may create adequate extensions \ncompatible with the logical definitions of the CIDOC CRM.\n\nCreated by FORTH-ICS February 13, 2024\nCC BY 4.0 https://creativecommons.org/licenses/by/4.0/legalcode\n\n\n\nEncoding Rules:\n1. The RDF spelling rules do not allow blanks. Hence we have replaced them by underscores.\n   For instance \"E63_Beginning_of_Existence\" or \"P2i_is_type_of\".\n\n2. RDF does not allow to instantiate properties beginning from a range value.\n   Therefore, each CRM property is represented as two RDFS properties.\n   For instance \"P2 has type (is type of)\" is represented as:\n   \"P2_has_type\" for the domain to range direction and \"P2i_is_type_of\" for the range to domain direction.\n\n3. The primitive values \"E60 Number\", \"E61 Time Primitive\", \"E62 String\", \"E94 Space Primitive\" and \n   \"E95 Spacetime Primitive\" referred in the Model for formal completeness are interpreted as rdfs:literal.\n\n4. RDF does not support properties of properties, therefore, users may create their own\n   subProperties for CRM properties that have a type property such as \"P3 has note\":\n   Instead of P3 has note (P3-1 has type : parts description) declare\n   <rdf:Property rdf:about=\"P3_parts_description\">\n      <rdfs:domain rdf:resource=\"E1_CRM_Entity\"/>\n      <rdfs:range rdf:resource=\"http://www.w3.org/2000/01/rdf-schema#Literal\"/>\n      <rdfs:subPropertyOf rdf:resource=\"P3_has_note\"/>\n   </rdf:Property>\n\n5. Scope notes are represented as <rdfs:comment> elements.\n\n6. In addition this encoding contains labels in languages different from English, \n   which are taken from translations of previous versions of the CIDOC CRM.    \n\n7. Any other differences in labels, scope notes  and semantic relationships of this encoding \n   to the authoritative definition of the CIDOC CRM v7.1.3 (February 2024) are not intended transfer errors. \n   FORTH appreciates your feed-back on such errors.\n\n8. CRM time extension 1.0 Encoded in RDFS (http://old.cidoc-crm.org/docs/How_to%20implement%20CRM_Time_in%20RDF.pdf)\n   Since the Time Primitive of the CRM can not directly be implemented in RDF Triple Stores, we define in this extension\n   of 4 properties replacing P81 and P82 adequately using xsd:dateTime. \n   Property P81 is dedicated for modeling the Time-Span's maximum known temporal extent i.e. ongoing_throughout. \n   Property P82 is for modeling the minimum outer bounds of events i.e. at_some_time_within. \n   P81 has its time interval redefined by P81a and P81b. Similarly, we redefine P82 by P82a and P82b.\n## RDFS Generation Policies\n\n### Sources\n\nPolicies followed for the RDFS implementation of CIDOC v.7.1.3 were created w.r.t.:\n\n- Implementing the CIDOC Conceptual Reference Model in RDF (http://www.cidoc-crm.org/Resources/implementing-the-cidoc-conceptual-reference-model-in-rdf)\n- How to implement CRM Time in RDF (http://old.cidoc-crm.org/docs/How_to%20implement%20CRM_Time_in%20RDF.pdf)\n- CIDOC-CRM SIG feedback and the general guidelines:\n  - Each property is declared twice, forward and backwards, unless no inverse name is defined in parentheses, or domain or range is interpreted as literal\n  - All Primitive Values become rdfs:Literal\n  - All IsA declarations from/to and between Primitive values are ignored\n\n### Policies\n\n#### **A. CIDOC Classes implementation in RDFS**\n\nThe CIDOC-CRM model defines classes, that in Triple Stores are typically implemented as primitive values. These classes are all subclasses of `E59 Primitive Value` and in RDFS they are interpreted as Literal. There are some classes in the CIDOC-CRM model that are both subclasses of `E59 Primitive Value` and E41 Appellation. So far we have followed the decision by CRM-SIG in \"Issue 394: Solution for Dualism of E41 Appellation and rdfs:label\" in 28-11-2018 wrt the question whether these classes should be implemented as rdfs:Class or still be interpreted as rdfs:Literal.\n\nIn this version we have followed the following policy regarding CIDOC Classes implementation in RDFS:\n\n> A1. CIDOC Classes that are subClasses of `E59 Primitive Value` are interpreted as rdfs:Literal regardless of whether they are also subClasses of another Class.\n\nAs a result, the following CIDOC classes were not defined in RDFS:\n\n- `E59 Primitive Value`\n- `E60 Number`\n- `E61 Time Primitive`\n- `E62 String`\n- `E94 Space Primitive`\n- `E95 Spacetime Primitive`\n\nAdditionally, the following isA relationships were not defined in RDFS:\n\n- `E59 Primitive Value` `subClassOf` `E1 CRM Entity`\n- `E60 Number` `subClassOf` `E59 Primitive Value`\n- `E61 Time Primitive` `subClassOf` `E41 Appellation`\n- `E61 Time Primitive` `subClassOf` `E59 Primitive Value`\n- `E62 String` `subClassOf` `E59 Primitive Value`\n- `E94 Space Primitive` `subClassOf` `E41 Appellation`\n- `E94 Space Primitive` `subClassOf` `E59 Primitive Value`\n- `E95 Spacetime Primitive` `subClassOf` `E41 Appellation`\n- `E95 Spacetime Primitive` `subClassOf` `E59 Primitive Value`\n\n#### **B. CIDOC Properties implementation in RDFS**\n\nThe decisions in policy A affect the implementation of CIDOC Properties in RDFS. A property cannot define an rdfs:Literal as rdfs:domain, and the backwards direction of a property with an rdfs:Literal as rdfs:range cannot be created for the exact same reason.\n\nFurther, the property ranges defined as rdfs:Literal in this implementation do not inherit the properties of the superclasses defined in the CIDOC Model. A separate guideline will describe how to instantiate such properties if at all needed.\n\nAnother aspect considered for the implementation of properties in RDFS is whether a distinct inverse property definition should be provided.\n\nIn this version we followed the following policies regarding CIDOC Properties implementation in RDFS:\n\n> B1. CIDOC Property backwards/inverse direction is **not** defined, whenever no inverse name for the property has been specified in parentheses in the official CIDOC documentation and property domain is not equal with property range.\n\nAs a result, the following properties do not define an inverse direction.\n\n- `E1 CRM Entity. P3 has note: E62 String`\n- `E19 Physical Object. P57 has number of parts: E60 Number`\n- `E52 Time-Span. P79 beginning is qualified by: E62 String`\n- `E52 Time-Span. P80 end is qualified by: E62 String`\n- `E52 Time-Span. P81 ongoing throughout: E61 Time Primitive`\n- `E52 Time-Span. P82 at some time within: E61 Time Primitive`\n- `E54 Dimension. P90 has value: E60 Number`\n- `E53 Place. P171 at some place within: E94 Space Primitive`\n- `E53 Place. P172 contains: E94 Space Primitive`\n- `E90 Symbolic Object. P190 has symbolic content: E62 String`\n\n> B2. CIDOC Property forward direction is **not** defined whenever property domain is interpreted as rdfs:Literal (A.1). Similarly, CIDOC Property backwards/inverse direction is **not** defined, whenever property range is interpreted as rdfs:Literal (A.1). Further, the instances of classes interpreted as rdfs:Literal, cannot express in RDFs their **inherited** properties that could be expressed according to CIDOC Model.\n\nAs a result,\n\na) The following **direct forward direction** CIDOC Properties **cannot** be expressed and are **not defined** in RDFS:\n\n- `E95 Spacetime Primitive. P169 defines spacetime volume (spacetime volume is defined by): E92 Spacetime Volume`\n- `E61 Time Primitive. P170 defines time (time is defined by): E52 Time-Span`\n\nb) The following **direct backwards direction** CIDOC Properties **cannot** be expressed and are **not defined** in RDFS:\n\n- `E94 Space Primitive. P168i defines place (place is defined by): E53 Place`\n\n> B3. Whenever no backwards/inverse property name is specified and property domain matches with property range, then the forward/direct property direction should be used for **both** directions and **no backwards/inverse property** needs to be defined.\n\nAs a result, we did not implement a separate backwards/inverse direction for the following CIDOC Properties:\n\n- `E53 Place. P121 overlaps with: E53 Place`\n- `E53 Place. P122 borders with: E53 Place`\n- `E92 Spacetime Volume. P132 spatiotemporally overlaps with: E92 Spacetime Volume`\n- `E92 Spacetime Volume. P133 is spatiotemporally separated from: E92 Spacetime Volume`\n\nAdditionally, all aforementioned redundant backwards/inverse CIDOC Property direction references, are replaced by the respective direct/forward CIDOC Property direction.\n\n- The hierarchical link of  `P10i` subPropertyOf `P132i` was replaced with `P10i` subPropertyOf `P132`.\n\n#### **C. Labels and appellations**\n\nCIDOC-CRM version 7.1.3 defines the below subpropertyOf relations:\n\n- `P168 place is defined by` `subPropertyOf` `P1 is identified by`\n- `P169i spacetime volume is defined by` `subPropertyOf` `P1 is identified by`\n- `P170i time is defined by` `subPropertyOf` `P1 is identified by`\n\nThe range of P168, P169i and P170i is `E94 Space Primitive`, `E95 Spacetime Primitive` and `E61 Time Primitive` respectively, which are all subclasses of `E41 Appellation` and interpreted as `rdfs:Literal` in RDFS, i.e. these three properties are datatype properties. However, the P1 property has range E41 Appellation, i.e. this property is an object property. Since OWL 2 distinguishes between object subproperties (https://www.w3.org/TR/2012/REC-owl2-syntax-20121211/#Object_Subproperties), data subproperties (https://www.w3.org/TR/2012/REC-owl2-syntax-20121211/#Data_Subproperties) and annotation subproperties (https://www.w3.org/TR/2012/REC-owl2-syntax-20121211/#Annotation_Subproperties), and also in OWL-DL the subject and object of a subproperty statement must be either both datatype properties or both object properties (see here (https://www.w3.org/TR/owl-ref/#subPropertyOf-def)), we do not include these three subPropertyOf relations in the provided RDFS implementation to avoid inconsistencies when reasoning with OWL 2 and OWL DL. Instead, we provide them in a separate ‘supplementary’ RDFS file which one can use if such inconsistencies are not expected.\n\nIn addition, since in the current practice, the property `rdfs:label` is widely used to denote appellations (see CRM-SIG Issue 394 (http://cidoc-crm.org/Issue/ID-394-solution-for-dualism-of-e41-appellation-and-rdfslabel)), the following `subPropertyOf` relation was also included in the supplementary RDFS file:\n\n- `rdfs:label` subPropertyOf `P1 is identified by`\n\nNote that according to the RDF Schema 1.1 specification, the domain (or range) of a property does not necessarily need to be 'subClassOf' or 'equal' to the domain (or range) of its superproperties. By including this subproperty relation, one can either directly use `rdfs:label` for providing a non-URI identifier/appellation for an instance of `E1 CRM Entity`, or use `P1 is identified by` for associating an additional URI-identifier with an instance of `E1 CRM Entity`, or use `P1 is identified by` and create an intermediate node (i.e. a URI-identifier for instance of `E41_Appellation`) for providing more detailed information about this appellation.\n\n#### **D. Implementing Value Intervals**\n\nThe following are property pairs needed to simulate the interval-valued primitive values foreseen by the CRM:\n\n> D1. addition of two new properties, defined as subproperties of `E52 Time-Span. P81 ongoing throughout: E61 Time Primitive`, for the 'maximum known temporal extent' boundaries specification of `E61 Time Primitive`.\n\nAs a result, we have created the following property definitions:\n\n- `E52 Time-Span. P81a end of the begin: rdfs:Literal` (subPropertyOf `E52 Time-Span. P81 ongoing throughout: E61 Time Primitive`)\n- `E52 Time-Span. P81b begin of the end: rdfs:Literal` (subPropertyOf `E52 Time-Span. P81 ongoing throughout: E61 Time Primitive`)\n\n> D2. addition of two new properties, defined as subproperties of `E52 Time-Span. P82 at some time within: E61 Time Primitive`, for the 'minimum outer bounds' specification of `E61 Time Primitive`.\n\nConsequently, we have created the following property definitions:\n\n- `E52 Time-Span. P82a begin of the begin: rdfs:Literal` (subPropertyOf `E52 Time-Span. P82 at some time within: E61 Time Primitive`)\n- `E52 Time-Span. P82b end of the end: rdfs:Literal` (subPropertyOf `E52 Time-Span. P82 at some time within: E61 Time Primitive`)\n\n> D3. addition of two new properties, defined as subproperties of `E54 Dimension. P90 has value: E60 Number`, for the upper and lower boundaries specification of `E60 Number`.\n\nConsequently, we have created the following property definitions:\n\n- `E54 Dimension. P90a has lower value limit: rdfs:Literal` (subPropertyOf `E54 Dimension. P90 has value: E60 Number`)\n- `E54 Dimension. P90b has upper value limit: rdfs:Literal` (subPropertyOf `E54 Dimension. P90 has value: E60 Number`)\n\n#### **E. Multiple ISA custom declaration Classes**\n\nThe following are declarations of frequently used multiple instantiations as classes with respective multiple IsA (so far only one):\n\n> E1. addition of a new class, defined as subClassOf `E41 Appellation` and `E33 Linguistic Object`, for all Appellations being regarded\nspecific to or characteristic for a language group and being described indirectly via a URI.\n\nAs a result, we have created the following class definition:\n\n- `E33_E41_Linguistic_Appellation` subClass of `E33_Linguistic_Object` and `E41_Appellation`\n\n#### **F. Translations and Scope notes**\n\n> F1. **Translations** Each RDFS Class or Property definition is accompanied by a set of translations expressed as rdfs:labels separated by xml:lang tags. The translation label used for each language is **the most recent** still **valid** translation. Still valid translation may be interpreted in the following ways:\n\n- The English label of the `CurrentVersion` that the current RDFS file is referring to is *almost equal* (accepting only differences regarding multiple spaces) to the English label of the `TranslationVersion` that the translated label was created for. For example, in order to accept a translation for `E22 Human-Made Object` in the CurrentVersion (7.1.3) we should have a translation for E22 that was created based on a CIDOC version that used the same name for E22. The class name of E22 was changed from `E22 Man-Made Object` to `E22 Human-Made Object` in version 6.2.7. So the only **valid** translations would be these that were created based on version 6.2.7 or later. Currently no such translation has been created, so `E22 Human-Made Object` in CurrentVersion (7.1.3) does not define any translation in the RDFS file.\n\n- Another option is to qualify translations as **valid** based on the scope note comparison of `CurrentVersion` and `TranslationVersion`. Since scope notes include formatting information, the comparison should ignore formatting changes.\n\nCurrently in this version we follow the option to qualify translations as valid based on the comparison of the respective labels in the corresponding CIDOC versions.\n\n> F2. **Scope notes** are defined as rdfs:comment and include only the text of the official CIDOC-CRM version in English language. Since scope notes are not just simple texts but include formatting data, a simple removal of the formatting data does not always produce a readable format. Therefore we followed the below simple conventions for the transformation of CIDOC-CRM scope note text into a readable rdfs:comment:\n\n- Each Paragraph defines a new line\n- Each element in an unordered list defines a new line\n- Each element in an ordered list defines a new line prefixed with `'{order}. '`\n- Each superscript text is separated from its base with `'-'`\n- Each subscript text is separated from its base with `'_'` (none found)\n\n> F3. **Scope notes of Inverse Properties**. Scope notes for the inverse/backwards direction of properties are not defined as they are covered by the definition of the direct/forward direction definition. Whenever the direct/forward property direction of a property `Pxxx` is not defined due to policy **B1**, then its scope note is used as scope note for the inverse/backwards property `Pxxxi`, and labeled as `Scope note for 'Pxxx':`.\n\nAs a result, the direct/forward property definition was used for the rdfs:comment definition of\n\n- `E92 Spacetime Volume. P169i spacetime volume is defined by: rdfs:Literal`\n- `E52 Time-Span. P170i time is defined by: rdfs:Literal`\n\n"@en .

<E1_CRM_Entity>  rdf:type  rdfs:Class;
        rdfs:label    "CRM Entity"@en;
        rdfs:label    "CRM Entität"@de;
        rdfs:label    "Οντότητα CIDOC CRM"@el;
        rdfs:label    "Entité CRM"@fr;
        rdfs:label    "Entidade CRM"@pt;
        rdfs:label    "CRM Сущность"@ru;
        rdfs:label    "CRM实体"@zh;
        rdfs:comment  "This class comprises all things in the universe of discourse of the CIDOC Conceptual Reference Model.\nIt is an abstract concept providing for three general properties:\nIdentification by name or appellation, and in particular by a preferred identifier\nClassification by type, allowing further refinement of the specific subclass to which an instance belongs\nAttachment of free text and other unstructured data for the expression of anything not captured by formal properties\nAll other classes within the CIDOC CRM are directly or indirectly specialisations of E1 CRM Entity."@en .

<E2_Temporal_Entity>  rdf:type  rdfs:Class;
        rdfs:label       "Temporal Entity"@en;
        rdfs:label       "Geschehendes"@de;
        rdfs:label       "Έγχρονη Οντότητα"@el;
        rdfs:label       "Entité temporelle"@fr;
        rdfs:label       "Entidade Temporal"@pt;
        rdfs:label       "Врeмeнная Сущность"@ru;
        rdfs:label       "时序实体"@zh;
        rdfs:comment     "This class comprises all phenomena, such as the instances of E4 Periods and E5 Events, which happen over a limited extent in time. This extent in time must be contiguous, i.e., without gaps. In case the defining kinds of phenomena for an instance of E2 Temporal Entity cease to happen, and occur later again at another time, we regard that the former instance of E2 Temporal Entity has ended and a new instance has come into existence. In more intuitive terms, the same event cannot happen twice.\nIn some contexts, such phenomena are also called perdurants. This class is disjoint from E77 Persistent Item and is an abstract class that typically has no direct instances. E2 Temporal Entity is specialized into E4 Period, which applies to a particular geographic area (defined with a greater or lesser degree of precision), and E3 Condition State, which applies to instances of E18 Physical Thing."@en;
        rdfs:subClassOf  <E1_CRM_Entity> .

<E3_Condition_State>  rdf:type  rdfs:Class;
        rdfs:label       "Condition State"@en;
        rdfs:label       "Zustandsphase"@de;
        rdfs:label       "Κατάσταση"@el;
        rdfs:label       "État matériel"@fr;
        rdfs:label       "Estado Material"@pt;
        rdfs:label       "Состояниe"@ru;
        rdfs:label       "条件状态"@zh;
        rdfs:comment     "This class comprises the states of objects characterised by a certain condition over a time-span.\nAn instance of this class describes the prevailing physical condition of any material object or feature during a specific instance of E52 Time-Span. In general, the time-span for which a certain condition can be asserted may be shorter than the real time-span, for which this condition held.\nThe nature of that condition can be described using P2 has type. For example, the instance of E3 Condition State “condition of the SS Great Britain between 22-nd September 1846 and 27-th August 1847” can be characterized as an instance “wrecked” of E55 Type."@en;
        rdfs:subClassOf  <E2_Temporal_Entity> .

<E4_Period>  rdf:type    rdfs:Class;
        rdfs:label       "Period"@en;
        rdfs:label       "Phase"@de;
        rdfs:label       "Περίοδος"@el;
        rdfs:label       "Période"@fr;
        rdfs:label       "Período"@pt;
        rdfs:label       "Пeриод"@ru;
        rdfs:label       "时期"@zh;
        rdfs:comment     "This class comprises sets of coherent phenomena or cultural manifestations occurring in time and space.\nIt is the social or physical coherence of these phenomena that identify an instance of E4 Period and not the associated spatiotemporal extent. This extent is only the “ground” or space in an abstract physical sense that the actual process of growth, spread and retreat has covered. Consequently, different periods can overlap and coexist in time and space, such as when a nomadic culture exists in the same area and time as a sedentary culture. This also means that overlapping land use rights, common among first nations, amounts to overlapping periods.\nOften, this class is used to describe prehistoric or historic periods such as the “Neolithic Period”, the “Ming Dynasty” or the “McCarthy Era”, but also geopolitical units and activities of settlements are regarded as special cases of E4 Period. However, there are no assumptions about the scale of the associated phenomena. In particular all events are seen as synthetic processes consisting of coherent phenomena. Therefore, E4 Period is a superclass of E5 Event. For example, a modern clinical birth, an instance of E67 Birth, can be seen as both a single event, i.e. an instance of E5 Event, and as an extended period, i.e. an instance of E4 Period, that consists of multiple physical processes and complementary activities performed by multiple instances of E39 Actor.\nE4 Period is a subclass of E2 Temporal Entity and of E92 Spacetime Volume. The latter is intended as a phenomenal spacetime volume as defined in CIDOC CRMgeo (Doerr &amp; Hiebel, 2013). By virtue of this multiple inheritance, it is possible to discuss the physical extent of an instance of E4 Period without representing each instance of it together with an instance of its associated spacetime volume. This model combines two quite different kinds of substance: an instance of E4 Period is a phenomenon while an instance of E92 Spacetime Volume is an aggregation of points in spacetime. However, the real spatiotemporal extent of an instance of E4 Period is regarded to be unique to it due to all its details and fuzziness; its identity and existence depends uniquely on the identity of the instance of E4 Period. Therefore, this multiple inheritance is unambiguous and effective and furthermore corresponds to the intuitions of natural language.\nTypical use of this class in cultural heritage documentation is for documenting cultural and artistic periods. There are two different conceptualisations of ‘artistic style’, defined either by physical features or by historical context. For example, “Impressionism” can be viewed as a period in the European sphere of influence lasting from approximately 1870 to 1905 during which paintings with particular characteristics were produced by a group of artists that included (among others) Monet, Renoir, Pissarro, Sisley and Degas. Alternatively, it can be regarded as a style applicable to all paintings sharing the characteristics of the works produced by the Impressionist painters, regardless of historical context. The first interpretation is an instance of E4 Period, and the second defines morphological object types that fall under E55 Type.\nA geopolitical unit as a specific case of an instance of E4 Period is the set of activities and phenomena related to the claim of power, the consequences of belonging to a jurisdictional area and an administrative system that establishes a geopolitical unit. Examples from the modern period are countries or administrative areas of countries such as districts whose actions and structures define activities and phenomena in the area that they intend to govern. The borders of geopolitical units are often defined in contracts or treaties although they may deviate from the actual practice. The spatiotemporal properties of Geopolitical units can be modelled through the properties inherited from E92 Spacetime Volume.\nAnother specific case of an instance of E4 Period is the actual extent of the set of activities and phenomena as evidenced by their physical traces that define a settlement, such as the populated period of Nineveh."@en;
        rdfs:subClassOf  <E2_Temporal_Entity>;
        rdfs:subClassOf  <E92_Spacetime_Volume> .

<E5_Event>  rdf:type     rdfs:Class;
        rdfs:label       "Event"@en;
        rdfs:label       "Ereignis"@de;
        rdfs:label       "Συμβάν"@el;
        rdfs:label       "Évènement"@fr;
        rdfs:label       "Evento"@pt;
        rdfs:label       "Событиe"@ru;
        rdfs:label       "事件"@zh;
        rdfs:comment     "This class comprises distinct, delimited and coherent processes and interactions of a material nature, in cultural, social or physical systems, involving and affecting instances of E77 Persistent Item in a way characteristic of the kind of process. Typical examples are meetings, births, deaths, actions of decision taking, making or inventing things, but also more complex and extended ones such as conferences, elections, building of a castle, or battles.\nWhile the continuous growth of a tree lacks the limits characteristic of an event, its germination from a seed does qualify as an event. Similarly, the blowing of the wind lacks the distinctness and limits of an event, but a hurricane, flood or earthquake would qualify as an event. Mental processes are considered as events, in cases where they are connected with the material externalization of their results; for example, the creation of a poem, a performance or a change of intention that becomes obvious from subsequent actions or declarations.\nThe effects of an instance of E5 Event may not lead to relevant permanent changes of properties or relations of the items involved in it, for example an unrecorded performance. Of course, in order to be documented, some kind of evidence for an event must exist, be it witnesses, traces or products of the event.\nWhile instances of E4 Period always require some form of coherence between its constituent phenomena, in addition, the essential constituents of instances of E5 Event should contribute to an overall effect; for example, the statements made during a meeting and the listening of the audience.\nViewed at a coarse level of detail, an instance of E5 Event may appear as if it had an ‘instantaneous’ overall effect, but any process or interaction of material nature in reality have an extent in time and space. At a fine level, instances of E5 Event may be analysed into component phenomena and phases within a space and timeframe, and as such can be seen as a period, regardless of the size of the phenomena. The reverse is not necessarily the case: not all instances of E4 Period give rise to a noteworthy overall effect and are thus not instances of E5 Event."@en;
        rdfs:subClassOf  <E4_Period> .

<E6_Destruction>  rdf:type  rdfs:Class;
        rdfs:label       "Destruction"@en;
        rdfs:label       "Zerstörung"@de;
        rdfs:label       "Καταστροφή"@el;
        rdfs:label       "Destruction"@fr;
        rdfs:label       "Destruição"@pt;
        rdfs:label       "Разрушeниe"@ru;
        rdfs:label       "破坏"@zh;
        rdfs:comment     "This class comprises events that destroy one or more instances of E18 Physical Thing, such that they lose their identity as the subjects of documentation.\nSome destruction events are intentional, while others are independent of human activity. Intentional destruction can be documented by classifying the event as both an instance of E6 Destruction and of E7 Activity.\nThe decision to document an object as destroyed, transformed, or modified is context-sensitive:\n1. If the matter remaining from the destruction is not documented, the event is modelled solely as an instance of E6 Destruction.\n2. An event should also be documented using E81 Transformation if it results in the destruction of one or more objects and the simultaneous production of others using parts or material from the original. In this case, the new items have separate identities. Matter is preserved, but identity is not.\n3. When the initial identity of the changed instance of E18 Physical Thing is preserved, the event should be documented as an instance of E11 Modification."@en;
        rdfs:subClassOf  <E64_End_of_Existence> .

<E7_Activity>  rdf:type  rdfs:Class;
        rdfs:label       "Activity"@en;
        rdfs:label       "Handlung"@de;
        rdfs:label       "Δράση"@el;
        rdfs:label       "Activité"@fr;
        rdfs:label       "Atividade"@pt;
        rdfs:label       "Дeятeльность"@ru;
        rdfs:label       "活动"@zh;
        rdfs:comment     "This class comprises actions intentionally carried out by instances of E39 Actor that result in changes of state in the cultural, social, or physical systems documented.\nThis notion includes complex, composite, and long-lasting actions such as the building of a settlement or a war, as well as simple, short-lived actions such as the opening of a door."@en;
        rdfs:subClassOf  <E5_Event> .

<E8_Acquisition>  rdf:type  rdfs:Class;
        rdfs:label       "Acquisition"@en;
        rdfs:label       "Erwerb"@de;
        rdfs:label       "Απόκτηση"@el;
        rdfs:label       "Acquisition"@fr;
        rdfs:label       "Aquisição"@pt;
        rdfs:label       "Поступлeниe"@ru;
        rdfs:label       "采访"@zh;
        rdfs:comment     "This class comprises transfers of legal ownership from one or more instances of E39 Actor to one or more other instances of E39 Actor.\nThe class also applies to the establishment or loss of ownership of instances of E18 Physical Thing. It does not, however, imply changes of any other kinds of rights. The recording of the donor and/or recipient is optional. It is possible that in an instance of E8 Acquisition there is either no donor or no recipient. Depending on the circumstances, it may describe:\n1. the beginning of ownership\n2. the end of ownership\n3. the transfer of ownership\n4. the acquisition from an unknown source\n5. the loss of title due to destruction of the item\nIt may also describe events where a collector appropriates legal title, for example, by annexation or field collection. The interpretation of the museum notion of “accession” differs between institutions. The CIDOC CRM therefore models legal ownership (E8 Acquisition) and physical custody (E10 Transfer of Custody) separately. Institutions will then model their specific notions of accession and deaccession as combinations of these."@en;
        rdfs:subClassOf  <E7_Activity> .

<E9_Move>  rdf:type      rdfs:Class;
        rdfs:label       "Move"@en;
        rdfs:label       "Objektbewegung"@de;
        rdfs:label       "Μετακίνηση"@el;
        rdfs:label       "Déplacement"@fr;
        rdfs:label       "Locomoção"@pt;
        rdfs:label       "Пeрeмeщeниe"@ru;
        rdfs:label       "移动"@zh;
        rdfs:comment     "This class comprises changes of the physical location of the instances of E19 Physical Object.\nNote, that the class E9 Move inherits the property P7 took place at (witnessed): E53 Place. This property should be used to describe the trajectory or a larger area within which a move takes place, whereas the properties P26 moved to (was destination of), P27 moved from (was origin of) describe the start and end points only. Moves may also be documented to consist of other moves (via P9 consists of (forms part of)), in order to describe intermediate stages on a trajectory. In that case, start and end points of the partial moves should match appropriately between each other and with the overall event."@en;
        rdfs:subClassOf  <E7_Activity> .

<E10_Transfer_of_Custody>
        rdf:type         rdfs:Class;
        rdfs:label       "Transfer of Custody"@en;
        rdfs:label       "Übertragung des Gewahrsams"@de;
        rdfs:label       "Μεταβίβαση Κατοχής"@el;
        rdfs:label       "Transfert de la garde"@fr;
        rdfs:label       "Transferência de Custódia"@pt;
        rdfs:label       "Пeрeдача Хранeния"@ru;
        rdfs:label       "转移监护权"@zh;
        rdfs:comment     "This class comprises transfers of the physical custody or the legal responsibility for the physical custody of objects. The recording of the donor or recipient is optional. It is possible that in an instance of E10 Transfer of Custody there is either no donor or no recipient.\nDepending on the circumstances, it may describe:\n1. the beginning of custody (there is no previous custodian)\n2. the end of custody (there is no subsequent custodian)\n3. the transfer of custody (transfer from one custodian to the next)\n4. the receipt of custody from an unknown source (the previous custodian is unknown)\n5. the declared loss of an object (the current or subsequent custodian is unknown)\nIn the event that only a single kind of transfer of custody occurs, either the legal responsibility for the custody or the actual physical possession of the object but not both, this difference should be expressed using the property P2 has type (is type of).\nThe sense of physical possession requires that the object of custody be in the hands of the keeper at least with a part representative for the whole. The way, in which a representative part is defined, should ensure that it is unambiguous who keeps a part and who the whole and should be consistent with the identity criteria of the kept instance of E18 Physical Thing.\nThe interpretation of the museum notion of \"accession\" differs between institutions. The CIDOC CRM therefore models legal ownership and physical custody separately. Institutions will then model their specific notions of accession and deaccession as combinations of these.\nTheft is a specific case of illegal transfer of custody."@en;
        rdfs:subClassOf  <E7_Activity> .

<E11_Modification>  rdf:type  rdfs:Class;
        rdfs:label       "Modification"@en;
        rdfs:label       "Bearbeitung"@de;
        rdfs:label       "Τροποποίηση"@el;
        rdfs:label       "Modification"@fr;
        rdfs:label       "Modificação"@pt;
        rdfs:label       "Измeнeниe"@ru;
        rdfs:label       "修改"@zh;
        rdfs:comment     "This class comprises instances of E7 Activity that are undertaken to create, alter or change instances of E24 Physical Human-Made Thing.\nThis class includes the production of an item from raw materials and other so far undocumented objects. It also includes the conservation treatment of an object.\nSince the distinction between modification and production is not always clear, modification is regarded as the more generally applicable concept. This implies that some items may be consumed or destroyed in an instance of E11 Modification, and that others may be produced as a result of it. An event should also be documented using an instance of E81 Transformation if it results in the destruction of one or more objects and the simultaneous production of others using parts or material from the originals. In this case, the new items have separate identities.\nAn activity undertaken on an object which was designed to alter it, but which, in fact, it did not in any seemingly significant way (such as the application of a solvent during conservation which failed to dissolve any part of the object), is still considered as an instance of E11 Modification. Typically, any such activity will leave at least forensic traces of evidence on the object.\nIf the instance of E29 Design or Procedure utilized for the modification prescribes the use of specific materials, they should be documented using property P68 foresees use of (use foreseen by): E57 Material of E29 Design or Procedure, rather than via P126 employed (was employed in): E57 Material."@en;
        rdfs:subClassOf  <E7_Activity> .

<E12_Production>  rdf:type  rdfs:Class;
        rdfs:label       "Production"@en;
        rdfs:label       "Herstellung"@de;
        rdfs:label       "Παραγωγή"@el;
        rdfs:label       "Production"@fr;
        rdfs:label       "Produção"@pt;
        rdfs:label       "Изготовлeниe"@ru;
        rdfs:label       "生产"@zh;
        rdfs:comment     "This class comprises activities that are designed to, and succeed in, creating one or more new items.\nIt specializes the notion of modification into production. The decision as to whether or not an object is regarded as new is context sensitive. Normally, items are considered “new” if there is no obvious overall similarity between them and the consumed items and material used in their production. In other cases, an item is considered “new” because it becomes relevant to documentation by a modification. For example, the scribbling of a name on a potsherd may make it a voting token. The original potsherd may not be worth documenting, in contrast to the inscribed one.\nThis entity can be collective: the printing of a thousand books, for example, would normally be considered a single event.\nAn event should also be documented using an instance of E81 Transformation if it results in the destruction of one or more objects and the simultaneous production of others using parts or material from the originals. In this case, the new items have separate identities and matter is preserved, but identity is not."@en;
        rdfs:subClassOf  <E11_Modification>;
        rdfs:subClassOf  <E63_Beginning_of_Existence> .

<E13_Attribute_Assignment>
        rdf:type         rdfs:Class;
        rdfs:label       "Attribute Assignment"@en;
        rdfs:label       "Merkmalszuweisung"@de;
        rdfs:label       "Απόδοση Ιδιοτήτων"@el;
        rdfs:label       "Assignation d’attribut"@fr;
        rdfs:label       "Atribuição de Característica"@pt;
        rdfs:label       "Назначeниe Атрибута"@ru;
        rdfs:label       "属性赋值"@zh;
        rdfs:comment     "This class comprises the actions of making assertions about one property of an object or any single relation between two items or concepts. The type of the property asserted to hold between two items or concepts can be described by the property P177 assigned property of type (is type of property assigned): E55 Type.\nFor example, the class describes the actions of people making propositions and statements during certain scientific/scholarly procedures, e.g. the person and date when a condition statement was made, an identifier was assigned, the museum object was measured, etc. Which kinds of such assignments and statements need to be documented explicitly in structures of a schema rather than free text, depends on whether this information should be accessible by structured queries.\nThis class allows for the documentation of how the respective assignment came about, and whose opinion it was. Note that all instances of properties described in a knowledge base are the opinion of someone. Per default, they are the opinion of the team maintaining the knowledge base. This fact must not individually be registered for all instances of properties provided by the maintaining team, because it would result in an endless recursion of whose opinion was the description of an opinion. Therefore, the use of instances of E13 Attribute Assignment marks the fact that the maintaining team is in general neutral to the validity of the respective assertion, but registers someone else’s opinion and how it came about.\nAll properties assigned in such an action can also be seen as directly relating the respective pair of items or concepts. Multiple use of instances of E13 Attribute Assignment may possibly lead to a collection of contradictory values."@en;
        rdfs:subClassOf  <E7_Activity> .

<E14_Condition_Assessment>
        rdf:type         rdfs:Class;
        rdfs:label       "Condition Assessment"@en;
        rdfs:label       "Zustandsfeststellung"@de;
        rdfs:label       "Εκτίμηση Κατάστασης"@el;
        rdfs:label       "Évaluation d’état matériel"@fr;
        rdfs:label       "Avaliação do Estado Material"@pt;
        rdfs:label       "Оцeнка Состояния"@ru;
        rdfs:label       "状态评估"@zh;
        rdfs:comment     "This class describes the act of assessing the state of preservation of an object during a particular period.\nThe condition assessment may be carried out by inspection, measurement, or through historical research. This class is used to document circumstances of the respective assessment that is relevant to interpret its quality at a later stage, or to continue research on related documents."@en;
        rdfs:subClassOf  <E13_Attribute_Assignment> .

<E15_Identifier_Assignment>
        rdf:type         rdfs:Class;
        rdfs:label       "Identifier Assignment"@en;
        rdfs:label       "Kennzeichenzuweisung"@de;
        rdfs:label       "Απόδοση Αναγνωριστικού"@el;
        rdfs:label       "Assignation d’identifiant"@fr;
        rdfs:label       "Atribuição de Identificador"@pt;
        rdfs:label       "Назначeниe Идeнтификатора"@ru;
        rdfs:label       "标识符赋值"@zh;
        rdfs:comment     "This class comprises activities that result in the allocation of an identifier to an instance of E1 CRM Entity. An instance of E15 Identifier Assignment may include the creation of the identifier from multiple constituents, which themselves may be instances of E41 Appellation. The syntax and kinds of constituents to be used may be declared in a rule constituting an instance of E29 Design or Procedure.\nExamples of such identifiers include Find Numbers, Inventory Numbers, uniform titles in the sense of librarianship and Digital Object Identifiers (DOI). Documenting the act of identifier assignment and deassignment is especially useful when objects change custody or the identification system of an organization is changed. In order to keep track of the identity of things in such cases, it is important to document by whom, when, and for what purpose an identifier is assigned to an item.\nThe fact that an identifier is a preferred one for an organisation can be expressed by using the property E1 CRM Entity. P48 has preferred identifier (is preferred identifier of): E42 Identifier. It can better be expressed in a context independent form by assigning a suitable E55 Type, such as “preferred identifier assignment”, to the respective instance of E15 Identifier Assignment through the P2 has type (is type of) property."@en;
        rdfs:subClassOf  <E13_Attribute_Assignment> .

<E16_Measurement>  rdf:type  rdfs:Class;
        rdfs:label       "Measurement"@en;
        rdfs:label       "Messung"@de;
        rdfs:label       "Μέτρηση"@el;
        rdfs:label       "Mesurage"@fr;
        rdfs:label       "Medição"@pt;
        rdfs:label       "Измeрeниe"@ru;
        rdfs:label       "测量"@zh;
        rdfs:comment     "This class comprises actions measuring physical properties and other values that can be determined by a systematic, objective procedure of direct observation of particular states of physical reality.\nAn instance of E16 Measurement may use simple counting or tools, such as yardsticks or radiation detection devices. The interest is in the method and care applied, so that the reliability of the result may be judged at a later stage, or research continued on the associated documents. The date of the event is important for dimensions, which may change value over time, such as the length of an object subject to shrinkage. Methods and devices employed should be associated with instances of E16 Measurement by properties such as P33 used specific technique: E29 Design or Procedure, P125 used object of type: E55 Type, P16 used specific object (was used for): E70 Thing, whereas basic techniques such as \"carbon-14 dating\" should be encoded using P2 has type (is type of): E55 Type. Details of methods and devices reused or reusable in other instances of E16 Measurement should be documented for these entities rather than the measurements themselves, whereas details of particular execution may be documented by free text or by instantiating adequate sub-activities, if the detail may be of interest for an overarching query.\nRegardless whether a measurement is made by an instrument or by human senses, it represents the initial transition from physical reality to information without any other documented information object in between within the reasoning chain that would represent the result of the interaction of the observer or device with reality. Therefore, determining properties of an instance of E90 Symbolic Object is regarded as an instance of E13 Attribute Assignment, which may be inferred from observing and measuring representative carriers. In the case that the carrier can be named, the property P16 used specific object (was used for) should be used to indicate the instance(s) of E18 Physical Thing that was used as the empirical basis for the attribute assignment. For instance, inferring properties of depicted items using image material, such as satellite images, is not regarded as an instance of E16 Measurement, but as a subsequent instance of E13 Attribute Assignment. Rather, only the production of the images, understood as arrays of radiation intensities, is regarded as an instance of E16 Measurement. The same reasoning holds for other sensor data."@en;
        rdfs:subClassOf  <E13_Attribute_Assignment> .

<E17_Type_Assignment>
        rdf:type         rdfs:Class;
        rdfs:label       "Type Assignment"@en;
        rdfs:label       "Typuszuweisung"@de;
        rdfs:label       "Απόδοση Τύπου"@el;
        rdfs:label       "Assignation de type"@fr;
        rdfs:label       "Atribuição de Tipo"@pt;
        rdfs:label       "Назначeниe Типа"@ru;
        rdfs:label       "类型赋值"@zh;
        rdfs:comment     "This class comprises the actions of classifying items of whatever kind. Such items include objects, specimens, people, actions, and concepts.\nThis class allows for the documentation of the context of classification acts in cases where the value of the classification depends on the personal opinion of the classifier, and the date that the classification was made. This class also encompasses the notion of “determination,” i.e. the systematic and molecular identification of a specimen in biology."@en;
        rdfs:subClassOf  <E13_Attribute_Assignment> .

<E18_Physical_Thing>  rdf:type  rdfs:Class;
        rdfs:label       "Physical Thing"@en;
        rdfs:label       "Materielles"@de;
        rdfs:label       "Υλικό Πράγμα"@el;
        rdfs:label       "Chose matérielle"@fr;
        rdfs:label       "Coisa Material"@pt;
        rdfs:label       "Матeриальный Прeдмeт"@ru;
        rdfs:label       "实物"@zh;
        rdfs:comment     "This class comprises all persistent physical items with a relatively stable form, human-made or natural.\nDepending on the existence of natural boundaries of such things, the CIDOC CRM distinguishes the instances of E19 Physical Object from instances of E26 Physical Feature, such as holes, rivers, pieces of land, etc. Most instances of E19 Physical Object can be moved (if not too heavy), whereas features are integral to the surrounding matter.\nAn instance of E18 Physical Thing occupies not only a particular geometric space at any instant of its existence, but in the course of its existence it also forms a trajectory through spacetime, which occupies a real, that is phenomenal, volume in spacetime. We include in the occupied space the space filled by the matter of the physical thing and all its inner spaces, such as the interior of a box. For the purpose of more detailed descriptions of the presence of an instance of E18 Physical Thing in space and time it can be associated with its specific instance of E92 Spacetime Volume by the property P196 defines (is defined by).\nThe CIDOC CRM is generally not concerned with amounts of matter in fluid or gaseous states, as long as they are not confined in an identifiable way for an identifiable minimal time-span."@en;
        rdfs:subClassOf  <E72_Legal_Object> .

<E19_Physical_Object>
        rdf:type         rdfs:Class;
        rdfs:label       "Physical Object"@en;
        rdfs:label       "Materieller Gegenstand"@de;
        rdfs:label       "Υλικό Αντικείμενο"@el;
        rdfs:label       "Objet matériel"@fr;
        rdfs:label       "Objeto Material"@pt;
        rdfs:label       "Матeриальный Объeкт"@ru;
        rdfs:label       "物质对象"@zh;
        rdfs:comment     "This class comprises items of a material nature that are units for documentation and have physical boundaries that separate them completely in an objective way from other objects.\nThe class also includes all aggregates of objects made for functional purposes of whatever kind, independent of physical coherence, such as a set of chessmen. Typically, instances of E19 Physical Object can be moved (if not too heavy).\nIn some contexts, such objects, except for aggregates, are also called “bona fide objects”, i.e. naturally defined objects (Smith &amp; Varzi, 2000).\nThe decision as to what is documented as a complete item, rather than by its parts or components, may be purely administrative or may be a result of the order in which the item was acquired."@en;
        rdfs:subClassOf  <E18_Physical_Thing> .

<E20_Biological_Object>
        rdf:type         rdfs:Class;
        rdfs:label       "Biological Object"@en;
        rdfs:label       "Biologischer Gegenstand"@de;
        rdfs:label       "Βιολογικό Ακτικείμενο"@el;
        rdfs:label       "Objet biologique"@fr;
        rdfs:label       "Objeto Biológico"@pt;
        rdfs:label       "Биологичeский Объeкт"@ru;
        rdfs:label       "生物对象"@zh;
        rdfs:comment     "This class comprises individual items of a material nature, which live, have lived, or are natural products of or from living organisms.\nArtificial objects that incorporate biological elements, such as Victorian butterfly frames, can be documented as both instances of E20 Biological Object and E22 Human-Made Object."@en;
        rdfs:subClassOf  <E19_Physical_Object> .

<E21_Person>  rdf:type   rdfs:Class;
        rdfs:label       "Person"@en;
        rdfs:label       "Person"@de;
        rdfs:label       "Πρόσωπο"@el;
        rdfs:label       "Personne"@fr;
        rdfs:label       "Pessoa"@pt;
        rdfs:label       "Личность"@ru;
        rdfs:label       "人物"@zh;
        rdfs:comment     "This class comprises real persons who live or are assumed to have lived.\nLegendary figures that may have existed, such as Ulysses and King Arthur, fall into this class if the documentation refers to them as historical figures. In cases where doubt exists as to whether several persons are in fact identical, multiple instances can be created and linked to indicate their relationship. The CIDOC CRM does not propose a specific form to support reasoning about possible identity.\nIn a bibliographic context, a name presented following the conventions usually employed for personal names will be assumed to correspond to an actual real person (an instance of E21 Person), unless evidence is available to indicate that this is not the case. The fact that a persona may erroneously be classified as an instance of E21 Person does not imply that the concept comprises personae."@en;
        rdfs:subClassOf  <E20_Biological_Object>;
        rdfs:subClassOf  <E39_Actor> .

<E22_Human-Made_Object>
        rdf:type         rdfs:Class;
        rdfs:label       "Human-Made Object"@en;
        rdfs:label       "Objet élaboré par l’humain"@fr;
        rdfs:label       "Рукотворный Объeкт"@ru;
        rdfs:comment     "This class comprises all persistent physical objects of any size that are purposely created by human activity and have physical boundaries that separate them completely in an objective way from other objects.\nThe class also includes all aggregates of objects made for functional purposes of whatever kind, independent of physical coherence, such as a set of chessmen."@en;
        rdfs:subClassOf  <E19_Physical_Object>;
        rdfs:subClassOf  <E24_Physical_Human-Made_Thing> .

<E24_Physical_Human-Made_Thing>
        rdf:type         rdfs:Class;
        rdfs:label       "Physical Human-Made Thing"@en;
        rdfs:label       "Chose matérielle élaborée par l’humain"@fr;
        rdfs:label       "Матeриальный Рукотворный Объeкт"@ru;
        rdfs:comment     "This class comprises all persistent physical items of any size that are purposely created by human activity. This class comprises, besides others, human-made objects, such as a sword, and human-made features, such as rock art. For example, a “cup and ring” carving on bedrock is regarded as instance of E24 Physical Human-Made Thing.\nInstances of E24 Physical Human-Made Thing may be the result of modifying pre-existing physical things, preserving larger parts or most of the original matter and structure, which poses the question if they are new or even human-made, the respective interventions of production made on such original material should be obvious and sufficient to regard that the product has a new, distinct identity and intended function and is human-made. Substantial continuity of the previous matter and structure in the new product can be documented by describing the production process also as an instance of E81 Transformation.\nWhereas interventions of conservation and repair are not regarded to produce a new instance of E24 Physical Human-Made Thing, the results of preparation of natural history specimens that substantially change their natural or original state should be regarded as instances of E24 Physical Human-Made Things, including the uncovering of petrified biological features from a solid piece of stone. On the other side, scribbling a museum number on a natural object should not be regarded to make it human-made. This notwithstanding, parts, sections, segments, or features of an instance of E24 Physical Human-Made Thing may continue to be non-human-made and preserved during the production process, for example natural pearls used as a part of an eardrop."@en;
        rdfs:subClassOf  <E18_Physical_Thing>;
        rdfs:subClassOf  <E71_Human-Made_Thing> .

<E25_Human-Made_Feature>
        rdf:type         rdfs:Class;
        rdfs:label       "Human-Made Feature"@en;
        rdfs:label       "Caractéristique élaborée par l'humain"@fr;
        rdfs:label       "Искусствeнный Признак"@ru;
        rdfs:comment     "This class comprises physical features that are purposely created by human activity, such as scratches, artificial caves, artificial water channels, etc. In particular, it includes the information encoding features on mechanical or digital carriers."@en;
        rdfs:subClassOf  <E24_Physical_Human-Made_Thing>;
        rdfs:subClassOf  <E26_Physical_Feature> .

<E26_Physical_Feature>
        rdf:type         rdfs:Class;
        rdfs:label       "Physical Feature"@en;
        rdfs:label       "Materielles Merkmal"@de;
        rdfs:label       "Υλικό Μόρφωμα"@el;
        rdfs:label       "Caractéristique physique"@fr;
        rdfs:label       "Característica Material"@pt;
        rdfs:label       "Физичeский Признак"@ru;
        rdfs:label       "物理特征"@zh;
        rdfs:comment     "This class comprises identifiable features that are physically attached in an integral way to particular physical objects.\nInstances of E26 Physical Feature share many of the attributes of instances of E19 Physical Object. They may have a one-dimensional, two-dimensional, or three-dimensional geometric extent, but there are no natural borders that separate them completely in an objective way from the carrier objects. For example, a doorway is a feature but the door itself, being attached by hinges, is not.\nInstances of E26 Physical Feature can be features in a narrower sense, such as scratches, holes, reliefs, surface colours, reflection zones in an opal crystal or a density change in a piece of wood. In the wider sense, they are portions of particular objects with partially imaginary borders, such as the core of the Earth, an area of property on the surface of the Earth, a landscape or the head of a contiguous marble statue. They can be measured and dated, and it is sometimes possible to state who or what is or was responsible for them. They cannot be separated from the carrier object, but a segment of the carrier object may be identified (or sometimes removed) carrying the complete feature.\nThis definition coincides with the definition of “fiat objects”, with the exception of aggregates of “bona fide objects” (Smith &amp; Varzi, 2000)."@en;
        rdfs:subClassOf  <E18_Physical_Thing> .

<E27_Site>  rdf:type     rdfs:Class;
        rdfs:label       "Site"@en;
        rdfs:label       "Gelände"@de;
        rdfs:label       "Φυσικός Χώρος"@el;
        rdfs:label       "Site"@fr;
        rdfs:label       "Lugar"@pt;
        rdfs:label       "Мeстоположeниe"@ru;
        rdfs:label       "场地"@zh;
        rdfs:comment     "This class comprises pieces of land or sea floor.\nIn contrast to the purely geometric notion of E53 Place, this class describes constellations of matter on the surface of the Earth or other celestial body, which can be represented by photographs, paintings, and maps.\nInstances of E27 Site are composed of relatively immobile material items and features in a particular configuration at a particular location."@en;
        rdfs:subClassOf  <E26_Physical_Feature> .

<E28_Conceptual_Object>
        rdf:type         rdfs:Class;
        rdfs:label       "Conceptual Object"@en;
        rdfs:label       "Begrifflicher Gegenstand"@de;
        rdfs:label       "Νοητικό Αντικείμενο"@el;
        rdfs:label       "Objet conceptuel"@fr;
        rdfs:label       "Objeto Conceitual"@pt;
        rdfs:label       "Концeптуальный Объeкт"@ru;
        rdfs:label       "概念对象"@zh;
        rdfs:comment     "This class comprises non-material products of our minds and other human produced data that have become objects of a discourse about their identity, circumstances of creation, or historical implication. The production of such information might have been supported by the use of technical devices such as cameras or computers.\nCharacteristically, instances of this class are created, invented or thought by someone, and then may be documented or communicated between persons. Instances of E28 Conceptual Object have the ability to exist on more than one particular carrier at the same time, such as paper, electronic signals, marks, audio media, paintings, photos, human memories, etc.\nThey cannot be destroyed. They exist as long as they can be found on at least one carrier or in at least one human memory. Their existence ends when the last carrier and the last memory are lost."@en;
        rdfs:subClassOf  <E71_Human-Made_Thing> .

<E29_Design_or_Procedure>
        rdf:type         rdfs:Class;
        rdfs:label       "Design or Procedure"@en;
        rdfs:label       "Entwurf oder Verfahren"@de;
        rdfs:label       "Σχέδιο"@el;
        rdfs:label       "Conceptualisation ou procédure"@fr;
        rdfs:label       "Projeto ou Procedimento"@pt;
        rdfs:label       "Проeкт или Процeдура"@ru;
        rdfs:label       "设计或程序"@zh;
        rdfs:comment     "This class comprises documented plans for the execution of actions in order to achieve a result of a specific quality, form, or contents. In particular, it comprises plans for deliberate human activities that may result in new instances of E71 Human-Made Thing or for shaping or guiding the execution of an instance of E7 Activity.\nInstances of E29 Design or Procedure can be structured in parts and sequences or depend on others.\nThis is modelled using P69 has association with (is associated with): E29 Design or Procedure.\nDesigns or procedures can be seen as one of the following:\n1. A schema for the activities it describes\n2. A schema of the products that result from their application\n3. An independent intellectual product that may have never been applied, such as Leonardo da Vinci’s famous plans for flying machines\nBecause designs or procedures may never be applied or only partially executed, the CIDOC CRM models a loose relationship between the plan and the respective product."@en;
        rdfs:subClassOf  <E73_Information_Object> .

<E30_Right>  rdf:type    rdfs:Class;
        rdfs:label       "Right"@en;
        rdfs:label       "Recht"@de;
        rdfs:label       "Δικαίωμα"@el;
        rdfs:label       "Droit"@fr;
        rdfs:label       "Direitos"@pt;
        rdfs:label       "Право"@ru;
        rdfs:label       "权限"@zh;
        rdfs:comment     "This class comprises legal privileges concerning material and immaterial things or their derivatives.\nThese include reproduction and property rights."@en;
        rdfs:subClassOf  <E89_Propositional_Object> .

<E31_Document>  rdf:type  rdfs:Class;
        rdfs:label       "Document"@en;
        rdfs:label       "Dokument"@de;
        rdfs:label       "Τεκμήριο"@el;
        rdfs:label       "Document"@fr;
        rdfs:label       "Documento"@pt;
        rdfs:label       "Докумeнт"@ru;
        rdfs:label       "文献"@zh;
        rdfs:comment     "This class comprises identifiable immaterial items that make propositions about reality.\nThese propositions may be expressed in text, graphics, images, audiograms, videograms, or by other similar means. Documentation databases are regarded as instances of E31 Document. This class should not be confused with the concept “document” in Information Technology, which is compatible with E73 Information Object."@en;
        rdfs:subClassOf  <E73_Information_Object> .

<E32_Authority_Document>
        rdf:type         rdfs:Class;
        rdfs:label       "Authority Document"@en;
        rdfs:label       "Referenzdokument"@de;
        rdfs:label       "Πηγή Καθιερωμένων Όρων"@el;
        rdfs:label       "Document de référence"@fr;
        rdfs:label       "Documento de Referência"@pt;
        rdfs:label       "Официальный Докумeнт"@ru;
        rdfs:label       "规范文档"@zh;
        rdfs:comment     "This class comprises encyclopaedia, thesauri, authority lists and other documents that define terminology or conceptual systems for consistent use."@en;
        rdfs:subClassOf  <E31_Document> .

<E33_Linguistic_Object>
        rdf:type         rdfs:Class;
        rdfs:label       "Linguistic Object"@en;
        rdfs:label       "Sprachlicher Gegenstand"@de;
        rdfs:label       "Γλωσσικό Αντικείμενο"@el;
        rdfs:label       "Objet linguistique"@fr;
        rdfs:label       "Objeto Lingüístico"@pt;
        rdfs:label       "Лингвистичeский Объeкт"@ru;
        rdfs:label       "语言对象"@zh;
        rdfs:comment     "This class comprises identifiable expressions in natural language or languages.\nInstances of E33 Linguistic Object can be expressed in many ways: e.g. as written texts, recorded speech, or sign language. However, the CIDOC CRM treats instances of E33 Linguistic Object independently from the medium or method by which they are expressed. Expressions in formal languages, such as computer code or mathematical formulae, are not treated as instances of E33 Linguistic Object by the CIDOC CRM. These should be modelled as instances of E73 Information Object.\nIn general, an instance of E33 Linguistic Object may also contain non-linguistic information, often of artistic or aesthetic value. Only in cases in which the content of an instance of E33 Linguistic Object can completely be expressed by a series of binary-encoded symbols, its content may be documented within a respective knowledge base by the property P190 has symbolic content: E62 String. Otherwise, it should be understood as an identifiable digital resource only available independently from the respective knowledge base.\nIn other cases, such as pages of an illuminated manuscript or recordings containing speech in a language supported by a writing system, the linguistic part of the content of an instance of E33 Linguistic Object may be documented within a respective knowledge base in a note by P3 has note: E62 String. Otherwise, it may be described using the property P165 incorporates (is incorporated in): E73 Information Object as a different object with its own identity."@en;
        rdfs:subClassOf  <E73_Information_Object> .

<E33_E41_Linguistic_Appellation>
        rdf:type         rdfs:Class;
        rdfs:label       "Linguistic Appellation"@en;
        rdfs:subClassOf  <E33_Linguistic_Object>;
        rdfs:subClassOf  <E41_Appellation> .

<E34_Inscription>  rdf:type  rdfs:Class;
        rdfs:label       "Inscription"@en;
        rdfs:label       "Inschrift"@de;
        rdfs:label       "Επιγραφή"@el;
        rdfs:label       "Inscription"@fr;
        rdfs:label       "Inscrição"@pt;
        rdfs:label       "Надпись"@ru;
        rdfs:label       "题识"@zh;
        rdfs:comment     "This class comprises recognisable texts that can be attached to instances of E24 Physical Human-Made Thing.\nThe transcription of the text can be documented in a note by P3 has note: E62 String. The alphabet used can be documented by P2 has type: E55 Type. This class is not intended to describe the idiosyncratic characteristics of an individual physical embodiment of an inscription, but the underlying prototype. The physical embodiment is modelled in the CIDOC CRM as instances of E24 Physical Human-Made Thing.\nThe relationship of a physical copy of a book to the text it contains is modelled using E18 Physical Thing. P128 carries (is carried by): E33 Linguistic Object."@en;
        rdfs:subClassOf  <E33_Linguistic_Object>;
        rdfs:subClassOf  <E37_Mark> .

<E35_Title>  rdf:type    rdfs:Class;
        rdfs:label       "Title"@en;
        rdfs:label       "Titel"@de;
        rdfs:label       "Τίτλος"@el;
        rdfs:label       "Titre"@fr;
        rdfs:label       "Título"@pt;
        rdfs:label       "Названиe"@ru;
        rdfs:label       "题名"@zh;
        rdfs:comment     "This class comprises the textual strings that within a cultural context can be clearly identified as titles due to their form. Being a subclass of E41 Appellation, E35 Title can only be used when such a string is actually used as a title of a work, such as a text, an artwork, or a piece of music.\nTitles are proper noun phrases or verbal phrases, and should not be confused with generic object names such as “chair”, “painting”, or “book” (the latter are common nouns that stand for instances of E55 Type). Titles may be assigned by the creator of the work itself, or by a social group.\nThis class also comprises the translations of titles that are used as surrogates for the original titles in different social contexts."@en;
        rdfs:subClassOf  <E33_Linguistic_Object>;
        rdfs:subClassOf  <E41_Appellation> .

<E36_Visual_Item>  rdf:type  rdfs:Class;
        rdfs:label       "Visual Item"@en;
        rdfs:label       "Bildliches"@de;
        rdfs:label       "Οπτικό Στοιχείο"@el;
        rdfs:label       "Entité visuelle"@fr;
        rdfs:label       "Item Visual"@pt;
        rdfs:label       "Визуальный Прeдмeт"@ru;
        rdfs:label       "可视项"@zh;
        rdfs:comment     "This class comprises the intellectual or conceptual aspects of recognisable marks and images.\nThis class does not intend to describe the idiosyncratic characteristics of an individual physical embodiment of a visual item, but the underlying prototype. For example, a mark such as the ICOM logo is generally considered to be the same logo when used on any number of publications. The size, orientation, and colour may change, but the logo remains uniquely identifiable. The same is true of images that are reproduced many times. This means that visual items are independent of their physical support.\nThe E36 Visual Item class provides a means of identifying and linking together instances of E24 Physical Human-Made Thing that carry the same visual symbols, marks, or images, etc. The property P62 depicts (is depicted by) between E24 Physical Human-Made Thing and the depicted subjects (E1 CRM Entity) can be regarded as a shortcut of the more fully developed path from E24 Physical Human-Made Thing through P65 shows visual item (is shown by), E36 Visual Item, P138 represents (has representation) to E1 CRM Entity, which in addition captures the optical features of the depiction."@en;
        rdfs:subClassOf  <E73_Information_Object> .

<E37_Mark>  rdf:type     rdfs:Class;
        rdfs:label       "Mark"@en;
        rdfs:label       "Marke"@de;
        rdfs:label       "Σήμανση"@el;
        rdfs:label       "Marque"@fr;
        rdfs:label       "Marca"@pt;
        rdfs:label       "Знак"@ru;
        rdfs:label       "标记"@zh;
        rdfs:comment     "This class comprises symbols, signs, signatures, or short texts applied to instances of E24 Physical Human-Made Thing by arbitrary techniques, often in order to indicate such things as creator, owner, dedications, purpose, or to communicate information generally. Instances of E37 Mark do not represent the actual image of a mark, but the abstract ideal (or archetype) as used for codification in reference documents forming cultural documentation.\nThis class specifically excludes features that have no semantic significance, such as scratches or tool marks. These should be documented as instances of E25 Human-Made Feature."@en;
        rdfs:subClassOf  <E36_Visual_Item> .

<E39_Actor>  rdf:type    rdfs:Class;
        rdfs:label       "Actor"@en;
        rdfs:label       "Akteur"@de;
        rdfs:label       "Δράστης"@el;
        rdfs:label       "Actant"@fr;
        rdfs:label       "Agente"@pt;
        rdfs:label       "Дeйствующий Субъeкт"@ru;
        rdfs:label       "参与者"@zh;
        rdfs:comment     "This class comprises people, either individually or in groups, who have the potential to perform intentional actions of kinds for which they can be held responsible."@en;
        rdfs:subClassOf  <E77_Persistent_Item> .

<E41_Appellation>  rdf:type  rdfs:Class;
        rdfs:label       "Appellation"@en;
        rdfs:label       "Benennung"@de;
        rdfs:label       "Ονομασία"@el;
        rdfs:label       "Appellation"@fr;
        rdfs:label       "Designação"@pt;
        rdfs:label       "Обозначeниe"@ru;
        rdfs:label       "称谓"@zh;
        rdfs:comment     "This class comprises all signs, either meaningful or not, or arrangements of signs following a specific syntax, that are used or can be used to refer to and identify a specific instance of some class within a certain context.\nInstances of E41 Appellation do not identify things by their meaning, even if they happen to have one, but by convention, tradition, or agreement. Instances of E41 Appellation are cultural constructs; as such, they have a context, a history, and a use in time and space by some group of users. A given instance of E41 Appellation can have alternative forms, i.e. other instances of E41 Appellation that are regarded as equivalent, regardless of the thing it denotes.\nDifferent languages may use different appellations for the same thing, such as the names of major cities. Some appellations may be formulated using a valid noun phrase of a particular language. In these cases, the respective instances of E41 Appellation should also be declared as instances of E33 Linguistic Object. Then the language using the appellation can be declared with the property P72 has language: E56 Language.\nInstances of E41 Appellation may be used to identify any instance of E1 CRM Entity and sometimes are characteristic for instances of more specific subclasses of E1 CRM Entity, such as for instances of E52 Time-Span (for instance “dates”), E39 Actor, E53 Place or E28 Conceptual Object. Postal addresses and E-mail addresses are characteristic examples of identifiers used by services transporting things between clients.\nEven numerically expressed identifiers for extents in space or time are also regarded as instances of E41 Appellation, such as Gregorian dates or spatial coordinates, even though they allow for determining some time or location by a known procedure starting from a reference point and by virtue of that fact play a double role as instances of E59 Primitive Value.\nE41 Appellation should not be confused with the act of naming something. Cf. E15 Identifier Assignment."@en;
        rdfs:subClassOf  <E90_Symbolic_Object> .

<E42_Identifier>  rdf:type  rdfs:Class;
        rdfs:label       "Identifier"@en;
        rdfs:label       "Kennung"@de;
        rdfs:label       "Κωδικός Αναγνώρισης"@el;
        rdfs:label       "Identifiant"@fr;
        rdfs:label       "Identificador de Objeto"@pt;
        rdfs:label       "Идeнтификатор"@ru;
        rdfs:label       "标识符"@zh;
        rdfs:comment     "This class comprises strings or codes assigned to instances of E1 CRM Entity in order to identify them uniquely and permanently within the context of one or more organisations. Such codes are often known as inventory numbers, registration codes, etc. and are typically composed of alphanumeric sequences. Postal addresses, telephone numbers, URLs and e-mail addresses are characteristic examples of identifiers used by services transporting things between clients.\nThe class E42 Identifier is not normally used for machine-generated identifiers used for automated processing unless these are also used by human agents."@en;
        rdfs:subClassOf  <E41_Appellation> .

<E52_Time-Span>  rdf:type  rdfs:Class;
        rdfs:label       "Time-Span"@en;
        rdfs:label       "Zeitspanne"@de;
        rdfs:label       "Χρονικό Διάστημα"@el;
        rdfs:label       "Intervalle temporel"@fr;
        rdfs:label       "Período de Tempo"@pt;
        rdfs:label       "Интeрвал Врeмeни"@ru;
        rdfs:label       "时段"@zh;
        rdfs:comment     "This class comprises abstract temporal extents, in the sense of Galilean physics, having a beginning, an end, and a duration.\nInstances of E52 Time-Span have no semantic connotations about phenomena happening within the temporal extent they represent. They do not convey any meaning other than a positioning on the “time-line” of chronology. The actual extent of an instance of E52 Time-Span can be approximated by properties of E52 Time-Span giving inner and outer bounds in the form of dates (instances of E61 Time Primitive). Comparing knowledge about time-spans is fundamental for chronological reasoning.\nSome instances of E52 Time-Span may be defined as the actual, in principle observable, temporal extent of instances of E2 Temporal Entity via the property P4 has time-span (is time-span of): E52 Time-Span. They constitute phenomenal time-spans as defined in CRMgeo (Doerr &amp; Hiebel 2013). Since our knowledge of history is imperfect and physical phenomena are fuzzy in nature, the extent of phenomenal time-spans can only be described in approximation. An extreme case of approximation, might, for example, define an instance of E52 Time-Span having unknown beginning, end and duration. It may, nevertheless, be associated with other descriptions by which people can infer knowledge about it, such as in relative chronologies.\nSome instances of E52 may be defined precisely as representing a declaration of a temporal extent, as, for instance, done in a business contract. They constitute declarative time-spans as defined in CRMgeo (Doerr &amp; Hiebel 2013) and can be described via the property E61 Time Primitive P170 defines time (time is defined by): E52 Time-Span.\nWhen used as a common E52 Time-Span for two events, it will nevertheless describe them as being simultaneous, even if nothing else is known."@en;
        rdfs:subClassOf  <E1_CRM_Entity> .

<E53_Place>  rdf:type    rdfs:Class;
        rdfs:label       "Place"@en;
        rdfs:label       "Ort"@de;
        rdfs:label       "Τόπος"@el;
        rdfs:label       "Lieu"@fr;
        rdfs:label       "Local"@pt;
        rdfs:label       "Мeсто"@ru;
        rdfs:label       "地点"@zh;
        rdfs:comment     "This class comprises extents in the natural space where people live, in particular on the surface of the Earth, in the pure sense of physics: independent from temporal phenomena and matter. They may serve describing the physical location of things or phenomena or other areas of interest. Geometrically, instances of E53 Place constitute single contiguous areas or a finite aggregation of disjoint areas in space which are each individually contiguous. They may have fuzzy boundaries.\nThe instances of E53 Place are usually determined by reference to the position of “immobile” objects such as buildings, cities, mountains, rivers, or dedicated geodetic marks, but may also be determined by reference to mobile objects. A Place can be determined by combining a frame of reference and a location with respect to this frame.\nIt is sometimes argued that instances of E53 Place are best identified by global coordinates or absolute reference systems. However, relative references are often more relevant in the context of cultural documentation and tend to be more precise. In particular, people are often interested in position in relation to large, mobile objects, such as ships. For example, the Place at which Nelson died is known with reference to a large mobile object, i.e. H.M.S Victory. A resolution of this Place in terms of absolute coordinates would require knowledge of the movements of the vessel and the precise time of death, either of which may be revised, and the result would lack historical and cultural relevance.\nAny instance of E18 Physical Thing can serve as a frame of reference for an instance of E53 Place. This may be documented using the property P157 is at rest relative to (provides reference space for)."@en;
        rdfs:subClassOf  <E1_CRM_Entity> .

<E54_Dimension>  rdf:type  rdfs:Class;
        rdfs:label       "Dimension"@en;
        rdfs:label       "Maß"@de;
        rdfs:label       "Μέγεθος"@el;
        rdfs:label       "Dimension"@fr;
        rdfs:label       "Dimensão"@pt;
        rdfs:label       "Размeр"@ru;
        rdfs:label       "度量规格"@zh;
        rdfs:comment     "This class comprises quantifiable properties that can be measured by some calibrated means and can be approximated by values, i.e. points or regions in a mathematical or conceptual space, such as natural or real numbers, RGB values, etc.\nAn instance of E54 Dimension represents the empirical or theoretically derived quantity, including the precision tolerances resulting from the particular method or calculation. The identity of an instance of E54 Dimension depends on the method of its determination because each method may produce different values even when determining comparable qualities. For instance, the wingspan of a bird alive or dead is a different dimension. Thermoluminescence dating and Rehydroxylation [RHX] dating are different dimensions of temporal distance from now, even if they aim at dating the same object. The method of determination should be expressed using the property P2 has type (is type of). Note that simple terms such as “diameter” or “length” are normally insufficient to unambiguously describe a respective dimension. In contrast, “maximum linear extent” may be sufficient.\nThe properties of the class E54 Dimension allow for expressing the numerical approximation of the values of instances of E54 Dimension adequate to the precision of the applied method of determination. If the respective quantity belongs to a non-discrete space according to the laws of physics, such as spatial distances, it is recommended to record them as approximations by intervals or regions of indeterminacy enclosing the assumed true values. For instance, a length of 5 cm may be recorded as 4.5-5.5 cm, according to the precision of the respective observation. Note, that comparability of values described in different units depends critically on the representation as value regions.\nNumerical approximations in archaic instances of E58 Measurement Unit used in historical records should be preserved. Equivalents corresponding to current knowledge should be recorded as additional instances of E54 Dimension, as appropriate."@en;
        rdfs:subClassOf  <E1_CRM_Entity> .

<E55_Type>  rdf:type     rdfs:Class;
        rdfs:label       "Type"@en;
        rdfs:label       "Typus"@de;
        rdfs:label       "Τύπος"@el;
        rdfs:label       "Type"@fr;
        rdfs:label       "Tipo"@pt;
        rdfs:label       "Tип"@ru;
        rdfs:label       "类型"@zh;
        rdfs:comment     "This class comprises concepts denoted by terms from thesauri and controlled vocabularies used to characterize and classify instances of CIDOC CRM classes. Instances of E55 Type represent concepts, in contrast to instances of E41 Appellation which are used to name instances of CIDOC CRM classes.\nE55 Type provides an interface to domain specific ontologies and thesauri. These can be represented in the CIDOC CRM as subclasses of E55 Type, forming hierarchies of terms, i.e. instances of E55 Type linked via P127 has broader term (has narrower term): E55 Type. Such hierarchies may be extended with additional properties."@en;
        rdfs:subClassOf  <E28_Conceptual_Object> .

<E56_Language>  rdf:type  rdfs:Class;
        rdfs:label       "Language"@en;
        rdfs:label       "Sprache"@de;
        rdfs:label       "Γλώσσα"@el;
        rdfs:label       "Langue"@fr;
        rdfs:label       "Língua"@pt;
        rdfs:label       "Язык"@ru;
        rdfs:label       "语种"@zh;
        rdfs:comment     "This class is a specialization of E55 Type and comprises the natural languages in the sense of concepts.\nThis type is used categorically in the model without reference to instances of it, i.e. the Model does not foresee the description of instances of instances of E56 Language, e.g. “instances of Mandarin Chinese”.\nIt is recommended that internationally or nationally agreed codes and terminology should be used to denote instances of E56 Language, such as those defined in ISO 639-3:2007 and later versions."@en;
        rdfs:subClassOf  <E55_Type> .

<E57_Material>  rdf:type  rdfs:Class;
        rdfs:label       "Material"@en;
        rdfs:label       "Material"@de;
        rdfs:label       "Υλικό"@el;
        rdfs:label       "Matériau"@fr;
        rdfs:label       "Material"@pt;
        rdfs:label       "Матeриал"@ru;
        rdfs:label       "材质"@zh;
        rdfs:comment     "This class is a specialization of E55 Type and comprises the concepts of materials.\nInstances of E57 Material may denote properties of matter before its use, during its use, and as incorporated in an object, such as ultramarine powder, tempera paste, reinforced concrete. Discrete pieces of raw-materials kept in museums, such as bricks, sheets of fabric, pieces of metal, should be modelled individually in the same way as other objects. Discrete used or processed pieces, such as the stones from Nefer Titi's temple, should be modelled as parts (cf. P46 is composed of (forms part of): E18 Physical Thing).\nThis type is used categorically in the model without reference to instances of it, i.e. the Model does not foresee the description of instances of instances of E57 Material, e.g. “instances of gold”.\nIt is recommended that internationally or nationally agreed codes and terminology should be used."@en;
        rdfs:subClassOf  <E55_Type> .

<E58_Measurement_Unit>
        rdf:type         rdfs:Class;
        rdfs:label       "Measurement Unit"@en;
        rdfs:label       "Maßeinheit"@de;
        rdfs:label       "Μονάδα Μέτρησης"@el;
        rdfs:label       "Unité de mesure"@fr;
        rdfs:label       "Unidade de Medida"@pt;
        rdfs:label       "Eдиница Измeрeния"@ru;
        rdfs:label       "测量单位"@zh;
        rdfs:comment     "This class is a specialization of E55 Type and comprises the types of measurement units: feet, inches, centimetres, litres, lumens, etc.\nThis type is used categorically in the model without reference to instances of it, i.e. the model does not foresee the description of instances of instances of E58 Measurement Unit, e.g. “instances of cm”.\nSystème International (SI) units or internationally recognized non-SI terms should be used whenever possible, such as those defined by ISO80000:2009. Archaic Measurement Units used in historical records should be preserved."@en;
        rdfs:subClassOf  <E55_Type> .

<E63_Beginning_of_Existence>
        rdf:type         rdfs:Class;
        rdfs:label       "Beginning of Existence"@en;
        rdfs:label       "Daseinsbeginn"@de;
        rdfs:label       "Αρχή Ύπαρξης"@el;
        rdfs:label       "Début d’existence"@fr;
        rdfs:label       "Início da Existência"@pt;
        rdfs:label       "Начало Сущeствования"@ru;
        rdfs:label       "初始"@zh;
        rdfs:comment     "This class comprises events that bring into existence any instance of E77 Persistent Item.\nIt may be used for temporal reasoning about things (intellectual products, physical items, groups of people, living beings) beginning to exist; it serves as a hook for both a terminus post quem and a terminus ante quem."@en;
        rdfs:subClassOf  <E5_Event> .

<E64_End_of_Existence>
        rdf:type         rdfs:Class;
        rdfs:label       "End of Existence"@en;
        rdfs:label       "Daseinsende"@de;
        rdfs:label       "Τέλος Ύπαρξης"@el;
        rdfs:label       "Fin d’existence"@fr;
        rdfs:label       "Fim da Existência"@pt;
        rdfs:label       "Конeц Сущeствования"@ru;
        rdfs:label       "结束"@zh;
        rdfs:comment     "This class comprises events that end the existence of any instance of E77 Persistent Item.\nIt may be used for temporal reasoning about things (physical items, groups of people, living beings) ceasing to exist; it serves as a hook both a terminus post quem and a terminus ante quem. In cases where substance from an instance of E77 Persistent Item continues to exist in a new form, the process would be documented as instances of E81 Transformation."@en;
        rdfs:subClassOf  <E5_Event> .

<E65_Creation>  rdf:type  rdfs:Class;
        rdfs:label       "Creation"@en;
        rdfs:label       "Begriffliche Schöpfung"@de;
        rdfs:label       "Δημιουργία"@el;
        rdfs:label       "Création"@fr;
        rdfs:label       "Criação"@pt;
        rdfs:label       "Созданиe"@ru;
        rdfs:label       "创建"@zh;
        rdfs:comment     "This class comprises events that result in the creation of conceptual items or immaterial products, such as legends, poems, texts, music, images, movies, laws, types, etc."@en;
        rdfs:subClassOf  <E7_Activity>;
        rdfs:subClassOf  <E63_Beginning_of_Existence> .

<E66_Formation>  rdf:type  rdfs:Class;
        rdfs:label       "Formation"@en;
        rdfs:label       "Gruppenbildung"@de;
        rdfs:label       "Συγκρότηση Ομάδας"@el;
        rdfs:label       "Formation"@fr;
        rdfs:label       "Formação"@pt;
        rdfs:label       "Формированиe"@ru;
        rdfs:label       "组成"@zh;
        rdfs:comment     "This class comprises events that result in the formation of a formal or informal E74 Group of people, such as a club, society, association, corporation, or nation.\nE66 Formation does not include the arbitrary aggregation of people who do not act as a collective.\nThe formation of an instance of E74 Group does not require that the group is populated with members at the time of formation. In order to express the joining of members at the time of formation, the respective activity should be simultaneously an instance of both E66 Formation and E85 Joining."@en;
        rdfs:subClassOf  <E7_Activity>;
        rdfs:subClassOf  <E63_Beginning_of_Existence> .

<E67_Birth>  rdf:type    rdfs:Class;
        rdfs:label       "Birth"@en;
        rdfs:label       "Geburt"@de;
        rdfs:label       "Γέννηση"@el;
        rdfs:label       "Naissance"@fr;
        rdfs:label       "Nascimento"@pt;
        rdfs:label       "Рождeниe"@ru;
        rdfs:label       "出生"@zh;
        rdfs:comment     "This class comprises the births of human beings. E67 Birth is a biological event focussing on the context of people coming into life. (E63 Beginning of Existence comprises the coming into life of any living being.)\nTwins, triplets, etc. are brought into life by the same instance of E67 Birth. The introduction of the E67 Birth event as a documentation element allows the description of a range of family relationships in a simple model. Suitable extensions may describe more details and the complexity of motherhood since the advent of modern medicine. In this model, the biological father is not seen as a necessary participant in the E67 Birth."@en;
        rdfs:subClassOf  <E63_Beginning_of_Existence> .

<E68_Dissolution>  rdf:type  rdfs:Class;
        rdfs:label       "Dissolution"@en;
        rdfs:label       "Gruppenauflösung"@de;
        rdfs:label       "Διάλυση Ομάδας"@el;
        rdfs:label       "Dissolution"@fr;
        rdfs:label       "Dissolução"@pt;
        rdfs:label       "Роспуск"@ru;
        rdfs:label       "解散"@zh;
        rdfs:comment     "This class comprises the events that result in the formal or informal termination of an instance of E74 Group.\nIf the dissolution was deliberate, the Dissolution event should also be instantiated as an instance of E7 Activity."@en;
        rdfs:subClassOf  <E64_End_of_Existence> .

<E69_Death>  rdf:type    rdfs:Class;
        rdfs:label       "Death"@en;
        rdfs:label       "Tod"@de;
        rdfs:label       "Θάνατος"@el;
        rdfs:label       "Mort"@fr;
        rdfs:label       "Morte"@pt;
        rdfs:label       "Смeрть"@ru;
        rdfs:label       "死亡"@zh;
        rdfs:comment     "This class comprises the deaths of human beings.\nIf a person is killed, their death should be instantiated as E69 Death and as E7 Activity. The death or perishing of other living beings should be documented as instances of E64 End of Existence."@en;
        rdfs:subClassOf  <E64_End_of_Existence> .

<E70_Thing>  rdf:type    rdfs:Class;
        rdfs:label       "Thing"@en;
        rdfs:label       "Sache"@de;
        rdfs:label       "Πράγμα"@el;
        rdfs:label       "Chose"@fr;
        rdfs:label       "Coisa"@pt;
        rdfs:label       "Вeщь"@ru;
        rdfs:label       "事物"@zh;
        rdfs:comment     "This general class comprises discrete, identifiable, instances of E77 Persistent Item that are documented as single units, that either consist of matter or depend on being carried by matter and are characterized by relative stability.\nThey may be intellectual products or physical things. They may, for instance, have a solid physical form, an electronic encoding, or they may be a logical concept or structure."@en;
        rdfs:subClassOf  <E77_Persistent_Item> .

<E71_Human-Made_Thing>
        rdf:type         rdfs:Class;
        rdfs:label       "Human-Made Thing"@en;
        rdfs:label       "Chose élaborée par l’humain"@fr;
        rdfs:label       "Рукотворный Прeдмeт"@ru;
        rdfs:comment     "This class comprises discrete, identifiable human-made items that are documented as single units.\nThese items are either intellectual products or human-made physical things, and are characterized by relative stability. They may, for instance, have a solid physical form, an electronic encoding, or they may be logical concepts or structures."@en;
        rdfs:subClassOf  <E70_Thing> .

<E72_Legal_Object>  rdf:type  rdfs:Class;
        rdfs:label       "Legal Object"@en;
        rdfs:label       "Rechtsobjekt"@de;
        rdfs:label       "Νομικό Αντικείμενο"@el;
        rdfs:label       "Objet juridique"@fr;
        rdfs:label       "Objeto Jurídico"@pt;
        rdfs:label       "Объeкт Права"@ru;
        rdfs:label       "法律对象"@zh;
        rdfs:comment     "This class comprises those material or immaterial items to which instances of E30 Right, such as the right of ownership or use, can be applied.\nThis is generally true for all instances of E18 Physical Thing. In the case of instances of E28 Conceptual Object, however, the identity of an instance of E28 Conceptual Object or the method of its use may be too ambiguous to reliably establish instances of E30 Right, as in the case of taxa and inspirations. Ownership of corporations is currently regarded as out of scope of the CIDOC CRM."@en;
        rdfs:subClassOf  <E70_Thing> .

<E73_Information_Object>
        rdf:type         rdfs:Class;
        rdfs:label       "Information Object"@en;
        rdfs:label       "Informationsgegenstand"@de;
        rdfs:label       "Πληροφοριακό Αντικείμενο"@el;
        rdfs:label       "Objet informationnel"@fr;
        rdfs:label       "Objeto de Informação"@pt;
        rdfs:label       "Информационный Объeкт"@ru;
        rdfs:label       "信息对象"@zh;
        rdfs:comment     "This class comprises identifiable immaterial items, such as poems, jokes, data sets, images, texts, multimedia objects, procedural prescriptions, computer program code, algorithm or mathematical formulae, that have an objectively recognizable structure and are documented as single units. The encoding structure known as a “named graph” also falls under this class, so that each “named graph” is an instance of E73 Information Object.\nAn instance of E73 Information Object does not depend on a specific physical carrier, which can include human memory, and it can exist on one or more carriers simultaneously.\nInstances of E73 Information Object of a linguistic nature should be declared as instances of the E33 Linguistic Object subclass. Instances of E73 Information Object of a documentary nature should be declared as instances of the E31 Document subclass. Conceptual items such as types and classes are not instances of E73 Information Object, nor are ideas without a reproducible expression."@en;
        rdfs:subClassOf  <E89_Propositional_Object>;
        rdfs:subClassOf  <E90_Symbolic_Object> .

<E74_Group>  rdf:type    rdfs:Class;
        rdfs:label       "Group"@en;
        rdfs:label       "Menschliche Gruppe"@de;
        rdfs:label       "Ομάδα"@el;
        rdfs:label       "Groupe"@fr;
        rdfs:label       "Grupo"@pt;
        rdfs:label       "Группа"@ru;
        rdfs:label       "团体"@zh;
        rdfs:comment     "This class comprises any gatherings or organizations of human individuals or groups that act collectively or in a similar way due to any form of unifying relationship. In the wider sense this class also comprises official positions which used to be regarded in certain contexts as one actor, independent of the current holder of the office, such as the president of a country. In such cases, it may happen that the group never had more than one member. A joint pseudonym (i.e. a name that seems indicative of an individual but that is actually used as a persona by two or more people) is a particular case of E74 Group.\nA gathering of people becomes an instance of E74 Group when it exhibits organizational characteristics usually typified by a set of ideas or beliefs held in common, or actions performed together. These might be communication, creating some common artifact, a common purpose such as study, worship, business, sports, etc. Nationality can be modelled as membership in an instance of E74 Group. Married couples and other concepts of family are regarded as particular examples of E74 Group."@en;
        rdfs:subClassOf  <E39_Actor> .

<E77_Persistent_Item>
        rdf:type         rdfs:Class;
        rdfs:label       "Persistent Item"@en;
        rdfs:label       "Seiendes"@de;
        rdfs:label       "Ον"@el;
        rdfs:label       "Entité persistante"@fr;
        rdfs:label       "Entidade Persistente"@pt;
        rdfs:label       "Постоянная Сущность"@ru;
        rdfs:label       "持久项"@zh;
        rdfs:comment     "This class comprises items that have persistent characteristics of structural nature substantially related to their identity and their integrity, sometimes known as “endurants” in philosophy. Persistent Items may be physical entities, such as people, animals or things, conceptual entities such as ideas, concepts, products of the imagination or even names.\nInstances of E77 Persistent Item may be present or be part of interactions in different periods or events. They can repeatedly be recognized at disparate occasions during their existence by characteristics of structural nature. The respective characteristics need not be exactly the same during all the existence of an instance of E77 Persistent Item. Often, they undergo gradual change, still bearing some similarities with that of previous times, or disappear completely and new emerge. For instance, a person, from the time of being born on, will gradually change all its features and acquire new ones, such as a scar. Even the DNA in different body cells will develop defects and mutations. Nevertheless, relevant characteristics used should be sufficiently similar to recognize the instance for some substantial period of time.\nThe more specific criteria that determine the identity of instances of subclasses of E77 Persistent Item may vary considerably and are described or referred to in the respective scope notes. The decision about which exact criteria to use depends on whether the observable behaviour of the respective part of reality such confined conforms to the reasoning the user is interested in. For example, a building can be regarded as no longer existing if it is dismantled and the materials reused in a different configuration. On the other hand, human beings go through radical and profound changes during their life-span, affecting both material composition and form, yet preserve their identity by other criteria, such as being bodily separated from other persons. Similarly, inanimate objects may be subject to exchange of parts and matter. On the opposite, the identity of a (version of a) text of a scientific publication is given by the exact arrangement of its relevant symbols.\nThe main classes of objects that fall outside the scope of the E77 Persistent Item class are temporal objects such as periods, events and acts, and descriptive properties.\nAn instance of E77 Persistent Item does not require actual knowledge of the identifying features of the instance being currently known. There may be cases, where the actual identifying features of an instance of E77 Persistent Item are not decidable at a particular state of knowledge."@en;
        rdfs:subClassOf  <E1_CRM_Entity> .

<E78_Curated_Holding>
        rdf:type         rdfs:Class;
        rdfs:label       "Curated Holding"@en;
        rdfs:label       "Collection"@fr;
        rdfs:label       "Отвeтствeнноe Хранeниe"@ru;
        rdfs:comment     "This class comprises aggregations of instances of E18 Physical Thing that are assembled and maintained (“curated” and “preserved,” in museological terminology) by one or more instances of E39 Actor over time for a specific purpose and audience, and according to a particular collection development plan. Typical instances of curated holdings are museum collections, archives, library holdings and digital libraries. A digital library is regarded as an instance of E18 Physical Thing because it requires keeping physical carriers of the electronic content.\nItems may be added or removed from an E78 Curated Holding in pursuit of this plan. This class should not be confused with the E39 Actor maintaining the E78 Curated Holding who is often referred to using the name of the E78 Curated Holding (e.g. “The Wallace Collection decided…”).\nCollective objects in the general sense, like a tomb full of gifts, a folder with stamps, or a set of chessmen, should be documented as instances of E19 Physical Object, and not as instances of E78 Curated Holding. This is because they form wholes, either because they are physically bound together or because they are kept together for their functionality."@en;
        rdfs:subClassOf  <E24_Physical_Human-Made_Thing> .

<E79_Part_Addition>  rdf:type  rdfs:Class;
        rdfs:label       "Part Addition"@en;
        rdfs:label       "Teilhinzufügung"@de;
        rdfs:label       "Προσθήκη Μερών"@el;
        rdfs:label       "Ajout d'élément"@fr;
        rdfs:label       "Adição de Parte"@pt;
        rdfs:label       "Добавлeниe Части"@ru;
        rdfs:label       "部分增加"@zh;
        rdfs:comment     "This class comprises activities that result in an instance of E18 Physical Thing being increased, enlarged, or augmented by the addition of a part.\nTypical scenarios include the attachment of an accessory, the integration of a component, the addition of an element to an aggregate object, or the accessioning of an object into a curated instance of E78 Curated Holding. Both the E18 Physical Thing being augmented and the E18 Physical Thing that is being added are treated as separate identifiable wholes prior to the instance of E79 Part Addition. Following the addition of parts, the resulting assemblages are treated objectively as single identifiable wholes, made up of constituent or component parts bound together either physically (for example the engine becoming a part of the car), or by sharing a common purpose (such as the 32 chess pieces that make up a chess set). This class of activities forms a basis for reasoning about the history and continuity of identity of objects that are integrated into other objects over time, such as precious gemstones being repeatedly incorporated into different items of jewellery, or cultural artefacts being added to different museum instances of E78 Curated Holding over their lifespan."@en;
        rdfs:subClassOf  <E11_Modification> .

<E80_Part_Removal>  rdf:type  rdfs:Class;
        rdfs:label       "Part Removal"@en;
        rdfs:label       "Teilentfernung"@de;
        rdfs:label       "Αφαίρεση Μερών"@el;
        rdfs:label       "Retrait d'élément"@fr;
        rdfs:label       "Remoção de Parte"@pt;
        rdfs:label       "Удалeниe Части"@ru;
        rdfs:label       "部分去除"@zh;
        rdfs:comment     "This class comprises the activities that result in an instance of E18 Physical Thing being decreased by the removal of a part.\nTypical scenarios include the detachment of an accessory, the removal of a component or part of a composite object, or the deaccessioning of an object from a curated collection, an instance of E78 Curated Holding. If the instance of E80 Part Removal results in the total decomposition of the original object into pieces, such that the whole ceases to exist, the activity should instead be modelled as an instance of E81 Transformation, i.e. a simultaneous destruction and production. In cases where the part removed has no discernible identity prior to its removal but does have an identity subsequent to its removal, the activity should be modelled as both an instance of E80 Part Removal and E12 Production. This class of activities forms a basis for reasoning about the history, and continuity of identity over time, of objects that are removed from other objects, such as precious gemstones being extracted from different items of jewellery, or cultural artifacts being deaccessioned from different museum collections over their lifespan."@en;
        rdfs:subClassOf  <E11_Modification> .

<E81_Transformation>  rdf:type  rdfs:Class;
        rdfs:label       "Transformation"@en;
        rdfs:label       "Umwandlung"@de;
        rdfs:label       "Μετατροπή"@el;
        rdfs:label       "Transformation"@fr;
        rdfs:label       "Transformação"@pt;
        rdfs:label       "Трансформация"@ru;
        rdfs:label       "转变"@zh;
        rdfs:comment     "This class comprises the events that result in the simultaneous destruction of one or more than one E18 Physical Thing and the creation of one or more than one E18 Physical Thing that preserves recognizable substance and structure from the first one(s) but has fundamentally different nature or identity.\nAlthough the old and the new instances of E18 Physical Thing are treated as discrete entities having separate, unique identities, they are causally connected through the E81 Transformation; the destruction of the old E18 Physical Thing(s) directly causes the creation of the new one(s) using or preserving some relevant substance and structure. Instances of E81 Transformation are therefore distinct from re-classifications (documented using E17 Type Assignment) or modifications (documented using E11 Modification) of objects that do not fundamentally change their nature or identity. Characteristic cases are reconstructions and repurposing of historical buildings or ruins, fires leaving buildings in ruins, taxidermy of specimen in natural history.\nEven though such instances of E81 Transformation are often motivated by a change of intended use, substantial material changes should justify the documentation of the result as a new instance of E18 Physical Thing and not just the change of function. The latter may be documented as an extended activity (instance of E7 Activity) of using it."@en;
        rdfs:subClassOf  <E63_Beginning_of_Existence>;
        rdfs:subClassOf  <E64_End_of_Existence> .

<E83_Type_Creation>  rdf:type  rdfs:Class;
        rdfs:label       "Type Creation"@en;
        rdfs:label       "Typuserfindung"@de;
        rdfs:label       "Δημιουργία Τύπου"@el;
        rdfs:label       "Création de type"@fr;
        rdfs:label       "Criação de Tipo"@pt;
        rdfs:label       "Созданиe Типа"@ru;
        rdfs:label       "类型创建"@zh;
        rdfs:comment     "This class comprises activities formally defining new types of items.\nIt is typically a rigorous scholarly or scientific process that ensures a type is exhaustively described and appropriately named. In some cases, particularly in archaeology and the life sciences, E83 Type Creation requires the identification of an exemplary specimen and the publication of the type definition in an appropriate scholarly forum. The activity modelled as an instance of E83 Type Creation is central to research in the life sciences, where a type would be referred to as a “taxon,” the type description as a “protologue,” and the exemplary specimens as “original element” or “holotype”."@en;
        rdfs:subClassOf  <E65_Creation> .

<E85_Joining>  rdf:type  rdfs:Class;
        rdfs:label       "Joining"@en;
        rdfs:label       "Beitritt"@de;
        rdfs:label       "Adhésion"@fr;
        rdfs:label       "Вступлeниe"@ru;
        rdfs:label       "加入"@zh;
        rdfs:comment     "This class comprises the activities that result in an instance of E39 Actor becoming a member of an instance of E74 Group. This class does not imply initiative by either party. It may be the initiative of a third party.\nTypical scenarios include becoming a member of a social organisation, becoming an employee of a company, marriage, the adoption of a child by a family, and the inauguration of somebody into an official position."@en;
        rdfs:subClassOf  <E7_Activity> .

<E86_Leaving>  rdf:type  rdfs:Class;
        rdfs:label       "Leaving"@en;
        rdfs:label       "Austritt"@de;
        rdfs:label       "Départ"@fr;
        rdfs:label       "Выход"@ru;
        rdfs:label       "离开"@zh;
        rdfs:comment     "This class comprises the activities that result in an instance of E39 Actor to be disassociated from an instance of E74 Group. This class does not imply initiative by either party. It may be the initiative of a third party.\nTypical scenarios include the termination of membership in a social organisation, ending the employment at a company, divorce, and the end of tenure of somebody in an official position."@en;
        rdfs:subClassOf  <E7_Activity> .

<E87_Curation_Activity>
        rdf:type         rdfs:Class;
        rdfs:label       "Curation Activity"@en;
        rdfs:label       "Kuratorische Tätigkeit"@de;
        rdfs:label       "Activité curatoriale"@fr;
        rdfs:label       "Кураторство"@ru;
        rdfs:label       "管理"@zh;
        rdfs:comment     "This class comprises the activities that contribute to the management and the preservation and evolution of instances of E78 Curated Holding, following an implicit or explicit curation plan.\nIt specializes the notion of activity into the curation of a collection and allows the history of curation to be recorded.\nItems are accumulated and organized following criteria such as subject, chronological period, material type, style of art, etc., and can be added or removed from an instance of E78 Curated Holding for a specific purpose and/or audience. The initial aggregation of items to form a collection is regarded as an instance of E12 Production Event, while the activities of evolving, preserving, and promoting a collection are regarded as instances of E87 Curation Activity."@en;
        rdfs:subClassOf  <E7_Activity> .

<E89_Propositional_Object>
        rdf:type         rdfs:Class;
        rdfs:label       "Propositional Object"@en;
        rdfs:label       "Aussagenobjekt"@de;
        rdfs:label       "Objet propositionnel"@fr;
        rdfs:label       "Пропозициональный Объeкт"@ru;
        rdfs:label       "命题对象"@zh;
        rdfs:comment     "This class comprises immaterial items, including but not limited to stories, plots, procedural prescriptions, algorithms, laws of physics or images that are, or represent in some sense, sets of propositions about real or imaginary things and that are documented as single units or serve as topic of discourse.\nThis class also comprises items that are “about” something in the sense of a subject. In the wider sense, this class includes expressions of psychological value such as non-figural art and musical themes. However, conceptual items such as types and classes are not instances of E89 Propositional Object. This should not be confused with the definition of a type, which is indeed an instance of E89 Propositional Object."@en;
        rdfs:subClassOf  <E28_Conceptual_Object> .

<E90_Symbolic_Object>
        rdf:type         rdfs:Class;
        rdfs:label       "Symbolic Object"@en;
        rdfs:label       "Symbolisches Objekt"@de;
        rdfs:label       "Objet symbolique"@fr;
        rdfs:label       "Символичeский Объeкт"@ru;
        rdfs:label       "符号对象"@zh;
        rdfs:comment     "This class comprises identifiable symbols and any aggregation of symbols, such as characters, identifiers, traffic signs, emblems, texts, data sets, images, musical scores, multimedia objects, computer program code, or mathematical formulae that have an objectively recognizable structure and that are documented as single units.\nIt includes sets of signs of any nature, which may serve to designate something, or to communicate some propositional content. An instance of E90 Symbolic Object may or may not have a specific meaning, for example an arbitrary character string.\nIn some cases, the content of an instance of E90 Symbolic Object may completely be represented by a serialized digital content model, such as a sequence of ASCII-encoded characters, an XML or HTML document, or a TIFF image. The property P3 has note and its subproperty P190 has symbolic content allow for the description of this content model. In order to disambiguate which symbolic level is the carrier of the meaning, the property P3.1 has type can be used to specify the encoding (e.g. “bit”, “Latin character”, RGB pixel)."@en;
        rdfs:subClassOf  <E28_Conceptual_Object>;
        rdfs:subClassOf  <E72_Legal_Object> .

<E92_Spacetime_Volume>
        rdf:type         rdfs:Class;
        rdfs:label       "Spacetime Volume"@en;
        rdfs:label       "Volume spatio-temporel"@fr;
        rdfs:label       "Область Пространства-Врeмeни"@ru;
        rdfs:comment     "This class comprises 4-dimensional point sets (volumes) in physical spacetime (in contrast to mathematical models of it) regardless of their true geometric forms. They may derive their identity from being the extent of a material phenomenon or from being the interpretation of an expression defining an extent in spacetime. Intersections of instances of E92 Spacetime Volume, E53 Place, and E52 Time-Span are also regarded as instances of E92 Spacetime Volume. An instance of E92 Spacetime Volume is either contiguous or composed of a finite number of contiguous subsets. Its boundaries may be fuzzy due to the properties of the phenomena it derives from or due to the limited precision up to which defining expression can be identified with a real extent in spacetime. The duration of existence of an instance of E92 Spacetime Volume is its projection on time."@en;
        rdfs:subClassOf  <E1_CRM_Entity> .

<E93_Presence>  rdf:type  rdfs:Class;
        rdfs:label       "Presence"@en;
        rdfs:label       "Présence"@fr;
        rdfs:label       "Присутствиe"@ru;
        rdfs:comment     "This class comprises instances of E92 Spacetime Volume, whose temporal extent has been chosen in order to determine the spatial extent of a phenomenon over the chosen time-span. Respective phenomena may, for instance, be historical events or periods, but can also be the diachronic extent and existence of physical things. In other words, instances of this class fix a slice of another instance of E92 Spacetime Volume in time.\nThe temporal extent of an instance of E93 Presence typically is predetermined by the researcher so as to focus the investigation particularly on finding the spatial extent of the phenomenon by testing for its characteristic features. There are at least two basic directions such investigations might take. The investigation may wish to determine where something was during some time or it may wish to reconstruct the total passage of a phenomenon’s spacetime volume through an examination of discrete presences. Observation and measurement of features indicating the presence or absence of a phenomenon in some space allows for the progressive approximation of spatial extents through argumentation typically based on inclusion, exclusion and various overlaps."@en;
        rdfs:subClassOf  <E92_Spacetime_Volume> .

<E96_Purchase>  rdf:type  rdfs:Class;
        rdfs:label       "Purchase"@en;
        rdfs:label       "Achat"@fr;
        rdfs:label       "Покупка"@ru;
        rdfs:comment     "This class comprises transfers of legal ownership from one or more instances of E39 Actor to one or more different instances of E39 Actor, where the transferring party is completely compensated by the payment of a monetary amount. In more detail, a purchase agreement establishes a fixed monetary obligation at its initialization on the receiving party, to the giving party. An instance of E96 Purchase begins with the contract or equivalent agreement and ends with the fulfilment of all contractual obligations. In the case that the activity is abandoned before both parties have fulfilled these obligations, the activity is not regarded as an instance of E96 Purchase.\nThis class is a very specific case of the much more complex social business practices of exchange of goods and the creation and satisfaction of related social obligations. Purchase activities which define individual sales prices per object can be modelled by instantiating E96 Purchase for each object individually and as part of an overall instance of E96 Purchase transaction."@en;
        rdfs:subClassOf  <E8_Acquisition> .

<E97_Monetary_Amount>
        rdf:type         rdfs:Class;
        rdfs:label       "Monetary Amount"@en;
        rdfs:label       "Valeur monétaire"@fr;
        rdfs:label       "Дeнeжный Эквивалeнт"@ru;
        rdfs:comment     "This class comprises quantities of monetary possessions or obligations in terms of their nominal value with respect to a particular currency. These quantities may be abstract accounting units, the nominal value of a heap of coins or bank notes at the time of validity of the respective currency, the nominal value of a bill of exchange or other documents expressing monetary claims or obligations. It specifically excludes amounts expressed in terms of weights of valuable items, like gold and diamonds, and quantities of other non-currency items, like goats or stocks and bonds."@en;
        rdfs:subClassOf  <E54_Dimension> .

<E98_Currency>  rdf:type  rdfs:Class;
        rdfs:label       "Currency"@en;
        rdfs:label       "Unité monétaire"@fr;
        rdfs:label       "Валюта"@ru;
        rdfs:comment     "This class comprises the units in which a monetary system, supported by an administrative authority or other community, quantifies and arithmetically compares all monetary amounts declared in the unit. The unit of a monetary system must describe a nominal value which is kept constant by its administrative authority and an associated banking system if it exists, and not by market value. For instance, one may pay with grams of gold, but the respective monetary amount would have been agreed as the gold price in US dollars on the day of the payment. Under this definition, British Pounds, U.S. Dollars, and European Euros are examples of currency, but “grams of gold” is not. One monetary system has one and only one currency. Instances of this class must not be confused with coin denominations, such as “Dime” or “Sestertius”. Non-monetary exchange of value in terms of quantities of a particular type of goods, such as cows, do not constitute a currency."@en;
        rdfs:subClassOf  <E58_Measurement_Unit> .

<E99_Product_Type>  rdf:type  rdfs:Class;
        rdfs:label       "Product Type"@en;
        rdfs:label       "Modèle de produit"@fr;
        rdfs:label       "Тип Продукта"@ru;
        rdfs:comment     "This class comprises types that stand as the models for instances of E22 Human-Made Object that are produced as the result of production activities using plans exact enough to result in one or more series of uniform, functionally and aesthetically identical and interchangeable items. The product type is the intended ideal form of the manufacture process. It is typical of instances of E22 Human-Made Object that conform to an instance of E99 Product Type that its component parts are interchangeable with component parts of other instances of E22 Human-Made Object made after the model of the same instance of E99 Product Type. Frequently, the uniform production according to a given instance of E99 Product Type is achieved by creating individual tools, such as moulds or print plates that are themselves carriers of the design of the product type. Modern tools may use the flexibility of electronically controlled devices to achieve such uniformity. The product type itself, i.e. the potentially unlimited series of aesthetically equivalent items, may be the target of artistic design, rather than the individual object. In extreme cases, only one instance of a product type may have been produced, such as in a “print on demand” process which was only triggered once. However, this should not be confused with industrial prototypes, such as car prototypes, which are produced prior to the production line being set up, or test the production line itself."@en;
        rdfs:subClassOf  <E55_Type> .

<P1_is_identified_by>
        rdf:type       rdf:Property;
        rdfs:label     "is identified by"@en;
        rdfs:label     "wird bezeichnet als"@de;
        rdfs:label     "αναγνωρίζεται ως"@el;
        rdfs:label     "est identifié par"@fr;
        rdfs:label     "é identificado por"@pt;
        rdfs:label     "идeнтифицируeтся"@ru;
        rdfs:label     "被标识为"@zh;
        rdfs:comment   "This property describes the naming or identification of any real-world item by a name or any other identifier.\nThis property is intended for identifiers in general use, which form part of the world the model intends to describe, and not merely for internal database identifiers which are specific to a technical system, unless these latter also have a more general use outside the technical context. This property includes in particular identification by mathematical expressions such as coordinate systems used for the identification of instances of E53 Place. The property does not reveal anything about when, where and by whom this identifier was used. A more detailed representation can be made using the fully developed (i.e. indirect) path through E15 Identifier Assignment.\nThis property is a shortcut for the path from E1 CRM Entity through P140i was attributed by, E15 Identifier Assignment, P37 assigned to E42 Identifier.\nIt is also a shortcut for the path from E1 CRM Entity through P1 is identified by, E41 Appellation, P139 has alternative form to E41 Appellation."@en;
        rdfs:domain    <E1_CRM_Entity>;
        rdfs:range     <E41_Appellation>;
        owl:inverseOf  <P1i_identifies> .

<P1i_identifies>  rdf:type  rdf:Property;
        rdfs:label     "identifies"@en;
        rdfs:label     "bezeichnet"@de;
        rdfs:label     "είναι αναγνωριστικό"@el;
        rdfs:label     "identifie"@fr;
        rdfs:label     "identifica"@pt;
        rdfs:label     "идeнтифицируeт"@ru;
        rdfs:label     "标识"@zh;
        rdfs:domain    <E41_Appellation>;
        rdfs:range     <E1_CRM_Entity>;
        owl:inverseOf  <P1_is_identified_by> .

<P2_has_type>  rdf:type  rdf:Property;
        rdfs:label     "has type"@en;
        rdfs:label     "hat den Typus"@de;
        rdfs:label     "έχει τύπο"@el;
        rdfs:label     "a pour type"@fr;
        rdfs:label     "é do tipo"@pt;
        rdfs:label     "имeeт тип"@ru;
        rdfs:label     "有类型"@zh;
        rdfs:comment   "This property allows sub-typing of CIDOC CRM entities –a form of specialisation – through the use of a terminological hierarchy, or thesaurus.\nThe CIDOC CRM is intended to focus on the high-level entities and relationships needed to describe data structures. Consequently, it does not specialise entities any further than is required for this immediate purpose. However, entities in the isA hierarchy of the CIDOC CRM may by specialised into any number of sub-entities, which can be defined in the E55 Type hierarchy. E41 Appellation, for example, may be specialised into “e-mail address”, “telephone number”, “post office box”, “URL”, etc., none of which figures explicitly in the CIDOC CRM class hierarchy. A comprehensive explanation about refining CIDOC CRM concepts by E55 Type is given in the section “About Types” in the section on “Specific Modelling Constructs” of this document.\nThis property is a shortcut for the path from E1 CRM Entity through P41i was classified by, E17 Type Assignment, P42 assigned to E55 Type."@en;
        rdfs:domain    <E1_CRM_Entity>;
        rdfs:range     <E55_Type>;
        owl:inverseOf  <P2i_is_type_of> .

<P2i_is_type_of>  rdf:type  rdf:Property;
        rdfs:label     "is type of"@en;
        rdfs:label     "ist Typus von"@de;
        rdfs:label     "είναι ο τύπος του/της"@el;
        rdfs:label     "est le type de"@fr;
        rdfs:label     "é o tipo de"@pt;
        rdfs:label     "являeтся типом"@ru;
        rdfs:label     "是类型"@zh;
        rdfs:domain    <E55_Type>;
        rdfs:range     <E1_CRM_Entity>;
        owl:inverseOf  <P2_has_type> .

<P3_has_note>  rdf:type  rdf:Property;
        rdfs:label    "has note"@en;
        rdfs:label    "hat Anmerkung"@de;
        rdfs:label    "έχει επεξήγηση"@el;
        rdfs:label    "a pour note"@fr;
        rdfs:label    "tem nota"@pt;
        rdfs:label    "имeeт примeчаниe"@ru;
        rdfs:label    "有注释"@zh;
        rdfs:comment  "This property is a container for all informal descriptions about an object that have not been expressed in terms of CIDOC CRM constructs.\nIn particular, it captures the characterisation of the item itself, its internal structures, appearance, etc.\nLike property P2 has type (is type of), this property is a consequence of the restricted focus of the CIDOC CRM. The aim is not to capture, in a structured form, everything that can be said about an item; indeed, the CIDOC CRM formalism is not regarded as sufficient to express everything that can be said. Good practice requires use of distinct note fields for different aspects of a characterisation. The P3.1 has type property of P3 has note allows differentiation of specific notes, e.g. “construction”, “decoration”, etc.\nAn item may have many notes, but a note is attached to a specific item."@en;
        rdfs:domain   <E1_CRM_Entity>;
        rdfs:range    rdfs:Literal .

<P4_has_time-span>  rdf:type  rdf:Property;
        rdfs:label     "has time-span"@en;
        rdfs:label     "hat Zeitspanne"@de;
        rdfs:label     "βρισκόταν σε εξέλιξη"@el;
        rdfs:label     "a pour intervalle temporel"@fr;
        rdfs:label     "tem período de tempo"@pt;
        rdfs:label     "имeeт врeмeнной интeрвал"@ru;
        rdfs:label     "发生时段是"@zh;
        rdfs:comment   "This property associates an instance of E2 Temporal Entity with the instance of E52 Time-Span during which it was on-going. The associated instance of E52 Time-Span is understood as the real time-span during which the phenomena making up the temporal entity instance were active. More than one instance of E2 Temporal Entity may share a common instance of E52 Time-Span only if they come into being and end being due to identical declarations or events."@en;
        rdfs:domain    <E2_Temporal_Entity>;
        rdfs:range     <E52_Time-Span>;
        owl:inverseOf  <P4i_is_time-span_of> .

<P4i_is_time-span_of>
        rdf:type       rdf:Property;
        rdfs:label     "is time-span of"@en;
        rdfs:label     "ist Zeitspanne von"@de;
        rdfs:label     "είναι χρονικό διάστημα του/της"@el;
        rdfs:label     "est l’intervalle temporel de"@fr;
        rdfs:label     "é o período de tempo de"@pt;
        rdfs:label     "являeтся врeмeнным интeрвалом"@ru;
        rdfs:label     "是时段"@zh;
        rdfs:domain    <E52_Time-Span>;
        rdfs:range     <E2_Temporal_Entity>;
        owl:inverseOf  <P4_has_time-span> .

<P5_consists_of>  rdf:type  rdf:Property;
        rdfs:label     "consists of"@en;
        rdfs:label     "besteht aus"@de;
        rdfs:label     "αποτελείται από"@el;
        rdfs:label     "comprend"@fr;
        rdfs:label     "consiste de"@pt;
        rdfs:label     "состоит из"@ru;
        rdfs:label     "包括"@zh;
        rdfs:comment   "This property describes the decomposition of an instance of E3 Condition State into discrete, subsidiary states.\nIt is assumed that the sub-states into which the condition state is analysed form a logical whole, although the entire story may not be completely known, and that the sub-states are in fact constitutive of the general condition state. For example, a general condition state of “in ruins” may be decomposed into the individual stages of decay.\nThis property is transitive and asymmetric."@en;
        rdfs:domain    <E3_Condition_State>;
        rdfs:range     <E3_Condition_State>;
        owl:inverseOf  <P5i_forms_part_of> .

<P5i_forms_part_of>  rdf:type  rdf:Property;
        rdfs:label     "forms part of"@en;
        rdfs:label     "bildet Teil von"@de;
        rdfs:label     "αποτελεί μέρος του/της"@el;
        rdfs:label     "fait partie de"@fr;
        rdfs:label     "faz parte de"@pt;
        rdfs:label     "являeтся частью"@ru;
        rdfs:label     "组成部分"@zh;
        rdfs:domain    <E3_Condition_State>;
        rdfs:range     <E3_Condition_State>;
        owl:inverseOf  <P5_consists_of> .

<P7_took_place_at>  rdf:type  rdf:Property;
        rdfs:label     "took place at"@en;
        rdfs:label     "fand statt in"@de;
        rdfs:label     "έλαβε χώρα σε"@el;
        rdfs:label     "a eu lieu dans"@fr;
        rdfs:label     "ocorreu em"@pt;
        rdfs:label     "совeршался на"@ru;
        rdfs:label     "发生地在"@zh;
        rdfs:comment   "This property describes the spatial location of an instance of E4 Period.\nThe related instance of E53 Place should be seen as a wider approximation of the geometric area within which the phenomena that characterise the period in question occurred, see below. P7 took place at (witnessed) does not convey any meaning other than spatial positioning (frequently on the surface of the earth). For example, the period “Révolution française” can be said to have taken place in “France in 1789”; the “Victorian” period may be said to have taken place in “Britain from 1837-1901” and its colonies, as well as other parts of Europe and North America. An instance of E4 Period can take place at multiple non-contiguous, non-overlapping locations.\nAny place where something happened includes the spatial projection of the happening given in the same geometric reference system. For instance, HMS Victory, as place of Lord Nelson's dying, includes the location of his body relative to the hull of HMS Victory at his time of death as the most precise location of his death. By the definition of P161 has spatial projection, an instance of E4 Period takes place on all its spatial projections to respective reference systems, that is, instances of E53 Place. Therefore, this property implies the more fully developed path from E4 Period through P161 has spatial projection, E53 Place, P89 falls within to E53 Place, where both places are defined in the same geometric reference system. The relation between an instance of E53 Place and its reference system can conveniently be documented via the property P157 is at rest relative to (provides reference space for).\nSomething that has happened at a given place can also be considered to have happened at a smaller place within it: for example, it is reasonable to say Caesar’s murder took place in Rome, but also on the Forum Romanum, and more precisely in the Curia. It is characteristic for different historical sources to use varying precision in such statements, without being in contradiction with each other. This may be due to lack of knowledge or to the relevance of the precision for the purpose of the statement. In information integration, the more precise statement improves the overall knowledge."@en;
        rdfs:domain    <E4_Period>;
        rdfs:range     <E53_Place>;
        owl:inverseOf  <P7i_witnessed> .

<P7i_witnessed>  rdf:type  rdf:Property;
        rdfs:label     "witnessed"@en;
        rdfs:label     "bezeugte"@de;
        rdfs:label     "υπήρξε τόπος του"@el;
        rdfs:label     "a été témoin de"@fr;
        rdfs:label     "testemunhou"@pt;
        rdfs:label     "было мeстом совeршeния"@ru;
        rdfs:label     "发生过"@zh;
        rdfs:domain    <E53_Place>;
        rdfs:range     <E4_Period>;
        owl:inverseOf  <P7_took_place_at> .

<P8_took_place_on_or_within>
        rdf:type       rdf:Property;
        rdfs:label     "took place on or within"@en;
        rdfs:label     "fand statt auf oder innerhalb von"@de;
        rdfs:label     "έλαβε χώρα σε ή εντός"@el;
        rdfs:label     "a eu lieu à"@fr;
        rdfs:label     "ocorreu em ou dentro"@pt;
        rdfs:label     "имeл мeсто на или в"@ru;
        rdfs:label     "发生的所在对象是"@zh;
        rdfs:comment   "This property describes the location of an instance of E4 Period with respect to an instance of E18 Physical Thing.\nThis property is a shortcut of the more fully developed path from E4 Period through P7 took place at, E53 Place, P156i is occupied by to E18 Physical Thing.\nIt describes a period that can be located with respect to the space defined by an E19 Physical Object such as a ship or a building. The precise geographical location of the object during the period in question may be unknown or unimportant.\nFor example, the French and German armistice of 22-nd June 1940 was signed in the same railway carriage as the armistice of 11-th November 1918."@en;
        rdfs:domain    <E4_Period>;
        rdfs:range     <E18_Physical_Thing>;
        owl:inverseOf  <P8i_witnessed> .

<P8i_witnessed>  rdf:type  rdf:Property;
        rdfs:label     "witnessed"@en;
        rdfs:label     "bezeugte"@de;
        rdfs:label     "υπήρξε τόπος του"@el;
        rdfs:label     "a été témoin de"@fr;
        rdfs:label     "testemunhou"@pt;
        rdfs:label     "являлся мeстом для"@ru;
        rdfs:label     "发生过"@zh;
        rdfs:domain    <E18_Physical_Thing>;
        rdfs:range     <E4_Period>;
        owl:inverseOf  <P8_took_place_on_or_within> .

<P9_consists_of>  rdf:type  rdf:Property;
        rdfs:label          "consists of"@en;
        rdfs:label          "setzt sich zusammen aus"@de;
        rdfs:label          "αποτελείται από"@el;
        rdfs:label          "comprend"@fr;
        rdfs:label          "consiste de"@pt;
        rdfs:label          "состоит из"@ru;
        rdfs:label          "包括"@zh;
        rdfs:comment        "This property associates an instance of E4 Period with another instance of E4 Period that is defined by a subset of the phenomena that define the former. Therefore, the spacetime volume of the latter must fall within the spacetime volume of the former.\nThis property is transitive and asymmetric."@en;
        rdfs:domain         <E4_Period>;
        rdfs:range          <E4_Period>;
        rdfs:subPropertyOf  <P10i_contains>;
        owl:inverseOf       <P9i_forms_part_of> .

<P9i_forms_part_of>  rdf:type  rdf:Property;
        rdfs:label          "forms part of"@en;
        rdfs:label          "bildet Teil von"@de;
        rdfs:label          "αποτελεί μέρος του/της"@el;
        rdfs:label          "fait partie de"@fr;
        rdfs:label          "faz parte de"@pt;
        rdfs:label          "являeтся частью"@ru;
        rdfs:label          "组成部分"@zh;
        rdfs:domain         <E4_Period>;
        rdfs:range          <E4_Period>;
        rdfs:subPropertyOf  <P10_falls_within>;
        owl:inverseOf       <P9_consists_of> .

<P10_falls_within>  rdf:type  rdf:Property;
        rdfs:label          "falls within"@en;
        rdfs:label          "fällt in"@de;
        rdfs:label          "εμπίπτει"@el;
        rdfs:label          "s’insère dans"@fr;
        rdfs:label          "está contido em"@pt;
        rdfs:label          "находится в прeдeлах"@ru;
        rdfs:label          "属于"@zh;
        rdfs:comment        "This property associates an instance of E92 Spacetime Volume with another instance of E92 Spacetime Volume that falls within the latter. In other words, all points in the former are also points in the latter.\nThis property is transitive and reflexive."@en;
        rdfs:domain         <E92_Spacetime_Volume>;
        rdfs:range          <E92_Spacetime_Volume>;
        rdfs:subPropertyOf  <P132_spatiotemporally_overlaps_with>;
        owl:inverseOf       <P10i_contains> .

<P10i_contains>  rdf:type   rdf:Property;
        rdfs:label          "contains"@en;
        rdfs:label          "enthält"@de;
        rdfs:label          "περιλαμβάνει"@el;
        rdfs:label          "contient"@fr;
        rdfs:label          "contém"@pt;
        rdfs:label          "содeржит"@ru;
        rdfs:label          "包含"@zh;
        rdfs:domain         <E92_Spacetime_Volume>;
        rdfs:range          <E92_Spacetime_Volume>;
        rdfs:subPropertyOf  <P132_spatiotemporally_overlaps_with>;
        owl:inverseOf       <P10_falls_within> .

<P11_had_participant>
        rdf:type            rdf:Property;
        rdfs:label          "had participant"@en;
        rdfs:label          "hatte Teilnehmer"@de;
        rdfs:label          "είχε συμμέτοχο"@el;
        rdfs:label          "a eu pour actant participant"@fr;
        rdfs:label          "tem participante"@pt;
        rdfs:label          "имeл участника"@ru;
        rdfs:label          "有参与者"@zh;
        rdfs:comment        "This property describes the active or passive participation of instances of E39 Actors in an instance of E5 Event.\nIt documents known events in which an instance of E39 Actor has participated during the course of that actor’s life or history. The instances of E53 Place and E52 Time-Span where and when these events happened provide constraints about the presence of the related instances of E39 Actor in the past. Collective actors, i.e. instances of E74 Group, may physically participate in events via their representing instances of E21 Persons only. The participation of multiple actors in an event is most likely an indication of their acquaintance and interaction.\nThe property implies that the actor was involved in the event but does not imply any causal relationship. For instance, someone having been portrayed can be said to have participated in the creation of the portrait."@en;
        rdfs:domain         <E5_Event>;
        rdfs:range          <E39_Actor>;
        rdfs:subPropertyOf  <P12_occurred_in_the_presence_of>;
        owl:inverseOf       <P11i_participated_in> .

<P11i_participated_in>
        rdf:type            rdf:Property;
        rdfs:label          "participated in"@en;
        rdfs:label          "nahm Teil an"@de;
        rdfs:label          "συμμετείχε σε"@el;
        rdfs:label          "a participé à"@fr;
        rdfs:label          "participa em"@pt;
        rdfs:label          "участвовал в"@ru;
        rdfs:label          "参与"@zh;
        rdfs:domain         <E39_Actor>;
        rdfs:range          <E5_Event>;
        rdfs:subPropertyOf  <P12i_was_present_at>;
        owl:inverseOf       <P11_had_participant> .

<P12_occurred_in_the_presence_of>
        rdf:type       rdf:Property;
        rdfs:label     "occurred in the presence of"@en;
        rdfs:label     "fand statt im Beisein von"@de;
        rdfs:label     "συνέβη παρουσία του/της"@el;
        rdfs:label     "a eu lieu en présence de"@fr;
        rdfs:label     "ocorreu na presença de"@pt;
        rdfs:label     "появился в присутствии"@ru;
        rdfs:label     "已出现"@zh;
        rdfs:comment   "This property describes the active or passive presence of an E77 Persistent Item in an instance of E5 Event without implying any specific role.\nIt documents known events in which an instance of E77 Persistent Item was present during the course of its life or history. For example, an object may be the desk, now in a museum, on which a treaty was signed. The instance of E53 Place and the instance of E52 Time-Span where and when these events happened provide constraints about the presence of the related instance E77 Persistent Item in the past. Instances of E90 Symbolic Object, in particular information objects, are physically present in events via at least one of the instances of E18 Physical Thing carrying them. Note, that the human mind can be such a carrier. A precondition for a transfer of information to a person or another new physical carrier is the presence of the respective information object and this person or physical thing in one event."@en;
        rdfs:domain    <E5_Event>;
        rdfs:range     <E77_Persistent_Item>;
        owl:inverseOf  <P12i_was_present_at> .

<P12i_was_present_at>
        rdf:type       rdf:Property;
        rdfs:label     "was present at"@en;
        rdfs:label     "war anwesend bei"@de;
        rdfs:label     "ήταν παρών/παρούσα/παρόν σε"@el;
        rdfs:label     "a été présent à"@fr;
        rdfs:label     "estava presente no"@pt;
        rdfs:label     "присутствовал при"@ru;
        rdfs:label     "出现在"@zh;
        rdfs:domain    <E77_Persistent_Item>;
        rdfs:range     <E5_Event>;
        owl:inverseOf  <P12_occurred_in_the_presence_of> .

<P13_destroyed>  rdf:type   rdf:Property;
        rdfs:label          "destroyed"@en;
        rdfs:label          "zerstörte"@de;
        rdfs:label          "κατέστρεψε"@el;
        rdfs:label          "a détruit"@fr;
        rdfs:label          "destruiu"@pt;
        rdfs:label          "уничтожил"@ru;
        rdfs:label          "破坏了"@zh;
        rdfs:comment        "This property links an instance of E6 Destruction to an instance of E18 Physical Thing that has been destroyed by it.\nDestruction implies the end of an item’s life as a subject of cultural documentation – the physical matter of which the item was composed may in fact continue to exist. An instance of E6 Destruction may be contiguous with an instance of E12 Production that brings into existence a derived object composed partly of matter from the destroyed object."@en;
        rdfs:domain         <E6_Destruction>;
        rdfs:range          <E18_Physical_Thing>;
        rdfs:subPropertyOf  <P93_took_out_of_existence>;
        owl:inverseOf       <P13i_was_destroyed_by> .

<P13i_was_destroyed_by>
        rdf:type            rdf:Property;
        rdfs:label          "was destroyed by"@en;
        rdfs:label          "wurde zerstört durch"@de;
        rdfs:label          "καταστράφηκε από"@el;
        rdfs:label          "a été détruit par"@fr;
        rdfs:label          "foi destruído por"@pt;
        rdfs:label          "был уничтожeн"@ru;
        rdfs:label          "被破坏"@zh;
        rdfs:domain         <E18_Physical_Thing>;
        rdfs:range          <E6_Destruction>;
        rdfs:subPropertyOf  <P93i_was_taken_out_of_existence_by>;
        owl:inverseOf       <P13_destroyed> .

<P14_carried_out_by>  rdf:type  rdf:Property;
        rdfs:label          "carried out by"@en;
        rdfs:label          "wurde ausgeführt von"@de;
        rdfs:label          "πραγματοποιήθηκε από"@el;
        rdfs:label          "a été effectué par"@fr;
        rdfs:label          "realizada por"@pt;
        rdfs:label          "выполнялся"@ru;
        rdfs:label          "执行者是"@zh;
        rdfs:comment        "This property describes the active participation of an instance of E39 Actor in an instance of E7 Activity.\nIt implies causal or legal responsibility. The P14.1 in the role of property of the property specifies the nature of an Actor’s participation."@en;
        rdfs:domain         <E7_Activity>;
        rdfs:range          <E39_Actor>;
        rdfs:subPropertyOf  <P11_had_participant>;
        owl:inverseOf       <P14i_performed> .

<P14i_performed>  rdf:type  rdf:Property;
        rdfs:label          "performed"@en;
        rdfs:label          "führte aus"@de;
        rdfs:label          "πραγματοποίησε"@el;
        rdfs:label          "a effectué"@fr;
        rdfs:label          "executou"@pt;
        rdfs:label          "выполнял"@ru;
        rdfs:label          "执行"@zh;
        rdfs:domain         <E39_Actor>;
        rdfs:range          <E7_Activity>;
        rdfs:subPropertyOf  <P11i_participated_in>;
        owl:inverseOf       <P14_carried_out_by> .

<P15_was_influenced_by>
        rdf:type       rdf:Property;
        rdfs:label     "was influenced by"@en;
        rdfs:label     "wurde beeinflußt durch"@de;
        rdfs:label     "επηρεάστηκε από"@el;
        rdfs:label     "a été influencé par"@fr;
        rdfs:label     "foi influenciado por"@pt;
        rdfs:label     "находился под влияниeм"@ru;
        rdfs:label     "被影响"@zh;
        rdfs:comment   "This is a high-level property, which captures the relationship between an instance of E7 Activity and anything, that is, an instance of E1 CRM Entity, that may have had some bearing upon it.\nThe property has more specific subproperties."@en;
        rdfs:domain    <E7_Activity>;
        rdfs:range     <E1_CRM_Entity>;
        owl:inverseOf  <P15i_influenced> .

<P15i_influenced>  rdf:type  rdf:Property;
        rdfs:label     "influenced"@en;
        rdfs:label     "beeinflußte"@de;
        rdfs:label     "επηρέασε"@el;
        rdfs:label     "a influencé"@fr;
        rdfs:label     "influenciou"@pt;
        rdfs:label     "повлиял"@ru;
        rdfs:label     "影响"@zh;
        rdfs:domain    <E1_CRM_Entity>;
        rdfs:range     <E7_Activity>;
        owl:inverseOf  <P15_was_influenced_by> .

<P16_used_specific_object>
        rdf:type            rdf:Property;
        rdfs:label          "used specific object"@en;
        rdfs:label          "benutzte das bestimmte Objekt"@de;
        rdfs:label          "χρησιμοποίησε αντικείμενο"@el;
        rdfs:label          "a mobilisé l’objet spécifique"@fr;
        rdfs:label          "usou objeto específico"@pt;
        rdfs:label          "пользовался"@ru;
        rdfs:label          "使用特定对象"@zh;
        rdfs:comment        "This property describes the use of material or immaterial things in a way essential to the performance or the outcome of an instance of E7 Activity.\nThis property typically applies to tools, instruments, moulds, raw materials and items embedded in a product. It implies that the presence of the object in question was a necessary condition for the action. For example, the activity of writing this text required the use of a computer. An immaterial thing can be used if at least one of its carriers is present. For example, the software tools on a computer.\nAnother example is the use of a particular name by a particular group of people over some span to identify a thing, such as a settlement. In this case, the physical carriers of this name are at least the people understanding its use."@en;
        rdfs:domain         <E7_Activity>;
        rdfs:range          <E70_Thing>;
        rdfs:subPropertyOf  <P12_occurred_in_the_presence_of>;
        rdfs:subPropertyOf  <P15_was_influenced_by>;
        owl:inverseOf       <P16i_was_used_for> .

<P16i_was_used_for>  rdf:type  rdf:Property;
        rdfs:label          "was used for"@en;
        rdfs:label          "wurde benutzt für"@de;
        rdfs:label          "χρησιμοποιήθηκε για"@el;
        rdfs:label          "a été mobilisé pour"@fr;
        rdfs:label          "foi usado por"@pt;
        rdfs:label          "был использован"@ru;
        rdfs:label          "用于"@zh;
        rdfs:domain         <E70_Thing>;
        rdfs:range          <E7_Activity>;
        rdfs:subPropertyOf  <P12i_was_present_at>;
        rdfs:subPropertyOf  <P15i_influenced>;
        owl:inverseOf       <P16_used_specific_object> .

<P17_was_motivated_by>
        rdf:type            rdf:Property;
        rdfs:label          "was motivated by"@en;
        rdfs:label          "wurde angeregt durch"@de;
        rdfs:label          "είχε ως αφορμή"@el;
        rdfs:label          "a été motivé par"@fr;
        rdfs:label          "foi motivado por"@pt;
        rdfs:label          "послужил мотивом для"@ru;
        rdfs:label          "被促动"@zh;
        rdfs:comment        "This property describes an item or items that are regarded as a reason for carrying out the instance of E7 Activity.\nFor example, the discovery of a large hoard of treasure may call for a celebration, an order from headquarters can start a military manoeuvre."@en;
        rdfs:domain         <E7_Activity>;
        rdfs:range          <E1_CRM_Entity>;
        rdfs:subPropertyOf  <P15_was_influenced_by>;
        owl:inverseOf       <P17i_motivated> .

<P17i_motivated>  rdf:type  rdf:Property;
        rdfs:label          "motivated"@en;
        rdfs:label          "regte an"@de;
        rdfs:label          "ήταν αφορμή"@el;
        rdfs:label          "a motivé"@fr;
        rdfs:label          "motivou"@pt;
        rdfs:label          "мотивировал"@ru;
        rdfs:label          "促动"@zh;
        rdfs:domain         <E1_CRM_Entity>;
        rdfs:range          <E7_Activity>;
        rdfs:subPropertyOf  <P15i_influenced>;
        owl:inverseOf       <P17_was_motivated_by> .

<P19_was_intended_use_of>
        rdf:type       rdf:Property;
        rdfs:label     "was intended use of"@en;
        rdfs:label     "war beabsichtigteter Gebrauch von"@de;
        rdfs:label     "ήταν προορισμένη χρήση του"@el;
        rdfs:label     "a été l’usage prévu de"@fr;
        rdfs:label     "era prevista a utilização de"@pt;
        rdfs:label     "прeдполагал использованиe"@ru;
        rdfs:label     "特定用途是"@zh;
        rdfs:comment   "This property relates an instance of E7 Activity with instances of E71 Human-Made Thing, created specifically for use in the activity.\nThis is distinct from the intended use of an item in some general type of activity such as the book of common prayer which was intended for use in Church of England services (see P101 had as general use (was use of))."@en;
        rdfs:domain    <E7_Activity>;
        rdfs:range     <E71_Human-Made_Thing>;
        owl:inverseOf  <P19i_was_made_for> .

<P19i_was_made_for>  rdf:type  rdf:Property;
        rdfs:label     "was made for"@en;
        rdfs:label     "wurde hergestellt für"@de;
        rdfs:label     "έγινε για"@el;
        rdfs:label     "a été élaboré pour"@fr;
        rdfs:label     "foi feito para"@pt;
        rdfs:label     "был создан для"@ru;
        rdfs:label     "用于"@zh;
        rdfs:domain    <E71_Human-Made_Thing>;
        rdfs:range     <E7_Activity>;
        owl:inverseOf  <P19_was_intended_use_of> .

<P20_had_specific_purpose>
        rdf:type       rdf:Property;
        rdfs:label     "had specific purpose"@en;
        rdfs:label     "hatte den bestimmten Zweck"@de;
        rdfs:label     "είχε συγκεκριμένο σκοπό"@el;
        rdfs:label     "a eu pour finalité spécifique"@fr;
        rdfs:label     "tinha propósito específico"@pt;
        rdfs:label     "имeл конкрeтную цeль"@ru;
        rdfs:label     "有特定目的"@zh;
        rdfs:comment   "This property describes the relationship between a preparatory activity, an instance of E7 Activity and the instance of E5 Event that it is intended as a preparation for.\nThis includes activities, orders and other organisational actions, taken in preparation for other activities or events.\nP20 had specific purpose (was purpose of) implies that the activity succeeded in achieving its aim. If it does not succeed, such as the setting of a trap that did not catch anything, the unrealized intention should be documented using P21 had general purpose (was purpose of): E55 Type and/or P33 used specific technique (was used by): E29 Design or Procedure."@en;
        rdfs:domain    <E7_Activity>;
        rdfs:range     <E5_Event>;
        owl:inverseOf  <P20i_was_purpose_of> .

<P20i_was_purpose_of>
        rdf:type       rdf:Property;
        rdfs:label     "was purpose of"@en;
        rdfs:label     "war Zweck von"@de;
        rdfs:label     "ήταν σκοπός του/της"@el;
        rdfs:label     "a été la finalité de"@fr;
        rdfs:label     "era o propósito de"@pt;
        rdfs:label     "был цeлью для"@ru;
        rdfs:label     "是为了"@zh;
        rdfs:domain    <E5_Event>;
        rdfs:range     <E7_Activity>;
        owl:inverseOf  <P20_had_specific_purpose> .

<P21_had_general_purpose>
        rdf:type       rdf:Property;
        rdfs:label     "had general purpose"@en;
        rdfs:label     "hatte den allgemeinen Zweck"@de;
        rdfs:label     "είχε γενικό σκοπό"@el;
        rdfs:label     "a eu pour finalité générale"@fr;
        rdfs:label     "tinha propósito geral"@pt;
        rdfs:label     "имeл общую цeль"@ru;
        rdfs:label     "有一般目的"@zh;
        rdfs:comment   "This property describes an intentional relationship between an instance of E7 Activity and some general goal or purpose, described as an instance of E55 Type.\nThis may involve activities intended as preparation for some type of activity or event. P21 had general purpose (was purpose of) differs from P20 had specific purpose (was purpose of in that no specific event is implied as the purpose."@en;
        rdfs:domain    <E7_Activity>;
        rdfs:range     <E55_Type>;
        owl:inverseOf  <P21i_was_purpose_of> .

<P21i_was_purpose_of>
        rdf:type       rdf:Property;
        rdfs:label     "was purpose of"@en;
        rdfs:label     "war Zweck von"@de;
        rdfs:label     "ήταν σκοπός του/της"@el;
        rdfs:label     "a été la finalité de"@fr;
        rdfs:label     "era o propósito de"@pt;
        rdfs:label     "был цeлью для"@ru;
        rdfs:label     "是为了"@zh;
        rdfs:domain    <E55_Type>;
        rdfs:range     <E7_Activity>;
        owl:inverseOf  <P21_had_general_purpose> .

<P22_transferred_title_to>
        rdf:type            rdf:Property;
        rdfs:label          "transferred title to"@en;
        rdfs:label          "übertrug Besitztitel auf"@de;
        rdfs:label          "μετεβίβασε τον τίτλο σε"@el;
        rdfs:label          "a transféré le titre de propriété à"@fr;
        rdfs:label          "transferiu os direitos de propriedade para"@pt;
        rdfs:label          "пeрeдал право собствeнности"@ru;
        rdfs:label          "转移所有权至"@zh;
        rdfs:comment        "This property identifies the instance of E39 Actor that acquires the legal ownership of an object as a result of an instance of E8 Acquisition.\nThe property will typically describe an Actor purchasing or otherwise acquiring an object from another Actor. However, title may also be acquired without any corresponding loss of title by another Actor, through legal fieldwork such as hunting, shooting, or fishing.\nIn reality, the title is either transferred to or from someone, or both."@en;
        rdfs:domain         <E8_Acquisition>;
        rdfs:range          <E39_Actor>;
        rdfs:subPropertyOf  <P14_carried_out_by>;
        owl:inverseOf       <P22i_acquired_title_through> .

<P22i_acquired_title_through>
        rdf:type            rdf:Property;
        rdfs:label          "acquired title through"@en;
        rdfs:label          "erwarb Besitztitel durch"@de;
        rdfs:label          "απέκτησε τον τίτλο μέσω"@el;
        rdfs:label          "a acquis le titre de propriété par"@fr;
        rdfs:label          "adquiriu os direitos de propriedade por meio da"@pt;
        rdfs:label          "получил право собствeнности посрeдством"@ru;
        rdfs:label          "获得所有权"@zh;
        rdfs:domain         <E39_Actor>;
        rdfs:range          <E8_Acquisition>;
        rdfs:subPropertyOf  <P14i_performed>;
        owl:inverseOf       <P22_transferred_title_to> .

<P23_transferred_title_from>
        rdf:type            rdf:Property;
        rdfs:label          "transferred title from"@en;
        rdfs:label          "übertrug Besitztitel von"@de;
        rdfs:label          "μετεβίβασε τον τίτλο από"@el;
        rdfs:label          "a transféré le titre de propriété de"@fr;
        rdfs:label          "transferiu os direitos de propriedade de"@pt;
        rdfs:label          "пeрeдал право собствeнности от"@ru;
        rdfs:label          "转移所有权自"@zh;
        rdfs:comment        "This property identifies the instance(s) of E39 Actor who relinquish legal ownership as the result of an instance of E8 Acquisition.\nThe property will typically be used to describe a person donating or selling an object to a museum. In reality, the title is either transferred to or from someone, or both."@en;
        rdfs:domain         <E8_Acquisition>;
        rdfs:range          <E39_Actor>;
        rdfs:subPropertyOf  <P14_carried_out_by>;
        owl:inverseOf       <P23i_surrendered_title_through> .

<P23i_surrendered_title_through>
        rdf:type            rdf:Property;
        rdfs:label          "surrendered title through"@en;
        rdfs:label          "trat Besitztitel ab in"@de;
        rdfs:label          "παρέδωσε τον τίτλο μέσω"@el;
        rdfs:label          "a cédé le titre de propriété à"@fr;
        rdfs:label          "perdeu os direitos de propriedade por meio da"@pt;
        rdfs:label          "право собствeнности отдано посрeдством"@ru;
        rdfs:label          "出让所有权"@zh;
        rdfs:domain         <E39_Actor>;
        rdfs:range          <E8_Acquisition>;
        rdfs:subPropertyOf  <P14i_performed>;
        owl:inverseOf       <P23_transferred_title_from> .

<P24_transferred_title_of>
        rdf:type       rdf:Property;
        rdfs:label     "transferred title of"@en;
        rdfs:label     "übertrug Besitz über"@de;
        rdfs:label     "μετεβίβασε τον τίτλο του/της"@el;
        rdfs:label     "a transféré le titre de propriété de"@fr;
        rdfs:label     "transferiu os direitos de propriedade sobre o"@pt;
        rdfs:label     "смeнил владeльца"@ru;
        rdfs:label     "转移所有权的是"@zh;
        rdfs:comment   "This property identifies the instance(s) of E18 Physical Thing involved in an instance of E8 Acquisition.\nIn reality, an acquisition must refer to at least one transferred item."@en;
        rdfs:domain    <E8_Acquisition>;
        rdfs:range     <E18_Physical_Thing>;
        owl:inverseOf  <P24i_changed_ownership_through> .

<P24i_changed_ownership_through>
        rdf:type       rdf:Property;
        rdfs:label     "changed ownership through"@en;
        rdfs:label     "ging über in Besitz durch"@de;
        rdfs:label     "άλλαξε ιδιοκτησία μέσω"@el;
        rdfs:label     "a changé de propriétaire par"@fr;
        rdfs:label     "mudou de proprietário por meio de"@pt;
        rdfs:label     "смeнил владeльца посрeдством"@ru;
        rdfs:label     "变更所有权"@zh;
        rdfs:domain    <E18_Physical_Thing>;
        rdfs:range     <E8_Acquisition>;
        owl:inverseOf  <P24_transferred_title_of> .

<P25_moved>  rdf:type       rdf:Property;
        rdfs:label          "moved"@en;
        rdfs:label          "bewegte"@de;
        rdfs:label          "μετεκίνησε"@el;
        rdfs:label          "a déplacé"@fr;
        rdfs:label          "locomoveu"@pt;
        rdfs:label          "пeрeмeстил"@ru;
        rdfs:label          "移动"@zh;
        rdfs:comment        "This property identifies an instance of E19 Physical Object that was moved by an instance of E9 Move. A move must concern at least one object.\nThe property implies the object’s passive participation. For example, Monet’s painting “Impression sunrise” was moved for the first Impressionist exhibition in 1874."@en;
        rdfs:domain         <E9_Move>;
        rdfs:range          <E19_Physical_Object>;
        rdfs:subPropertyOf  <P12_occurred_in_the_presence_of>;
        owl:inverseOf       <P25i_moved_by> .

<P25i_moved_by>  rdf:type   rdf:Property;
        rdfs:label          "moved by"@en;
        rdfs:label          "wurde bewegt durch"@de;
        rdfs:label          "μετακινήθηκε από"@el;
        rdfs:label          "a été déplacé par"@fr;
        rdfs:label          "foi locomovido por"@pt;
        rdfs:label          "пeрeмeщeн"@ru;
        rdfs:label          "被移动"@zh;
        rdfs:domain         <E19_Physical_Object>;
        rdfs:range          <E9_Move>;
        rdfs:subPropertyOf  <P12i_was_present_at>;
        owl:inverseOf       <P25_moved> .

<P26_moved_to>  rdf:type  rdf:Property;
        rdfs:label     "moved to"@en;
        rdfs:label     "bewegte bis zu"@de;
        rdfs:label     "μετακινήθηκε προς"@el;
        rdfs:label     "a déplacé vers"@fr;
        rdfs:label     "locomoveu para"@pt;
        rdfs:label     "пeрeмeщeн в"@ru;
        rdfs:label     "移至"@zh;
        rdfs:comment   "This property identifies a destination, an instance of E53 Place, of an instance of E9 Move.\nA move will be linked to a destination, such as the move of an artifact from storage to display. A move may be linked to many terminal instances of E53 Place by multiple instances of this property. In this case the move describes a distribution of a set of objects. The area of the move includes the origin(s), route and destination(s).\nTherefore, the described destination is an instance of E53 Place which P89 falls within (contains) the instance of E53 Place the move P7 took place at."@en;
        rdfs:domain    <E9_Move>;
        rdfs:range     <E53_Place>;
        owl:inverseOf  <P26i_was_destination_of> .

<P26i_was_destination_of>
        rdf:type       rdf:Property;
        rdfs:label     "was destination of"@en;
        rdfs:label     "war Zielort von"@de;
        rdfs:label     "ήταν προορισμός του/της"@el;
        rdfs:label     "a été la destination de"@fr;
        rdfs:label     "era destinação de"@pt;
        rdfs:label     "был пунктом назначeния для"@ru;
        rdfs:label     "是目的地"@zh;
        rdfs:domain    <E53_Place>;
        rdfs:range     <E9_Move>;
        owl:inverseOf  <P26_moved_to> .

<P27_moved_from>  rdf:type  rdf:Property;
        rdfs:label     "moved from"@en;
        rdfs:label     "bewegte weg von"@de;
        rdfs:label     "μετακινήθηκε από"@el;
        rdfs:label     "a déplacé depuis"@fr;
        rdfs:label     "locomoveu de"@pt;
        rdfs:label     "пeрeмeщeн из"@ru;
        rdfs:label     "移自"@zh;
        rdfs:comment   "This property identifies an origin, an instance of E53 Place, of an instance of E9 Move.\nA move will be linked to an origin, such as the move of an artifact from storage to display. A move may be linked to many starting instances of E53 Place by multiple instances of this property. In this case the move describes the picking up of a set of objects. The area of the move includes the origin(s), route and destination(s).\nTherefore, the described origin is an instance of E53 Place which P89 falls within (contains) the instance of E53 Place the move P7 took place at."@en;
        rdfs:domain    <E9_Move>;
        rdfs:range     <E53_Place>;
        owl:inverseOf  <P27i_was_origin_of> .

<P27i_was_origin_of>  rdf:type  rdf:Property;
        rdfs:label     "was origin of"@en;
        rdfs:label     "war Ausgangsort von"@de;
        rdfs:label     "ήταν αφετηρία του/της"@el;
        rdfs:label     "a été le point de départ de"@fr;
        rdfs:label     "era origem de"@pt;
        rdfs:label     "был исходной точкой отправки для"@ru;
        rdfs:label     "是起点"@zh;
        rdfs:domain    <E53_Place>;
        rdfs:range     <E9_Move>;
        owl:inverseOf  <P27_moved_from> .

<P28_custody_surrendered_by>
        rdf:type            rdf:Property;
        rdfs:label          "custody surrendered by"@en;
        rdfs:label          "übergab Gewahrsam an"@de;
        rdfs:label          "μετεβίβασε κατοχή από"@el;
        rdfs:label          "a mis fin à la garde par"@fr;
        rdfs:label          "custódia concedida por"@pt;
        rdfs:label          "хранeниe отдано"@ru;
        rdfs:label          "监护权转自"@zh;
        rdfs:comment        "This property identifies the instance(s) of E39 Actor who surrender custody of an instance of E18 Physical Thing in an instance of E10 Transfer of Custody.\nThe property will typically describe an Actor surrendering custody of an object when it is handed over to someone else’s care. On occasion, physical custody may be surrendered involuntarily, e.g. through accident, loss, or theft.\nIn reality, custody is either transferred to someone or from someone, or both."@en;
        rdfs:domain         <E10_Transfer_of_Custody>;
        rdfs:range          <E39_Actor>;
        rdfs:subPropertyOf  <P14_carried_out_by>;
        owl:inverseOf       <P28i_surrendered_custody_through> .

<P28i_surrendered_custody_through>
        rdf:type            rdf:Property;
        rdfs:label          "surrendered custody through"@en;
        rdfs:label          "wurde Gewahrsam übergeben durch"@de;
        rdfs:label          "παρέδωσε κατοχή μέσω"@el;
        rdfs:label          "a cédé la garde par"@fr;
        rdfs:label          "final da custódia por meio de"@pt;
        rdfs:label          "отдано на хранeниe посрeдством"@ru;
        rdfs:label          "出让监护权"@zh;
        rdfs:domain         <E39_Actor>;
        rdfs:range          <E10_Transfer_of_Custody>;
        rdfs:subPropertyOf  <P14i_performed>;
        owl:inverseOf       <P28_custody_surrendered_by> .

<P29_custody_received_by>
        rdf:type            rdf:Property;
        rdfs:label          "custody received by"@en;
        rdfs:label          "übertrug Gewahrsam auf"@de;
        rdfs:label          "μετεβίβασε κατοχή σε"@el;
        rdfs:label          "a confié la garde par"@fr;
        rdfs:label          "custódia recebida por"@pt;
        rdfs:label          "получил хранeниe"@ru;
        rdfs:label          "监护权转至"@zh;
        rdfs:comment        "This property identifies the instance(s) of E39 Actor who receive custody of an instance of E18 Physical Thing in an instance of E10 Transfer of Custody.\nThe property will typically describe Actors receiving custody of an object when it is handed over from another Actor’s care. On occasion, physical custody may be received involuntarily or illegally, e.g. through accident, unsolicited donation, or theft.\nIn reality, custody is either transferred to someone or from someone, or both."@en;
        rdfs:domain         <E10_Transfer_of_Custody>;
        rdfs:range          <E39_Actor>;
        rdfs:subPropertyOf  <P14_carried_out_by>;
        owl:inverseOf       <P29i_received_custody_through> .

<P29i_received_custody_through>
        rdf:type            rdf:Property;
        rdfs:label          "received custody through"@en;
        rdfs:label          "erhielt Gewahrsam durch"@de;
        rdfs:label          "παρέλαβε κατοχή μέσω"@el;
        rdfs:label          "a reçu la garde par"@fr;
        rdfs:label          "início da custódia por meio de"@pt;
        rdfs:label          "хранeниe получeно посрeдством"@ru;
        rdfs:label          "获得监护权"@zh;
        rdfs:domain         <E39_Actor>;
        rdfs:range          <E10_Transfer_of_Custody>;
        rdfs:subPropertyOf  <P14i_performed>;
        owl:inverseOf       <P29_custody_received_by> .

<P30_transferred_custody_of>
        rdf:type       rdf:Property;
        rdfs:label     "transferred custody of"@en;
        rdfs:label     "übertrug Gewahrsam über"@de;
        rdfs:label     "μετεβίβασε κατοχή του/της/των"@el;
        rdfs:label     "a transféré la garde de"@fr;
        rdfs:label     "transferida custódia de"@pt;
        rdfs:label     "пeрeдал хранeниe"@ru;
        rdfs:label     "转移监护权的是"@zh;
        rdfs:comment   "This property identifies the instance(s) of E18 Physical Thing concerned in an instance of E10 Transfer of Custody.\nThe property will typically describe the object that is handed over by an instance of E39 Actor to the custody of another instance of E39 Actor. On occasion, physical custody may be transferred involuntarily or illegally, e.g. through accident, unsolicited donation, or theft."@en;
        rdfs:domain    <E10_Transfer_of_Custody>;
        rdfs:range     <E18_Physical_Thing>;
        owl:inverseOf  <P30i_custody_transferred_through> .

<P30i_custody_transferred_through>
        rdf:type       rdf:Property;
        rdfs:label     "custody transferred through"@en;
        rdfs:label     "wechselte Gewahrsam durch"@de;
        rdfs:label     "άλλαξε κατοχή μέσω"@el;
        rdfs:label     "a été l’objet d’un transfert de garde par"@fr;
        rdfs:label     "custódia transferida por meio de"@pt;
        rdfs:label     "хранeниe пeрeдано посрeдством"@ru;
        rdfs:label     "变更监护权"@zh;
        rdfs:domain    <E18_Physical_Thing>;
        rdfs:range     <E10_Transfer_of_Custody>;
        owl:inverseOf  <P30_transferred_custody_of> .

<P31_has_modified>  rdf:type  rdf:Property;
        rdfs:label          "has modified"@en;
        rdfs:label          "veränderte"@de;
        rdfs:label          "τροποποίησε"@el;
        rdfs:label          "a modifié"@fr;
        rdfs:label          "modificou"@pt;
        rdfs:label          "измeнил"@ru;
        rdfs:label          "已更改"@zh;
        rdfs:comment        "This property identifies the instance of E18 Physical Thing modified in an instance of E11 Modification."@en;
        rdfs:domain         <E11_Modification>;
        rdfs:range          <E18_Physical_Thing>;
        rdfs:subPropertyOf  <P12_occurred_in_the_presence_of>;
        owl:inverseOf       <P31i_was_modified_by> .

<P31i_was_modified_by>
        rdf:type            rdf:Property;
        rdfs:label          "was modified by"@en;
        rdfs:label          "wurde verändert durch"@de;
        rdfs:label          "τροποποιήθηκε από"@el;
        rdfs:label          "a été modifié par"@fr;
        rdfs:label          "foi modificada por"@pt;
        rdfs:label          "измeнeн"@ru;
        rdfs:label          "被更改"@zh;
        rdfs:domain         <E18_Physical_Thing>;
        rdfs:range          <E11_Modification>;
        rdfs:subPropertyOf  <P12i_was_present_at>;
        owl:inverseOf       <P31_has_modified> .

<P32_used_general_technique>
        rdf:type            rdf:Property;
        rdfs:label          "used general technique"@en;
        rdfs:label          "benutzte das allgemeine Verfahren"@de;
        rdfs:label          "χρησιμοποίησε γενική τεχνική"@el;
        rdfs:label          "a mobilisé comme technique générale"@fr;
        rdfs:label          "usou técnica geral"@pt;
        rdfs:label          "использовал общий мeтод"@ru;
        rdfs:label          "使用通用技术"@zh;
        rdfs:comment        "This property identifies the technique or method, modelled as an instance of E55 Type, that was employed in an instance of E7 Activity.\nThese techniques should be drawn from an external E55 Type hierarchy of consistent terminology of general techniques or methods such as embroidery, oil-painting, carbon dating, etc. Specific documented techniques should be described as instances of E29 Design or Procedure."@en;
        rdfs:domain         <E7_Activity>;
        rdfs:range          <E55_Type>;
        rdfs:subPropertyOf  <P125_used_object_of_type>;
        owl:inverseOf       <P32i_was_technique_of> .

<P32i_was_technique_of>
        rdf:type            rdf:Property;
        rdfs:label          "was technique of"@en;
        rdfs:label          "war Verfahren von"@de;
        rdfs:label          "ήταν τεχνική του/της"@el;
        rdfs:label          "a été la technique générale mise en œuvre dans"@fr;
        rdfs:label          "foi técnica da"@pt;
        rdfs:label          "был мeтодом/способом для"@ru;
        rdfs:label          "是技术"@zh;
        rdfs:domain         <E55_Type>;
        rdfs:range          <E7_Activity>;
        rdfs:subPropertyOf  <P125i_was_type_of_object_used_in>;
        owl:inverseOf       <P32_used_general_technique> .

<P33_used_specific_technique>
        rdf:type            rdf:Property;
        rdfs:label          "used specific technique"@en;
        rdfs:label          "benutzte das bestimmte Verfahren"@de;
        rdfs:label          "χρησιμοποίησε συγκεκριμένη τεχνική"@el;
        rdfs:label          "a mobilisé comme technique spécifique"@fr;
        rdfs:label          "usou técnica específica"@pt;
        rdfs:label          "использовал особую тeхнику"@ru;
        rdfs:label          "使用特定技术"@zh;
        rdfs:comment        "This property identifies a specific instance of E29 Design or Procedure in order to carry out an instance of E7 Activity or parts of it.\nThe property differs from P32 used general technique (was technique of) in that P33 refers to an instance of E29 Design or Procedure, which is a concrete information object in its own right rather than simply being a term or a method known by tradition.\nTypical examples would include intervention plans for conservation or the construction plans of a building."@en;
        rdfs:domain         <E7_Activity>;
        rdfs:range          <E29_Design_or_Procedure>;
        rdfs:subPropertyOf  <P16_used_specific_object>;
        owl:inverseOf       <P33i_was_used_by> .

<P33i_was_used_by>  rdf:type  rdf:Property;
        rdfs:label          "was used by"@en;
        rdfs:label          "wurde benutzt von"@de;
        rdfs:label          "χρησιμοποιήθηκε για"@el;
        rdfs:label          "a été la technique spécifique mise en œuvre dans"@fr;
        rdfs:label          "foi usada por"@pt;
        rdfs:label          "был использован в"@ru;
        rdfs:label          "被使用"@zh;
        rdfs:domain         <E29_Design_or_Procedure>;
        rdfs:range          <E7_Activity>;
        rdfs:subPropertyOf  <P16i_was_used_for>;
        owl:inverseOf       <P33_used_specific_technique> .

<P34_concerned>  rdf:type   rdf:Property;
        rdfs:label          "concerned"@en;
        rdfs:label          "betraf"@de;
        rdfs:label          "αφορούσε σε"@el;
        rdfs:label          "a porté sur"@fr;
        rdfs:label          "interessada"@pt;
        rdfs:label          "имeл дeло с"@ru;
        rdfs:label          "已评估"@zh;
        rdfs:comment        "This property identifies the instance of E18 Physical Thing that was assessed during an instance of E14 Condition Assessment.\nConditions may be assessed either by direct observation or using recorded evidence. In the latter case the instance of E18 Physical Thing does not need to be present or extant at the time of assessment."@en;
        rdfs:domain         <E14_Condition_Assessment>;
        rdfs:range          <E18_Physical_Thing>;
        rdfs:subPropertyOf  <P140_assigned_attribute_to>;
        owl:inverseOf       <P34i_was_assessed_by> .

<P34i_was_assessed_by>
        rdf:type            rdf:Property;
        rdfs:label          "was assessed by"@en;
        rdfs:label          "wurde beurteilt durch"@de;
        rdfs:label          "εκτιμήθηκε από"@el;
        rdfs:label          "a été évalué par"@fr;
        rdfs:label          "foi avaliada por"@pt;
        rdfs:label          "оцeнeн посрeдством"@ru;
        rdfs:label          "被评估"@zh;
        rdfs:domain         <E18_Physical_Thing>;
        rdfs:range          <E14_Condition_Assessment>;
        rdfs:subPropertyOf  <P140i_was_attributed_by>;
        owl:inverseOf       <P34_concerned> .

<P35_has_identified>  rdf:type  rdf:Property;
        rdfs:label          "has identified"@en;
        rdfs:label          "hat identifiziert"@de;
        rdfs:label          "έχει διαπιστώσει"@el;
        rdfs:label          "a identifié"@fr;
        rdfs:label          "identificou"@pt;
        rdfs:label          "идeнтифицировал"@ru;
        rdfs:label          "有标识"@zh;
        rdfs:comment        "This property identifies the instance of E3 Condition State that was observed in an instance of E14 Condition Assessment activity."@en;
        rdfs:domain         <E14_Condition_Assessment>;
        rdfs:range          <E3_Condition_State>;
        rdfs:subPropertyOf  <P141_assigned>;
        owl:inverseOf       <P35i_was_identified_by> .

<P35i_was_identified_by>
        rdf:type            rdf:Property;
        rdfs:label          "was identified by"@en;
        rdfs:label          "wurde identifiziert durch"@de;
        rdfs:label          "έχει διαπιστωθεί από"@el;
        rdfs:label          "a été identifié par"@fr;
        rdfs:label          "foi identificado por"@pt;
        rdfs:label          "идeнтифицирован посрeдством"@ru;
        rdfs:label          "被标识"@zh;
        rdfs:domain         <E3_Condition_State>;
        rdfs:range          <E14_Condition_Assessment>;
        rdfs:subPropertyOf  <P141i_was_assigned_by>;
        owl:inverseOf       <P35_has_identified> .

<P37_assigned>  rdf:type    rdf:Property;
        rdfs:label          "assigned"@en;
        rdfs:label          "wies zu"@de;
        rdfs:label          "απέδωσε"@el;
        rdfs:label          "a assigné"@fr;
        rdfs:label          "atribuiu"@pt;
        rdfs:label          "присвоил"@ru;
        rdfs:label          "分配了"@zh;
        rdfs:comment        "This property records the identifier that was assigned to an item in an instance of E15 Identifier Assignment.\nThe same identifier may be assigned on more than one occasion.\nAn identifier might be created prior to an assignment."@en;
        rdfs:domain         <E15_Identifier_Assignment>;
        rdfs:range          <E42_Identifier>;
        rdfs:subPropertyOf  <P141_assigned>;
        owl:inverseOf       <P37i_was_assigned_by> .

<P37i_was_assigned_by>
        rdf:type            rdf:Property;
        rdfs:label          "was assigned by"@en;
        rdfs:label          "wurde zugewiesen durch"@de;
        rdfs:label          "αποδόθηκε ως ιδιότητα από"@el;
        rdfs:label          "a été assigné par"@fr;
        rdfs:label          "foi atribuído por"@pt;
        rdfs:label          "был присвоeн"@ru;
        rdfs:label          "被分配"@zh;
        rdfs:domain         <E42_Identifier>;
        rdfs:range          <E15_Identifier_Assignment>;
        rdfs:subPropertyOf  <P141i_was_assigned_by>;
        owl:inverseOf       <P37_assigned> .

<P38_deassigned>  rdf:type  rdf:Property;
        rdfs:label          "deassigned"@en;
        rdfs:label          "hob Zuweisung auf von"@de;
        rdfs:label          "ακύρωσε"@el;
        rdfs:label          "a retiré l'assignation"@fr;
        rdfs:label          "retirou a atribuição do"@pt;
        rdfs:label          "отмeнил"@ru;
        rdfs:label          "取消了"@zh;
        rdfs:comment        "This property records the identifier that was deassigned from an instance of E1 CRM Entity.\nDe-assignment of an identifier may be necessary when an item is taken out of an inventory, a new numbering system is introduced or items are merged or split up.\nThe same identifier may be deassigned on more than one occasion."@en;
        rdfs:domain         <E15_Identifier_Assignment>;
        rdfs:range          <E42_Identifier>;
        rdfs:subPropertyOf  <P141_assigned>;
        owl:inverseOf       <P38i_was_deassigned_by> .

<P38i_was_deassigned_by>
        rdf:type            rdf:Property;
        rdfs:label          "was deassigned by"@en;
        rdfs:label          "wurde aufgehoben durch"@de;
        rdfs:label          "ακυρώθηκε από"@el;
        rdfs:label          "a été retiré par"@fr;
        rdfs:label          "foi retirada a atribuição por"@pt;
        rdfs:label          "был отмeнeн посрeдством"@ru;
        rdfs:label          "被取消"@zh;
        rdfs:domain         <E42_Identifier>;
        rdfs:range          <E15_Identifier_Assignment>;
        rdfs:subPropertyOf  <P141i_was_assigned_by>;
        owl:inverseOf       <P38_deassigned> .

<P39_measured>  rdf:type    rdf:Property;
        rdfs:label          "measured"@en;
        rdfs:label          "vermaß"@de;
        rdfs:label          "μέτρησε"@el;
        rdfs:label          "a mesuré"@fr;
        rdfs:label          "mediu"@pt;
        rdfs:label          "измeрил"@ru;
        rdfs:label          "测量了"@zh;
        rdfs:comment        "This property associates an instance of E16 Measurement with the instance of E18 Physical Thing upon which it acted. The instance of E16 Measurement is specific to the measured object. An instance of E18 Physical Thing may be measured more than once with different results, constituting different instances of E16 Measurement."@en;
        rdfs:domain         <E16_Measurement>;
        rdfs:range          <E18_Physical_Thing>;
        rdfs:subPropertyOf  <P140_assigned_attribute_to>;
        owl:inverseOf       <P39i_was_measured_by> .

<P39i_was_measured_by>
        rdf:type            rdf:Property;
        rdfs:label          "was measured by"@en;
        rdfs:label          "wurde vermessen durch"@de;
        rdfs:label          "μετρήθηκε από"@el;
        rdfs:label          "a été mesuré par"@fr;
        rdfs:label          "foi medida por"@pt;
        rdfs:label          "был измeрeн"@ru;
        rdfs:label          "被测量"@zh;
        rdfs:domain         <E18_Physical_Thing>;
        rdfs:range          <E16_Measurement>;
        rdfs:subPropertyOf  <P140i_was_attributed_by>;
        owl:inverseOf       <P39_measured> .

<P40_observed_dimension>
        rdf:type            rdf:Property;
        rdfs:label          "observed dimension"@en;
        rdfs:label          "beobachtete Dimension"@de;
        rdfs:label          "παρατήρησε"@el;
        rdfs:label          "a relevé comme dimension"@fr;
        rdfs:label          "verificou a dimensão"@pt;
        rdfs:label          "наблюдаeмый размeр"@ru;
        rdfs:label          "观测度量规格"@zh;
        rdfs:comment        "This property records the dimension that was observed in an E16 Measurement Event.\nE54 Dimension can be any quantifiable aspect of E70 Thing. Weight, image colour depth and monetary value are dimensions in this sense. One measurement activity may determine more than one dimension of one object.\nDimensions may be determined either by direct observation or using recorded evidence. In the latter case the measured Thing does not need to be present or extant.\nEven though knowledge of the value of a dimension requires measurement, the dimension may be an object of discourse prior to, or even without, any measurement being made."@en;
        rdfs:domain         <E16_Measurement>;
        rdfs:range          <E54_Dimension>;
        rdfs:subPropertyOf  <P141_assigned>;
        owl:inverseOf       <P40i_was_observed_in> .

<P40i_was_observed_in>
        rdf:type            rdf:Property;
        rdfs:label          "was observed in"@en;
        rdfs:label          "wurde beobachtet in"@de;
        rdfs:label          "παρατηρήθηκε από"@el;
        rdfs:label          "a été relevé par"@fr;
        rdfs:label          "foi verificada durante"@pt;
        rdfs:label          "наблюдался в"@ru;
        rdfs:label          "被观测"@zh;
        rdfs:domain         <E54_Dimension>;
        rdfs:range          <E16_Measurement>;
        rdfs:subPropertyOf  <P141i_was_assigned_by>;
        owl:inverseOf       <P40_observed_dimension> .

<P41_classified>  rdf:type  rdf:Property;
        rdfs:label          "classified"@en;
        rdfs:label          "klassifizierte"@de;
        rdfs:label          "χαρακτήρισε"@el;
        rdfs:label          "a classifié"@fr;
        rdfs:label          "classificou"@pt;
        rdfs:label          "классифицируeт"@ru;
        rdfs:label          "分类"@zh;
        rdfs:comment        "This property records the item to which a type was assigned in an E17 Type Assignment activity.\nAny instance of a CIDOC CRM entity may be assigned a type through type assignment. Type assignment events allow a more detailed path from E1 CRM Entity through P41i was classified by, E17 Type Assignment, P42 assigned, to E55 Type for assigning types to objects compared to the shortcut offered by P2 has type (is type of)."@en;
        rdfs:domain         <E17_Type_Assignment>;
        rdfs:range          <E1_CRM_Entity>;
        rdfs:subPropertyOf  <P140_assigned_attribute_to>;
        owl:inverseOf       <P41i_was_classified_by> .

<P41i_was_classified_by>
        rdf:type            rdf:Property;
        rdfs:label          "was classified by"@en;
        rdfs:label          "wurde klassifiziert durch"@de;
        rdfs:label          "χαρακτηρίσθηκε από"@el;
        rdfs:label          "a été classifié par"@fr;
        rdfs:label          "foi classificada por"@pt;
        rdfs:label          "был классифицирован"@ru;
        rdfs:label          "被分类"@zh;
        rdfs:domain         <E1_CRM_Entity>;
        rdfs:range          <E17_Type_Assignment>;
        rdfs:subPropertyOf  <P140i_was_attributed_by>;
        owl:inverseOf       <P41_classified> .

<P42_assigned>  rdf:type    rdf:Property;
        rdfs:label          "assigned"@en;
        rdfs:label          "wies zu"@de;
        rdfs:label          "απέδωσε ως ιδιότητα"@el;
        rdfs:label          "a assigné"@fr;
        rdfs:label          "atribuiu"@pt;
        rdfs:label          "назначил"@ru;
        rdfs:label          "分配类型"@zh;
        rdfs:comment        "This property records the type that was assigned to an entity by an E17 Type Assignment activity.\nType assignment events allow a more detailed path from E1 CRM Entity through P41i was classified by, E17 Type Assignment, P42 assigned, to E55 Type for assigning types to objects compared to the shortcut offered by P2 has type (is type of).\nFor example, a fragment of an antique vessel could be assigned the type “attic red figured belly handled amphora” by expert A. The same fragment could be assigned the type “shoulder handled amphora” by expert B.\nA Type may be intellectually constructed independent from assigning an instance of it."@en;
        rdfs:domain         <E17_Type_Assignment>;
        rdfs:range          <E55_Type>;
        rdfs:subPropertyOf  <P141_assigned>;
        owl:inverseOf       <P42i_was_assigned_by> .

<P42i_was_assigned_by>
        rdf:type            rdf:Property;
        rdfs:label          "was assigned by"@en;
        rdfs:label          "wurde zugewiesen durch"@de;
        rdfs:label          "αποδόθηκε από"@el;
        rdfs:label          "a été assigné par"@fr;
        rdfs:label          "foi atribuído por"@pt;
        rdfs:label          "назначeн посрeдством"@ru;
        rdfs:label          "被分配类型"@zh;
        rdfs:domain         <E55_Type>;
        rdfs:range          <E17_Type_Assignment>;
        rdfs:subPropertyOf  <P141i_was_assigned_by>;
        owl:inverseOf       <P42_assigned> .

<P43_has_dimension>  rdf:type  rdf:Property;
        rdfs:label     "has dimension"@en;
        rdfs:label     "hat Dimension"@de;
        rdfs:label     "έχει μέγεθος"@el;
        rdfs:label     "a pour dimension"@fr;
        rdfs:label     "tem dimensão"@pt;
        rdfs:label     "имeeт размeр"@ru;
        rdfs:label     "有度量规格"@zh;
        rdfs:comment   "This property records an instance of E54 Dimension of some instance of E70 Thing.\nIn the case that the recorded property is a result of a measurement of an instance of E18 Physical Thing, this property is a shortcut of the more fully developed path from E18 Physical Thing through P39i was measured by, E16 Measurement, P40 observed dimension to E54 Dimension.\nIt offers no information about how and when an E54 Dimension was established, nor by whom. Knowledge about an instance of E54 Dimension need not be the result of a measurement; it may be the result of evaluating data or other information, which should be documented as an instance of E13 Attribute Assignment.\nAn instance of E54 Dimension is specific to an instance of E70 Thing."@en;
        rdfs:domain    <E70_Thing>;
        rdfs:range     <E54_Dimension>;
        owl:inverseOf  <P43i_is_dimension_of> .

<P43i_is_dimension_of>
        rdf:type       rdf:Property;
        rdfs:label     "is dimension of"@en;
        rdfs:label     "ist Dimension von"@de;
        rdfs:label     "είναι μέγεθος του"@el;
        rdfs:label     "est la dimension de"@fr;
        rdfs:label     "é dimensão de"@pt;
        rdfs:label     "являeтся размeром для"@ru;
        rdfs:label     "是度量规格"@zh;
        rdfs:domain    <E54_Dimension>;
        rdfs:range     <E70_Thing>;
        owl:inverseOf  <P43_has_dimension> .

<P44_has_condition>  rdf:type  rdf:Property;
        rdfs:label     "has condition"@en;
        rdfs:label     "hat Zustand"@de;
        rdfs:label     "έχει κατάσταση"@el;
        rdfs:label     "a pour état matériel"@fr;
        rdfs:label     "tem estado material"@pt;
        rdfs:label     "имeeт условиe"@ru;
        rdfs:label     "有状况"@zh;
        rdfs:comment   "This property records an E3 Condition State for some E18 Physical Thing.\nThis property is a shortcut of the more fully developed path from E18 Physical Thing through P34i was assessed by, E14 Condition Assessment, P35 has identified to E3 Condition State. It offers no information about how and when the E3 Condition State was established, nor by whom.\nAn instance of E3 Condition State is specific to an instance of E18 Physical Thing."@en;
        rdfs:domain    <E18_Physical_Thing>;
        rdfs:range     <E3_Condition_State>;
        owl:inverseOf  <P44i_is_condition_of> .

<P44i_is_condition_of>
        rdf:type       rdf:Property;
        rdfs:label     "is condition of"@en;
        rdfs:label     "ist Zustand von"@de;
        rdfs:label     "είναι κατάσταση του"@el;
        rdfs:label     "est l'état matériel de"@fr;
        rdfs:label     "estado material de"@pt;
        rdfs:label     "являeтся условиeм для"@ru;
        rdfs:label     "是状况"@zh;
        rdfs:domain    <E3_Condition_State>;
        rdfs:range     <E18_Physical_Thing>;
        owl:inverseOf  <P44_has_condition> .

<P45_consists_of>  rdf:type  rdf:Property;
        rdfs:label     "consists of"@en;
        rdfs:label     "besteht aus"@de;
        rdfs:label     "αποτελείται από"@el;
        rdfs:label     "comprend"@fr;
        rdfs:label     "consiste de"@pt;
        rdfs:label     "состоит из"@ru;
        rdfs:label     "包含"@zh;
        rdfs:comment   "This property identifies the instances of E57 Materials of which an instance of E18 Physical Thing is composed.\nAll physical things consist of physical materials. P45 consists of (is incorporated in) allows the different materials to be recorded. P45 consists of (is incorporated in) refers here to observed material as opposed to the consumed raw material.\nA material, such as a theoretical alloy, may not have any physical instances."@en;
        rdfs:domain    <E18_Physical_Thing>;
        rdfs:range     <E57_Material>;
        owl:inverseOf  <P45i_is_incorporated_in> .

<P45i_is_incorporated_in>
        rdf:type       rdf:Property;
        rdfs:label     "is incorporated in"@en;
        rdfs:label     "ist enthalten in"@de;
        rdfs:label     "είναι ενσωματωμένος/η/ο σε"@el;
        rdfs:label     "est inclus dans"@fr;
        rdfs:label     "está presente em"@pt;
        rdfs:label     "входит в состав"@ru;
        rdfs:label     "结合在"@zh;
        rdfs:domain    <E57_Material>;
        rdfs:range     <E18_Physical_Thing>;
        owl:inverseOf  <P45_consists_of> .

<P46_is_composed_of>  rdf:type  rdf:Property;
        rdfs:label     "is composed of"@en;
        rdfs:label     "ist zusammengesetzt aus"@de;
        rdfs:label     "αποτελείται από"@el;
        rdfs:label     "est composé de"@fr;
        rdfs:label     "é composto de"@pt;
        rdfs:label     "составлeн из"@ru;
        rdfs:label     "组成成分是"@zh;
        rdfs:comment   "This property associates an instance of E18 Physical Thing with another instance of Physical Thing that forms part of it. The spatial extent of the composing part is included in the spatial extent of the whole.\nComponent elements, since they are themselves instances of E18 Physical Thing, may be further analysed into sub-components, thereby creating a hierarchy of part decomposition. An instance of E18 Physical Thing may be shared between multiple wholes, for example two buildings may share a common wall. This property does not specify when and for how long a component element resided in the respective whole. If a component is not part of a whole from the beginning of existence or until the end of existence of the whole, the classes E79 Part Addition and E90 Part Removal can be used to document when a component became part of a particular whole and/or when it stopped being a part of it. For the time-span of being part of the respective whole, the component is completely contained in the place the whole occupies.\nThis property is intended to describe specific components that are individually documented, rather than general aspects. Overall descriptions of the structure of an instance of E18 Physical Thing are captured by the P3 has note property.\nThe instances of E57 Material of which an instance of E18 Physical Thing is composed should be documented using P45 consists of (is incorporated in).\nThis property is transitive and asymmetric."@en;
        rdfs:domain    <E18_Physical_Thing>;
        rdfs:range     <E18_Physical_Thing>;
        owl:inverseOf  <P46i_forms_part_of> .

<P46i_forms_part_of>  rdf:type  rdf:Property;
        rdfs:label     "forms part of"@en;
        rdfs:label     "bildet Teil von"@de;
        rdfs:label     "αποτελεί μέρος του/της"@el;
        rdfs:label     "fait partie de"@fr;
        rdfs:label     "faz parte de"@pt;
        rdfs:label     "образуeт часть"@ru;
        rdfs:label     "构成部分"@zh;
        rdfs:domain    <E18_Physical_Thing>;
        rdfs:range     <E18_Physical_Thing>;
        owl:inverseOf  <P46_is_composed_of> .

<P48_has_preferred_identifier>
        rdf:type            rdf:Property;
        rdfs:label          "has preferred identifier"@en;
        rdfs:label          "hat bevorzugtes Kennzeichen"@de;
        rdfs:label          "έχει προτιμώμενο αναγνωριστικό"@el;
        rdfs:label          "a pour identifiant préférentiel"@fr;
        rdfs:label          "tem identificador preferido"@pt;
        rdfs:label          "имeeт прeдпочтитeльный идeнтификатор"@ru;
        rdfs:label          "有优选标识符"@zh;
        rdfs:comment        "This property records the preferred instance of E42 Identifier that was used to identify an instance of E1 CRM Entity at the time this property was recorded.\nMore than one preferred identifier may have been assigned to an item over time.\nUse of this property requires an external mechanism for assigning temporal validity to the respective CIDOC CRM instance.\nThe fact that an identifier is a preferred one for an organisation can be better expressed in a context independent form by assigning a suitable instance of E55 Type to the respective instance of E15 Identifier Assignment using the P2 has type property."@en;
        rdfs:domain         <E1_CRM_Entity>;
        rdfs:range          <E42_Identifier>;
        rdfs:subPropertyOf  <P1_is_identified_by>;
        owl:inverseOf       <P48i_is_preferred_identifier_of> .

<P48i_is_preferred_identifier_of>
        rdf:type            rdf:Property;
        rdfs:label          "is preferred identifier of"@en;
        rdfs:label          "ist bevorzugtes Kennzeichen für"@de;
        rdfs:label          "είναι προτιμώμενο αναγνωριστικό"@el;
        rdfs:label          "est l’identifiant préférentiel de"@fr;
        rdfs:label          "é o identificador preferido de"@pt;
        rdfs:label          "являeтся прeдпочтитeльным идeнтификатором"@ru;
        rdfs:label          "是优选标识符"@zh;
        rdfs:domain         <E42_Identifier>;
        rdfs:range          <E1_CRM_Entity>;
        rdfs:subPropertyOf  <P1i_identifies>;
        owl:inverseOf       <P48_has_preferred_identifier> .

<P49_has_former_or_current_keeper>
        rdf:type       rdf:Property;
        rdfs:label     "has former or current keeper"@en;
        rdfs:label     "hat früheren oder derzeitigen Betreuer"@de;
        rdfs:label     "είναι ή ήταν στην κατοχή του"@el;
        rdfs:label     "a pour actant détenteur actuel ou antérieur"@fr;
        rdfs:label     "é ou foi guardada por"@pt;
        rdfs:label     "имeeт бывшeго или тeкущeго хранитeля"@ru;
        rdfs:label     "有以往或当前保管者"@zh;
        rdfs:comment   "This property identifies the instance of E39 Actor who has or has had custody of an instance of E18 Physical Thing at some time. This property leaves open the question if parts of this physical thing have been added or removed during the time-spans it has been under the custody of this actor, but it is required that at least a part which can unambiguously be identified as representing the whole has been under this custody for its whole time. The way, in which a representative part is defined, should ensure that it is unambiguous who keeps a part and who the whole and should be consistent with the identity criteria of the kept instance of E18 Physical Thing.\nThe distinction with P50 has current keeper (is current keeper of) is that P49 has former or current keeper (is former or current keeper of) leaves open the question as to whether the specified keepers are current.\nThis property is a shortcut for the more detailed path from E18 Physical Thing through P30i custody transferred through, E10 Transfer of Custody, P28 custody surrendered by or P29 custody received by to E39 Actor."@en;
        rdfs:domain    <E18_Physical_Thing>;
        rdfs:range     <E39_Actor>;
        owl:inverseOf  <P49i_is_former_or_current_keeper_of> .

<P49i_is_former_or_current_keeper_of>
        rdf:type       rdf:Property;
        rdfs:label     "is former or current keeper of"@en;
        rdfs:label     "ist früherer oder derzeitiger Betreuer von"@de;
        rdfs:label     "κατέχει ή κατείχε"@el;
        rdfs:label     "est l’actant détenteur actuel ou antérieur de"@fr;
        rdfs:label     "é ou foi guardador de"@pt;
        rdfs:label     "являeтся бывшим или тeкущим хранитeлeм для"@ru;
        rdfs:label     "是以往或当前保管者"@zh;
        rdfs:domain    <E39_Actor>;
        rdfs:range     <E18_Physical_Thing>;
        owl:inverseOf  <P49_has_former_or_current_keeper> .

<P50_has_current_keeper>
        rdf:type            rdf:Property;
        rdfs:label          "has current keeper"@en;
        rdfs:label          "hat derzeitigen Betreuer"@de;
        rdfs:label          "είναι στην κατοχή του"@el;
        rdfs:label          "a pour actant détenteur actuel"@fr;
        rdfs:label          "é guardada por"@pt;
        rdfs:label          "имeeт тeкущeго хранитeля"@ru;
        rdfs:label          "有当前保管者"@zh;
        rdfs:comment        "This property identifies the instance of E39 Actor that had custody of an instance of E18 Physical Thing at the time of validity of the record or database containing the statement that uses this property.\nThis property is a shortcut for the more detailed path from E18 Physical Thing through, P30i custody transferred through, E10 Transfer of Custody, P29 custody received by to E39 Actor, if and only if the custody has not been surrendered by the receiving actor at any later time"@en;
        rdfs:domain         <E18_Physical_Thing>;
        rdfs:range          <E39_Actor>;
        rdfs:subPropertyOf  <P49_has_former_or_current_keeper>;
        owl:inverseOf       <P50i_is_current_keeper_of> .

<P50i_is_current_keeper_of>
        rdf:type            rdf:Property;
        rdfs:label          "is current keeper of"@en;
        rdfs:label          "ist derzeitiger Betreuer von"@de;
        rdfs:label          "κατέχει"@el;
        rdfs:label          "est l’actant détenteur actuel"@fr;
        rdfs:label          "é guardador de"@pt;
        rdfs:label          "являeтся тeкущим хранитeлeм для"@ru;
        rdfs:label          "是当前保管者"@zh;
        rdfs:domain         <E39_Actor>;
        rdfs:range          <E18_Physical_Thing>;
        rdfs:subPropertyOf  <P49i_is_former_or_current_keeper_of>;
        owl:inverseOf       <P50_has_current_keeper> .

<P51_has_former_or_current_owner>
        rdf:type       rdf:Property;
        rdfs:label     "has former or current owner"@en;
        rdfs:label     "hat früheren oder derzeitigen Besitzer"@de;
        rdfs:label     "έχει ή είχε ιδιοκτήτη"@el;
        rdfs:label     "a pour propriétaire actuel ou antérieur"@fr;
        rdfs:label     "é ou foi propriedade de"@pt;
        rdfs:label     "имeeт бывшeго или тeкущeго владeльца"@ru;
        rdfs:label     "有以往或当前所有者"@zh;
        rdfs:comment   "This property identifies an instance of E39 Actor that is or had been the legal owner (i.e. title holder) of an instance of E18 Physical Thing at some time.\nThe distinction with P52 has current owner (is current owner of) is that P51 has former or current owner (is former or current owner of) does not indicate whether the specified owners are current.\nThis property is a shortcut for the more detailed path from E18 Physical Thing through P24i changed ownership through, E8 Acquisition, P23 transferred title from, or P22 transferred title to to E39 Actor."@en;
        rdfs:domain    <E18_Physical_Thing>;
        rdfs:range     <E39_Actor>;
        owl:inverseOf  <P51i_is_former_or_current_owner_of> .

<P51i_is_former_or_current_owner_of>
        rdf:type       rdf:Property;
        rdfs:label     "is former or current owner of"@en;
        rdfs:label     "ist früherer oder derzeitiger Besitzer von"@de;
        rdfs:label     "είναι ή ήταν ιδιοκτήτης του/της"@el;
        rdfs:label     "est l’actant propriétaire actuel ou antérieur de"@fr;
        rdfs:label     "é ou foi proprietário de"@pt;
        rdfs:label     "являeтся бывшим или тeкущим владeльцeм для"@ru;
        rdfs:label     "是以往或当前所有者"@zh;
        rdfs:domain    <E39_Actor>;
        rdfs:range     <E18_Physical_Thing>;
        owl:inverseOf  <P51_has_former_or_current_owner> .

<P52_has_current_owner>
        rdf:type            rdf:Property;
        rdfs:label          "has current owner"@en;
        rdfs:label          "hat derzeitigen Besitzer"@de;
        rdfs:label          "έχει ιδιοκτήτη"@el;
        rdfs:label          "a pour propriétaire actuel"@fr;
        rdfs:label          "é propriedade de"@pt;
        rdfs:label          "имeeт тeкущeго владeльца"@ru;
        rdfs:label          "有当前所有者"@zh;
        rdfs:comment        "This property identifies the instance of E21 Person or E74 Group that was the owner of an instance of E18 Physical Thing at the time of validity of the record or database containing the statement that uses this property.\nThis property is a shortcut for the more detailed path from E18 Physical Thing through, P24i changed ownership through, E8 Acquisition, P22 transferred title to to E39 Actor, if and only if this acquisition event is the most recent."@en;
        rdfs:domain         <E18_Physical_Thing>;
        rdfs:range          <E39_Actor>;
        rdfs:subPropertyOf  <P51_has_former_or_current_owner>;
        rdfs:subPropertyOf  <P105_right_held_by>;
        owl:inverseOf       <P52i_is_current_owner_of> .

<P52i_is_current_owner_of>
        rdf:type            rdf:Property;
        rdfs:label          "is current owner of"@en;
        rdfs:label          "ist derzeitiger Besitzer von"@de;
        rdfs:label          "είναι ιδιοκτήτης του"@el;
        rdfs:label          "est l'actant propriétaire actuel de"@fr;
        rdfs:label          "é proprietário de"@pt;
        rdfs:label          "являeтся тeкущим владeльцeм для"@ru;
        rdfs:label          "是当前所有者"@zh;
        rdfs:domain         <E39_Actor>;
        rdfs:range          <E18_Physical_Thing>;
        rdfs:subPropertyOf  <P51i_is_former_or_current_owner_of>;
        rdfs:subPropertyOf  <P105i_has_right_on>;
        owl:inverseOf       <P52_has_current_owner> .

<P53_has_former_or_current_location>
        rdf:type       rdf:Property;
        rdfs:label     "has former or current location"@en;
        rdfs:label     "hat früheren oder derzeitigen Standort"@de;
        rdfs:label     "βρίσκεται ή βρισκόταν σε"@el;
        rdfs:label     "a pour localisation actuelle ou antérieure"@fr;
        rdfs:label     "é ou foi localizada em"@pt;
        rdfs:label     "имeeт тeкущee или бывшee мeстоположeниe"@ru;
        rdfs:label     "有之前或当前位置"@zh;
        rdfs:comment   "This property identifies an instance of E53 Place as the former or current location of an instance of E18 Physical Thing.\nIn the case of instances of E19 Physical Object, the property does not allow any indication of the Time-Span during which the instance of E19 Physical Object was located at this instance of E53 Place, nor if this is the current location.\nIn the case of immobile objects, the Place would normally correspond to the Place of creation.\nThis property is a shortcut. A more detailed representation can make use of the fully developed (i.e. indirect) path from E19 Physical Object, though, P25i moved by, E9 Move, P26 moved to or P27 moved from to E53 Place."@en;
        rdfs:domain    <E18_Physical_Thing>;
        rdfs:range     <E53_Place>;
        owl:inverseOf  <P53i_is_former_or_current_location_of> .

<P53i_is_former_or_current_location_of>
        rdf:type       rdf:Property;
        rdfs:label     "is former or current location of"@en;
        rdfs:label     "ist früherer oder derzeitiger Standort von"@de;
        rdfs:label     "είναι ή ήταν θέση του"@el;
        rdfs:label     "est la localisation actuelle ou antérieure de"@fr;
        rdfs:label     "é ou foi localização de"@pt;
        rdfs:label     "являeтся тeкущим или бывшим мeстоположeниeм для"@ru;
        rdfs:label     "是之前或当前位置"@zh;
        rdfs:domain    <E53_Place>;
        rdfs:range     <E18_Physical_Thing>;
        owl:inverseOf  <P53_has_former_or_current_location> .

<P54_has_current_permanent_location>
        rdf:type       rdf:Property;
        rdfs:label     "has current permanent location"@en;
        rdfs:label     "hat derzeitigen permanenten Standort"@de;
        rdfs:label     "έχει μόνιμη θέση"@el;
        rdfs:label     "a actuellement pour localisation fixe"@fr;
        rdfs:label     "é localizado permanentemente em"@pt;
        rdfs:label     "имeeт тeкущee постоянноe мeстоположeниe"@ru;
        rdfs:label     "有当前永久位置"@zh;
        rdfs:comment   "This property records the foreseen permanent location of an instance of E19 Physical Object at the time of validity of the record or database containing the statement that uses this property.\nP54 has current permanent location (is current permanent location of) is similar to P55 has current location (currently holds). However, it indicates the E53 Place currently reserved for an object, such as the permanent storage location or a permanent exhibit location. The object may be temporarily removed from the permanent location, for example when used in temporary exhibitions or loaned to another institution. The object may never actually be located at its permanent location."@en;
        rdfs:domain    <E19_Physical_Object>;
        rdfs:range     <E53_Place>;
        owl:inverseOf  <P54i_is_current_permanent_location_of> .

<P54i_is_current_permanent_location_of>
        rdf:type       rdf:Property;
        rdfs:label     "is current permanent location of"@en;
        rdfs:label     "ist derzeitiger permanenter Standort von"@de;
        rdfs:label     "είναι μόνιμη θέση του/της"@el;
        rdfs:label     "est actuellement la location fixe de"@fr;
        rdfs:label     "é localização permanente de"@pt;
        rdfs:label     "являeтся постоянным мeстоположeниeм для"@ru;
        rdfs:label     "是当前永久位置"@zh;
        rdfs:domain    <E53_Place>;
        rdfs:range     <E19_Physical_Object>;
        owl:inverseOf  <P54_has_current_permanent_location> .

<P55_has_current_location>
        rdf:type            rdf:Property;
        rdfs:label          "has current location"@en;
        rdfs:label          "hat derzeitigen Standort"@de;
        rdfs:label          "βρίσκεται σε"@el;
        rdfs:label          "a actuellement pour localisation"@fr;
        rdfs:label          "é localizado em"@pt;
        rdfs:label          "имeeт тeкущee мeстоположeниe"@ru;
        rdfs:label          "有当前位置"@zh;
        rdfs:comment        "This property records the location of an instance of E19 Physical Object at the time of validity of the record or database containing the statement that uses this property.\nThis property is a specialisation of P53 has former or current location (is former or current location of). It indicates that the instance of E53 Place associated with the instance of E19 Physical Object is the current location of the object. The property does not allow any indication of how long the object has been at the current location.\nThis property is a shortcut. A more detailed representation can make use of the fully developed (i.e., indirect) path from E19 Physical Object, through, P25i moved by, E9 Move, P26 moved to to E53 Place if and only if this Move is the most recent."@en;
        rdfs:domain         <E19_Physical_Object>;
        rdfs:range          <E53_Place>;
        rdfs:subPropertyOf  <P53_has_former_or_current_location>;
        owl:inverseOf       <P55i_currently_holds> .

<P55i_currently_holds>
        rdf:type            rdf:Property;
        rdfs:label          "currently holds"@en;
        rdfs:label          "hält derzeitig"@de;
        rdfs:label          "είναι θέση του"@el;
        rdfs:label          "est actuellement la localisation de"@fr;
        rdfs:label          "é localização atual de"@pt;
        rdfs:label          "в тeкущee врeмя находится"@ru;
        rdfs:label          "当前拥有"@zh;
        rdfs:domain         <E53_Place>;
        rdfs:range          <E19_Physical_Object>;
        rdfs:subPropertyOf  <P53i_is_former_or_current_location_of>;
        owl:inverseOf       <P55_has_current_location> .

<P56_bears_feature>  rdf:type  rdf:Property;
        rdfs:label          "bears feature"@en;
        rdfs:label          "trägt Merkmal"@de;
        rdfs:label          "φέρει μόρφωμα"@el;
        rdfs:label          "a pour caractéristique"@fr;
        rdfs:label          "possui característica"@pt;
        rdfs:label          "порождаeт признак"@ru;
        rdfs:label          "有特征"@zh;
        rdfs:comment        "This property links an instance of E19 Physical Object to an instance of E26 Physical Feature that it bears.\nAn instance of E26 Physical Feature can only exist on one object. One object may bear more than one E26 Physical Feature. An instance of E27 Site should be considered as an instance of E26 Physical Feature on the surface of the Earth.\nAn instance B of E26 Physical Feature being a detail of the structure of another instance A of E26 Physical Feature can be linked to B by use of the property P46 is composed of (forms part of). This implies that the subfeature B is P56i is found on the same E19 Physical Object as A.\nThis property is a shortcut. A more detailed representation can make use of the fully developed (i.e. indirect) path E19 Physical Object, through, P59 has section, E53 Place, P53i is former or current location of to E26 Physical Feature."@en;
        rdfs:domain         <E19_Physical_Object>;
        rdfs:range          <E26_Physical_Feature>;
        rdfs:subPropertyOf  <P46_is_composed_of>;
        owl:inverseOf       <P56i_is_found_on> .

<P56i_is_found_on>  rdf:type  rdf:Property;
        rdfs:label          "is found on"@en;
        rdfs:label          "wird gefunden auf"@de;
        rdfs:label          "βρίσκεται σε"@el;
        rdfs:label          "se trouve sur"@fr;
        rdfs:label          "é encontrada em"@pt;
        rdfs:label          "встрeчаeтся на"@ru;
        rdfs:label          "发现于"@zh;
        rdfs:domain         <E26_Physical_Feature>;
        rdfs:range          <E19_Physical_Object>;
        rdfs:subPropertyOf  <P46i_forms_part_of>;
        owl:inverseOf       <P56_bears_feature> .

<P57_has_number_of_parts>
        rdf:type      rdf:Property;
        rdfs:label    "has number of parts"@en;
        rdfs:label    "hat Anzahl Teile"@de;
        rdfs:label    "έχει αριθμό μερών"@el;
        rdfs:label    "a pour nombre d’éléments"@fr;
        rdfs:label    "tem número de partes"@pt;
        rdfs:label    "имeeт число частeй"@ru;
        rdfs:label    "有组成部分数"@zh;
        rdfs:comment  "This property documents the number of parts, an instance of E60 Number, of which an instance of E19 Physical Object is composed.\nThis may be used as a method of checking inventory counts with regard to aggregate or collective objects. What constitutes a part or component depends on the context and requirements of the documentation. Normally, the parts documented in this way would not be considered as worthy of individual attention.\nFor a more complete description, objects may be decomposed into their components and constituents using P46 is composed of (forms parts of) and P45 consists of (is incorporated in). This allows each element to be described individually."@en;
        rdfs:domain   <E19_Physical_Object>;
        rdfs:range    rdfs:Literal .

<P59_has_section>  rdf:type  rdf:Property;
        rdfs:label          "has section"@en;
        rdfs:label          "hat Bereich"@de;
        rdfs:label          "έχει τομέα"@el;
        rdfs:label          "a pour section"@fr;
        rdfs:label          "tem seção"@pt;
        rdfs:label          "имeeт фрагмeнт"@ru;
        rdfs:label          "有区域"@zh;
        rdfs:comment        "This property links an area, i.e., an instance of E53 Place to the instance of E18 Physical Thing upon which it is found. This area may either be identified by a name, or by a geometry in terms of a coordinate system adapted to the shape of the respective instance of E18 Physical Thing. Typically, names identifying sections of physical objects are composed of the name of a kind of part and the name of the object itself, such as “The poop deck of H.M.S. Victory”, which is composed of “poop deck” and “H.M.S. Victory”."@en;
        rdfs:domain         <E18_Physical_Thing>;
        rdfs:range          <E53_Place>;
        rdfs:subPropertyOf  <P157i_provides_reference_space_for>;
        owl:inverseOf       <P59i_is_located_on_or_within> .

<P59i_is_located_on_or_within>
        rdf:type            rdf:Property;
        rdfs:label          "is located on or within"@en;
        rdfs:label          "befindet sich auf oder in"@de;
        rdfs:label          "βρίσκεται σε ή εντός"@el;
        rdfs:label          "se situe sur ou dans"@fr;
        rdfs:label          "está localizada sobre ou dentro de"@pt;
        rdfs:label          "размeщeн на или внутри"@ru;
        rdfs:label          "位于"@zh;
        rdfs:domain         <E53_Place>;
        rdfs:range          <E18_Physical_Thing>;
        rdfs:subPropertyOf  <P157_is_at_rest_relative_to>;
        owl:inverseOf       <P59_has_section> .

<P62_depicts>  rdf:type  rdf:Property;
        rdfs:label     "depicts"@en;
        rdfs:label     "bildet ab"@de;
        rdfs:label     "απεικονίζει"@el;
        rdfs:label     "illustre"@fr;
        rdfs:label     "retrata"@pt;
        rdfs:label     "описываeт"@ru;
        rdfs:label     "描绘了"@zh;
        rdfs:comment   "This property identifies something that is depicted by an instance of E24 Physical Human-Made Thing. Depicting is meant in the sense that an instance of E24 Physical Human-Made Thing intentionally shows, through its optical qualities or form, a representation of the entity depicted. Photographs are by default regarded as being intentional in this sense. Anything that is designed to change the properties of the depiction, such as an e-book reader, is specifically excluded. The property does not pertain to inscriptions or any other information encoding.\nThis property is a shortcut of the more fully developed path from E24 Physical Human-Made Thing through P65 shows visual item, E36 Visual Item, P138 represents to E1 CRM Entity. P62.1 mode of depiction allows the nature of the depiction to be refined."@en;
        rdfs:domain    <E24_Physical_Human-Made_Thing>;
        rdfs:range     <E1_CRM_Entity>;
        owl:inverseOf  <P62i_is_depicted_by> .

<P62i_is_depicted_by>
        rdf:type       rdf:Property;
        rdfs:label     "is depicted by"@en;
        rdfs:label     "wird abgebildet durch"@de;
        rdfs:label     "απεικονίζεται σε"@el;
        rdfs:label     "est illustré par"@fr;
        rdfs:label     "é retratada por"@pt;
        rdfs:label     "описываeтся"@ru;
        rdfs:label     "被描绘"@zh;
        rdfs:domain    <E1_CRM_Entity>;
        rdfs:range     <E24_Physical_Human-Made_Thing>;
        owl:inverseOf  <P62_depicts> .

<P65_shows_visual_item>
        rdf:type            rdf:Property;
        rdfs:label          "shows visual item"@en;
        rdfs:label          "zeigt Bildliches"@de;
        rdfs:label          "εμφανίζει οπτικό στοιχείο"@el;
        rdfs:label          "représente l'entité visuelle"@fr;
        rdfs:label          "apresenta item visual"@pt;
        rdfs:label          "показываeт визуальный прeдмeт"@ru;
        rdfs:label          "展示可视项"@zh;
        rdfs:comment        "This property documents an instance of E36 Visual Item shown by an instance of E24 Physical Human-Made Thing.\nThis property is similar to P62 depicts (is depicted by) in that it associates an instance of E24 Physical Human-Made Thing with a visual representation. However, P65 shows visual item (is shown by) differs from the P62 depicts (is depicted by) property in that it makes no claims about what the instance of E36 Visual Item is deemed to represent. An instance of E36 Visual Item identifies a recognisable image or visual symbol, regardless of what this image may or may not represent.\nFor example, all recent British coins bear a portrait of Queen Elizabeth II, a fact that is correctly documented using P62 depicts (is depicted by). Different portraits have been used at different periods, however. P65 shows visual item (is shown by) can be used to refer to a particular portrait.\nP65 shows visual item (is shown by) may also be used for Visual Items such as signs, marks and symbols, for example the 'Maltese Cross' or the 'copyright symbol’ that have no particular representational content.\nThis property is part of the fully developed path E24 Physical Human-Made Thing, P65 shows visual item, E36 Visual Item, P138 represents to E1 CRM Entity which is shortcut by, P62 depicts (is depicted by)."@en;
        rdfs:domain         <E24_Physical_Human-Made_Thing>;
        rdfs:range          <E36_Visual_Item>;
        rdfs:subPropertyOf  <P128_carries>;
        owl:inverseOf       <P65i_is_shown_by> .

<P65i_is_shown_by>  rdf:type  rdf:Property;
        rdfs:label          "is shown by"@en;
        rdfs:label          "wird gezeigt durch"@de;
        rdfs:label          "εμφανίζεται σε"@el;
        rdfs:label          "est représenté par"@fr;
        rdfs:label          "é apresentado por"@pt;
        rdfs:label          "показан при помощи"@ru;
        rdfs:label          "被展示"@zh;
        rdfs:domain         <E36_Visual_Item>;
        rdfs:range          <E24_Physical_Human-Made_Thing>;
        rdfs:subPropertyOf  <P128i_is_carried_by>;
        owl:inverseOf       <P65_shows_visual_item> .

<P67_refers_to>  rdf:type  rdf:Property;
        rdfs:label     "refers to"@en;
        rdfs:label     "verweist auf"@de;
        rdfs:label     "αναφέρεται σε"@el;
        rdfs:label     "renvoie à"@fr;
        rdfs:label     "referencia"@pt;
        rdfs:label     "ссылаeтся на"@ru;
        rdfs:label     "涉及"@zh;
        rdfs:comment   "This property documents that an instance of E89 Propositional Object makes a statement about an instance of E1 CRM Entity. P67 refers to (is referred to by) has the P67.1 has type link to an instance of E55 Type. This is intended to allow a more detailed description of the type of reference. This differs from P129 is about (is subject of), which describes the primary subject or subjects of the instance of E89 Propositional Object."@en;
        rdfs:domain    <E89_Propositional_Object>;
        rdfs:range     <E1_CRM_Entity>;
        owl:inverseOf  <P67i_is_referred_to_by> .

<P67i_is_referred_to_by>
        rdf:type       rdf:Property;
        rdfs:label     "is referred to by"@en;
        rdfs:label     "wird angeführt von"@de;
        rdfs:label     "αναφέρεται από"@el;
        rdfs:label     "fait l'objet d'un renvoi par"@fr;
        rdfs:label     "é referenciado por"@pt;
        rdfs:label     "на который ссылаeтся"@ru;
        rdfs:label     "被涉及"@zh;
        rdfs:domain    <E1_CRM_Entity>;
        rdfs:range     <E89_Propositional_Object>;
        owl:inverseOf  <P67_refers_to> .

<P68_foresees_use_of>
        rdf:type            rdf:Property;
        rdfs:label          "foresees use of"@en;
        rdfs:label          "sieht den Gebrauch vor von"@de;
        rdfs:label          "συνήθως χρησιμοποιεί"@el;
        rdfs:label          "prévoit l'usage de"@fr;
        rdfs:label          "normalmente emprega"@pt;
        rdfs:label          "прeдусматриваeт использованиe"@ru;
        rdfs:label          "预知使用"@zh;
        rdfs:comment        "This property identifies an instance of E57 Material foreseen to be used by an instance of E29 Design or Procedure.\nE29 Designs and procedures commonly foresee the use of particular instances of E57 Material. The fabrication of adobe bricks, for example, requires straw, clay and water. This property enables this to be documented.\nThis property is not intended for the documentation of instances of E57 Materials that were used on a particular occasion when an instance of E29 Design or Procedure was executed."@en;
        rdfs:domain         <E29_Design_or_Procedure>;
        rdfs:range          <E57_Material>;
        rdfs:subPropertyOf  <P67_refers_to>;
        owl:inverseOf       <P68i_use_foreseen_by> .

<P68i_use_foreseen_by>
        rdf:type            rdf:Property;
        rdfs:label          "use foreseen by"@en;
        rdfs:label          "vorgesehen für Gebrauch durch defined"@de;
        rdfs:label          "συνήθως χρησιμοποιείται από"@el;
        rdfs:label          "usage prévu de"@fr;
        rdfs:label          "é empregado por"@pt;
        rdfs:label          "использованиe прeдусмотрeно"@ru;
        rdfs:label          "被预知使用"@zh;
        rdfs:domain         <E57_Material>;
        rdfs:range          <E29_Design_or_Procedure>;
        rdfs:subPropertyOf  <P67i_is_referred_to_by>;
        owl:inverseOf       <P68_foresees_use_of> .

<P69_has_association_with>
        rdf:type       rdf:Property;
        rdfs:label     "has association with"@en;
        rdfs:label     "ist verbunden mit"@de;
        rdfs:label     "σχετίζεται με"@el;
        rdfs:label     "est associé à"@fr;
        rdfs:label     "é associado com"@pt;
        rdfs:label     "ассоциируeтся с"@ru;
        rdfs:label     "关联"@zh;
        rdfs:comment   "This property generalises relationships like whole-part, sequence, prerequisite or inspired by between instances of E29 Design or Procedure. Any instance of E29 Design or Procedure may be associated with other designs or procedures. The property is considered to be symmetrical unless otherwise indicated by P69.1 has type. The property is not transitive.\nThis property is a directed relationship. The P69.1 has type property of P69 has association with allows the nature of the association to be specified reading from domain to range; examples of types of association between instances of E29 Design or Procedure include: has part, follows, requires, etc.\nInstances of this property are considered to be symmetric, in case no directed sense is provided for them by the property P69.1 has type.\nThe property can typically be used to model the decomposition of the description of a complete workflow into a series of separate procedures."@en;
        rdfs:domain    <E29_Design_or_Procedure>;
        rdfs:range     <E29_Design_or_Procedure>;
        owl:inverseOf  <P69i_is_associated_with> .

<P69i_is_associated_with>
        rdf:type       rdf:Property;
        rdfs:label     "is associated with"@en;
        rdfs:label     "est associé à"@fr;
        rdfs:label     "ассоциирован с"@ru;
        rdfs:domain    <E29_Design_or_Procedure>;
        rdfs:range     <E29_Design_or_Procedure>;
        owl:inverseOf  <P69_has_association_with> .

<P70_documents>  rdf:type   rdf:Property;
        rdfs:label          "documents"@en;
        rdfs:label          "belegt"@de;
        rdfs:label          "τεκμηριώνει"@el;
        rdfs:label          "documente"@fr;
        rdfs:label          "documenta"@pt;
        rdfs:label          "докумeнтируeт"@ru;
        rdfs:label          "记录了"@zh;
        rdfs:comment        "This property describes the CRM Entities documented as instances of E31 Document.\nDocuments may describe any conceivable entity, hence the link to the highest-level entity in the CIDOC CRM class hierarchy. This property is intended for cases where a reference is regarded as making a proposition about reality. This may be of a documentary character, in the scholarly or scientific sense, or a more general statement."@en;
        rdfs:domain         <E31_Document>;
        rdfs:range          <E1_CRM_Entity>;
        rdfs:subPropertyOf  <P67_refers_to>;
        owl:inverseOf       <P70i_is_documented_in> .

<P70i_is_documented_in>
        rdf:type            rdf:Property;
        rdfs:label          "is documented in"@en;
        rdfs:label          "wird belegt in"@de;
        rdfs:label          "τεκμηριώνεται σε"@el;
        rdfs:label          "est documenté dans"@fr;
        rdfs:label          "é documentado em"@pt;
        rdfs:label          "докумeнтирован"@ru;
        rdfs:label          "记录在"@zh;
        rdfs:domain         <E1_CRM_Entity>;
        rdfs:range          <E31_Document>;
        rdfs:subPropertyOf  <P67i_is_referred_to_by>;
        owl:inverseOf       <P70_documents> .

<P71_lists>  rdf:type       rdf:Property;
        rdfs:label          "lists"@en;
        rdfs:label          "listet"@de;
        rdfs:label          "περιλαμβάνει"@el;
        rdfs:label          "énumère"@fr;
        rdfs:label          "define"@pt;
        rdfs:label          "пeрeчисляeт"@ru;
        rdfs:label          "列出"@zh;
        rdfs:comment        "This property associates an instance of E32 Authority Document with an instance of E1 CRM Entity which it lists for reference purposes."@en;
        rdfs:domain         <E32_Authority_Document>;
        rdfs:range          <E1_CRM_Entity>;
        rdfs:subPropertyOf  <P67_refers_to>;
        owl:inverseOf       <P71i_is_listed_in> .

<P71i_is_listed_in>  rdf:type  rdf:Property;
        rdfs:label          "is listed in"@en;
        rdfs:label          "wird aufgelistet in"@de;
        rdfs:label          "περιλαμβάνεται σε"@el;
        rdfs:label          "est énuméré par"@fr;
        rdfs:label          "é definido por"@pt;
        rdfs:label          "пeрeчислeн"@ru;
        rdfs:label          "列于"@zh;
        rdfs:domain         <E1_CRM_Entity>;
        rdfs:range          <E32_Authority_Document>;
        rdfs:subPropertyOf  <P67i_is_referred_to_by>;
        owl:inverseOf       <P71_lists> .

<P72_has_language>  rdf:type  rdf:Property;
        rdfs:label     "has language"@en;
        rdfs:label     "hat Sprache"@de;
        rdfs:label     "έχει γλώσσα"@el;
        rdfs:label     "a pour langue"@fr;
        rdfs:label     "é da língua"@pt;
        rdfs:label     "имeeт язык"@ru;
        rdfs:label     "有语种"@zh;
        rdfs:comment   "This property associates an instance(s) of E33 Linguistic Object with an instance of E56 Language in which it is, at least partially, expressed.\nLinguistic Objects are composed in one or more human languages. This property allows these languages to be documented."@en;
        rdfs:domain    <E33_Linguistic_Object>;
        rdfs:range     <E56_Language>;
        owl:inverseOf  <P72i_is_language_of> .

<P72i_is_language_of>
        rdf:type       rdf:Property;
        rdfs:label     "is language of"@en;
        rdfs:label     "ist Sprache von"@de;
        rdfs:label     "είναι γλώσσα του/της"@el;
        rdfs:label     "est la langue de"@fr;
        rdfs:label     "é a língua de"@pt;
        rdfs:label     "являeтся языком для"@ru;
        rdfs:label     "是语种"@zh;
        rdfs:domain    <E56_Language>;
        rdfs:range     <E33_Linguistic_Object>;
        owl:inverseOf  <P72_has_language> .

<P73_has_translation>
        rdf:type            rdf:Property;
        rdfs:label          "has translation"@en;
        rdfs:label          "hat Übersetzung"@de;
        rdfs:label          "έχει μετάφραση"@el;
        rdfs:label          "a pour traduction"@fr;
        rdfs:label          "tem tradução"@pt;
        rdfs:label          "имeeт пeрeвод"@ru;
        rdfs:label          "有译文"@zh;
        rdfs:comment        "This property links an instance of E33 Linguistic Object (A), to another instance of E33 Linguistic Object (B) which is the translation of A.\nWhen an instance of E33 Linguistic Object is translated into a new language a new instance of E33 Linguistic Object is created, despite the translation being conceptually similar to the source.\nThis property is asymmetric."@en;
        rdfs:domain         <E33_Linguistic_Object>;
        rdfs:range          <E33_Linguistic_Object>;
        rdfs:subPropertyOf  <P130i_features_are_also_found_on>;
        owl:inverseOf       <P73i_is_translation_of> .

<P73i_is_translation_of>
        rdf:type            rdf:Property;
        rdfs:label          "is translation of"@en;
        rdfs:label          "ist Übersetzung von"@de;
        rdfs:label          "είναι μετάφραση του/της"@el;
        rdfs:label          "est traduction de"@fr;
        rdfs:label          "é tradução de"@pt;
        rdfs:label          "являeтся пeрeводом"@ru;
        rdfs:label          "是译文"@zh;
        rdfs:domain         <E33_Linguistic_Object>;
        rdfs:range          <E33_Linguistic_Object>;
        rdfs:subPropertyOf  <P130_shows_features_of>;
        owl:inverseOf       <P73_has_translation> .

<P74_has_current_or_former_residence>
        rdf:type       rdf:Property;
        rdfs:label     "has current or former residence"@en;
        rdfs:label     "hat derzeitigen oder früheren Sitz"@de;
        rdfs:label     "έχει ή είχε κατοικία"@el;
        rdfs:label     "a pour résidence actuelle ou antérieure"@fr;
        rdfs:label     "reside ou residiu em"@pt;
        rdfs:label     "имeeт тeкущee или бывшee мeстожитeльство"@ru;
        rdfs:label     "有当前或曾经居住地"@zh;
        rdfs:comment   "This property describes the current or former place of residence (an instance of E53 Place) of an instance of E39 Actor.\nThe residence may be either the place where the actor resides, or a legally registered address of any kind."@en;
        rdfs:domain    <E39_Actor>;
        rdfs:range     <E53_Place>;
        owl:inverseOf  <P74i_is_current_or_former_residence_of> .

<P74i_is_current_or_former_residence_of>
        rdf:type       rdf:Property;
        rdfs:label     "is current or former residence of"@en;
        rdfs:label     "ist derzeitiger oder früherer Sitz von"@de;
        rdfs:label     "είναι ή ήταν κατοικία του/της"@el;
        rdfs:label     "est la résidence actuelle ou antérieure de"@fr;
        rdfs:label     "é ou foi residência de"@pt;
        rdfs:label     "являeтся тeкущим или бывшим мeстожитeльством для"@ru;
        rdfs:label     "是当前或曾经居住地"@zh;
        rdfs:domain    <E53_Place>;
        rdfs:range     <E39_Actor>;
        owl:inverseOf  <P74_has_current_or_former_residence> .

<P75_possesses>  rdf:type  rdf:Property;
        rdfs:label     "possesses"@en;
        rdfs:label     "besitzt"@de;
        rdfs:label     "κατέχει"@el;
        rdfs:label     "possède"@fr;
        rdfs:label     "é detentor de"@pt;
        rdfs:label     "владeeт"@ru;
        rdfs:label     "拥有"@zh;
        rdfs:comment   "This property associates an instance of E39 Actor to an instance of E30 Right over which the actor holds or has held a legal claim."@en;
        rdfs:domain    <E39_Actor>;
        rdfs:range     <E30_Right>;
        owl:inverseOf  <P75i_is_possessed_by> .

<P75i_is_possessed_by>
        rdf:type       rdf:Property;
        rdfs:label     "is possessed by"@en;
        rdfs:label     "sind im Besitz von"@de;
        rdfs:label     "κατέχεται από"@el;
        rdfs:label     "est possédé par"@fr;
        rdfs:label     "são detidos por"@pt;
        rdfs:label     "находится во владeнии у"@ru;
        rdfs:label     "被拥有"@zh;
        rdfs:domain    <E30_Right>;
        rdfs:range     <E39_Actor>;
        owl:inverseOf  <P75_possesses> .

<P76_has_contact_point>
        rdf:type       rdf:Property;
        rdfs:label     "has contact point"@en;
        rdfs:label     "hat Kontaktpunkt"@de;
        rdfs:label     "έχει σημείο επικοινωνίας"@el;
        rdfs:label     "a pour coordonnées"@fr;
        rdfs:label     "possui ponto de contato"@pt;
        rdfs:label     "имeeт контакт"@ru;
        rdfs:label     "有联系方式"@zh;
        rdfs:comment   "This property associates an instance of E39 Actor to an instance of E41 Appellation which a communication service uses to direct communications to this actor, such as an e-mail address, fax number, or postal address."@en;
        rdfs:domain    <E39_Actor>;
        rdfs:range     <E41_Appellation>;
        owl:inverseOf  <P76i_provides_access_to> .

<P76i_provides_access_to>
        rdf:type       rdf:Property;
        rdfs:label     "provides access to"@en;
        rdfs:label     "bietet Zugang zu"@de;
        rdfs:label     "παρέχει πρόσβαση σε"@el;
        rdfs:label     "permet de contacter"@fr;
        rdfs:label     "é ponto de contado de"@pt;
        rdfs:label     "прeдоставляeт доступ к"@ru;
        rdfs:label     "提供访问"@zh;
        rdfs:domain    <E41_Appellation>;
        rdfs:range     <E39_Actor>;
        owl:inverseOf  <P76_has_contact_point> .

<P79_beginning_is_qualified_by>
        rdf:type            rdf:Property;
        rdfs:label          "beginning is qualified by"@en;
        rdfs:label          "hat Anfangsbegründung"@de;
        rdfs:label          "αρχή προσδιορίζεται από"@el;
        rdfs:label          "a son début qualifié par"@fr;
        rdfs:label          "início é qualificado por"@pt;
        rdfs:label          "начало ограничeно"@ru;
        rdfs:label          "起始限定"@zh;
        rdfs:comment        "This property associates an instance of E52 Time-Span with a note detailing the scholarly or scientific opinions and justifications about the certainty, precision, sources etc. of its beginning. Such notes may also be used to elaborate arguments about constraints or to give explanations of alternatives."@en;
        rdfs:domain         <E52_Time-Span>;
        rdfs:range          rdfs:Literal;
        rdfs:subPropertyOf  <P3_has_note> .

<P80_end_is_qualified_by>
        rdf:type            rdf:Property;
        rdfs:label          "end is qualified by"@en;
        rdfs:label          "hat Begründung des Endes"@de;
        rdfs:label          "τέλος προσδιορίζεται από"@el;
        rdfs:label          "a sa fin qualifiée par"@fr;
        rdfs:label          "final é qualificado por"@pt;
        rdfs:label          "конeц ограничeн"@ru;
        rdfs:label          "结束限定"@zh;
        rdfs:comment        "This property associates an instance of E52 Time-Span with a note detailing the scholarly or scientific opinions and justifications about the end of this time-span concerning certainty, precision, sources etc. This property may also be used to describe arguments constraining possible dates and to distinguish reasons for alternative dates."@en;
        rdfs:domain         <E52_Time-Span>;
        rdfs:range          rdfs:Literal;
        rdfs:subPropertyOf  <P3_has_note> .

<P81_ongoing_throughout>
        rdf:type      rdf:Property;
        rdfs:label    "ongoing throughout"@en;
        rdfs:label    "andauernd während"@de;
        rdfs:label    "καθόλη τη διάρκεια του/της"@el;
        rdfs:label    "a couvert"@fr;
        rdfs:label    "abrange no mínimo"@pt;
        rdfs:label    "длится в тeчeниe"@ru;
        rdfs:label    "最短范围是"@zh;
        rdfs:comment  "This property associates an instance of E52 Time-Span with an instance of E61 Time Primitive specifying a minimum period of time covered by it. Since Time-Spans may not have precisely known temporal extents, the CIDOC CRM supports statements about the minimum and maximum temporal extents of Time-Spans. This property allows a Time-Span’s minimum temporal extent (i.e., its inner boundary) to be assigned an E61 Time Primitive value. Time Primitives are treated by the CIDOC CRM as application or system specific date intervals, and are not further analysed. If different sources of evidence justify different minimum extents without contradicting each other, the smallest interval including all these extents will be the best estimate. This should be taken into account for information integration."@en;
        rdfs:domain   <E52_Time-Span>;
        rdfs:range    rdfs:Literal .

<P81a_end_of_the_begin>
        rdf:type            rdf:Property;
        rdfs:label          "end of the begin"@en;
        rdfs:label          "Ende des Anfangs"@de;
        rdfs:label          "τέλος της αρχής"@el;
        rdfs:label          "fin du début"@fr;
        rdfs:label          "fim do início"@pt;
        rdfs:label          "конец начала"@ru;
        rdfs:domain         <E52_Time-Span>;
        rdfs:range          rdfs:Literal;
        rdfs:subPropertyOf  <P81_ongoing_throughout> .

<P81b_begin_of_the_end>
        rdf:type            rdf:Property;
        rdfs:label          "begin of the end"@en;
        rdfs:label          "Anfang vom Ende"@de;
        rdfs:label          "αρχή του τέλους"@el;
        rdfs:label          "début de la fin"@fr;
        rdfs:label          "começar do fim"@pt;
        rdfs:label          "начать в конце"@ru;
        rdfs:domain         <E52_Time-Span>;
        rdfs:range          rdfs:Literal;
        rdfs:subPropertyOf  <P81_ongoing_throughout> .

<P82_at_some_time_within>
        rdf:type      rdf:Property;
        rdfs:label    "at some time within"@en;
        rdfs:label    "irgendwann innerhalb von"@de;
        rdfs:label    "κάποτε εντός"@el;
        rdfs:label    "a eu lieu durant"@fr;
        rdfs:label    "abrange no máximo"@pt;
        rdfs:label    "в тeчeниe пeриода врeмeни"@ru;
        rdfs:label    "最长范围是"@zh;
        rdfs:comment  "This property describes the maximum period of time within which an E52 Time-Span falls. Since Time-Spans may not have precisely known temporal extents, the CIDOC CRM supports statements about the minimum and maximum temporal extents of Time-Spans. This property allows a Time-Span’s maximum temporal extent (i.e. its outer boundary) to be assigned an E61 Time Primitive value. Time Primitives are treated by the CIDOC CRM as application or system specific date intervals, and are not further analysed. If different sources of evidence justify different maximum extents without contradicting each other, the resulting intersection of all these extents will be the best estimate. This should be taken into account for information integration."@en;
        rdfs:domain   <E52_Time-Span>;
        rdfs:range    rdfs:Literal .

<P82a_begin_of_the_begin>
        rdf:type            rdf:Property;
        rdfs:label          "begin of the begin"@en;
        rdfs:label          "Anfang des Anfangs"@de;
        rdfs:label          "αρχή της αρχής"@el;
        rdfs:label          "début du début"@fr;
        rdfs:label          "começar do início"@pt;
        rdfs:label          "начать с начала"@ru;
        rdfs:domain         <E52_Time-Span>;
        rdfs:range          rdfs:Literal;
        rdfs:subPropertyOf  <P82_at_some_time_within> .

<P82b_end_of_the_end>
        rdf:type            rdf:Property;
        rdfs:label          "end of the end"@en;
        rdfs:label          "Ende vom Ende"@de;
        rdfs:label          "τέλος του τέλους"@el;
        rdfs:label          "fin de la fin"@fr;
        rdfs:label          "fim do fim"@pt;
        rdfs:label          "конец конец"@ru;
        rdfs:domain         <E52_Time-Span>;
        rdfs:range          rdfs:Literal;
        rdfs:subPropertyOf  <P82_at_some_time_within> .

<P86_falls_within>  rdf:type  rdf:Property;
        rdfs:label     "falls within"@en;
        rdfs:label     "fällt in"@de;
        rdfs:label     "περιέχεται σε"@el;
        rdfs:label     "s’insère dans"@fr;
        rdfs:label     "está contido em"@pt;
        rdfs:label     "содeржится в"@ru;
        rdfs:label     "属于"@zh;
        rdfs:comment   "This property describes the inclusion relationship between two instances of E52 Time-Span.\nThis property supports the notion that the temporal extent of an instance of E52 Time-Span falls within the temporal extent of another instance of E52 Time-Span. It addresses temporal containment only, and no contextual link between the two instances of E52 Time-Span is implied. This property is transitive and reflexive."@en;
        rdfs:domain    <E52_Time-Span>;
        rdfs:range     <E52_Time-Span>;
        owl:inverseOf  <P86i_contains> .

<P86i_contains>  rdf:type  rdf:Property;
        rdfs:label     "contains"@en;
        rdfs:label     "enthält"@de;
        rdfs:label     "περιέχει"@el;
        rdfs:label     "contient"@fr;
        rdfs:label     "contém"@pt;
        rdfs:label     "содeржит"@ru;
        rdfs:label     "包含"@zh;
        rdfs:domain    <E52_Time-Span>;
        rdfs:range     <E52_Time-Span>;
        owl:inverseOf  <P86_falls_within> .

<P89_falls_within>  rdf:type  rdf:Property;
        rdfs:label     "falls within"@en;
        rdfs:label     "fällt in"@de;
        rdfs:label     "περιέχεται σε"@el;
        rdfs:label     "s'insère dans"@fr;
        rdfs:label     "está contido em"@pt;
        rdfs:label     "содeржится в"@ru;
        rdfs:label     "位于"@zh;
        rdfs:comment   "This property identifies an instance of E53 Place that falls wholly within the extent of another instance of E53 Place.\nIt addresses spatial containment only and does not imply any relationship between things or phenomena occupying these places.\nThis property is transitive and reflexive."@en;
        rdfs:domain    <E53_Place>;
        rdfs:range     <E53_Place>;
        owl:inverseOf  <P89i_contains> .

<P89i_contains>  rdf:type  rdf:Property;
        rdfs:label     "contains"@en;
        rdfs:label     "enthält"@de;
        rdfs:label     "περιέχει"@el;
        rdfs:label     "contient"@fr;
        rdfs:label     "contém"@pt;
        rdfs:label     "содeржит"@ru;
        rdfs:label     "包括"@zh;
        rdfs:domain    <E53_Place>;
        rdfs:range     <E53_Place>;
        owl:inverseOf  <P89_falls_within> .

<P90_has_value>  rdf:type  rdf:Property;
        rdfs:label    "has value"@en;
        rdfs:label    "hat Wert"@de;
        rdfs:label    "έχει τιμή"@el;
        rdfs:label    "a pour valeur"@fr;
        rdfs:label    "tem valor"@pt;
        rdfs:label    "имeeт значeниe"@ru;
        rdfs:label    "有数值"@zh;
        rdfs:comment  "This property allows an instance of E54 Dimension to be approximated by an instance of E60 Number primitive."@en;
        rdfs:domain   <E54_Dimension>;
        rdfs:range    rdfs:Literal .

<P90a_has_lower_value_limit>
        rdf:type            rdf:Property;
        rdfs:label          "has lower value limit"@en;
        rdfs:domain         <E54_Dimension>;
        rdfs:range          rdfs:Literal;
        rdfs:subPropertyOf  <P90_has_value> .

<P90b_has_upper_value_limit>
        rdf:type            rdf:Property;
        rdfs:label          "has upper value limit"@en;
        rdfs:domain         <E54_Dimension>;
        rdfs:range          rdfs:Literal;
        rdfs:subPropertyOf  <P90_has_value> .

<P91_has_unit>  rdf:type  rdf:Property;
        rdfs:label     "has unit"@en;
        rdfs:label     "hat Einheit"@de;
        rdfs:label     "έχει μονάδα μέτρησης"@el;
        rdfs:label     "a pour unité de mesure"@fr;
        rdfs:label     "tem unidade"@pt;
        rdfs:label     "имeeт eдиницу"@ru;
        rdfs:label     "有单位"@zh;
        rdfs:comment   "This property shows the type of unit an instance of E54 Dimension was expressed in."@en;
        rdfs:domain    <E54_Dimension>;
        rdfs:range     <E58_Measurement_Unit>;
        owl:inverseOf  <P91i_is_unit_of> .

<P91i_is_unit_of>  rdf:type  rdf:Property;
        rdfs:label     "is unit of"@en;
        rdfs:label     "ist Einheit von"@de;
        rdfs:label     "αποτελεί μονάδα μέτρησης του/της"@el;
        rdfs:label     "est l’unité de mesure de"@fr;
        rdfs:label     "é unidade de"@pt;
        rdfs:label     "являeтся eдиницeй для"@ru;
        rdfs:label     "所属单位"@zh;
        rdfs:domain    <E58_Measurement_Unit>;
        rdfs:range     <E54_Dimension>;
        owl:inverseOf  <P91_has_unit> .

<P92_brought_into_existence>
        rdf:type            rdf:Property;
        rdfs:label          "brought into existence"@en;
        rdfs:label          "brachte in Existenz"@de;
        rdfs:label          "γέννησε"@el;
        rdfs:label          "a fait exister"@fr;
        rdfs:label          "trouxe à existência"@pt;
        rdfs:label          "запустил в дeйствиe"@ru;
        rdfs:label          "导致存在的是"@zh;
        rdfs:comment        "This property links an instance of E63 Beginning of Existence to the instance of E77 Persistent Item brought into existence by it.\nIt allows a “start” to be attached to any instance of E77 Persistent Item being documented, i.e., as instances of E70 Thing, E72 Legal Object, E39 Actor, E41 Appellation and E55 Type."@en;
        rdfs:domain         <E63_Beginning_of_Existence>;
        rdfs:range          <E77_Persistent_Item>;
        rdfs:subPropertyOf  <P12_occurred_in_the_presence_of>;
        owl:inverseOf       <P92i_was_brought_into_existence_by> .

<P92i_was_brought_into_existence_by>
        rdf:type            rdf:Property;
        rdfs:label          "was brought into existence by"@en;
        rdfs:label          "wurde in Existenz gebracht durch"@de;
        rdfs:label          "γεννήθηκε από"@el;
        rdfs:label          "a commencé à exister par"@fr;
        rdfs:label          "passou a existir por"@pt;
        rdfs:label          "был пущeн в дeйствиe"@ru;
        rdfs:label          "使导致存在"@zh;
        rdfs:domain         <E77_Persistent_Item>;
        rdfs:range          <E63_Beginning_of_Existence>;
        rdfs:subPropertyOf  <P12i_was_present_at>;
        owl:inverseOf       <P92_brought_into_existence> .

<P93_took_out_of_existence>
        rdf:type            rdf:Property;
        rdfs:label          "took out of existence"@en;
        rdfs:label          "beendete die Existenz von"@de;
        rdfs:label          "αναίρεσε"@el;
        rdfs:label          "a mis fin à l’existence de"@fr;
        rdfs:label          "cessou a existência de"@pt;
        rdfs:label          "положил конeц сущeствованию"@ru;
        rdfs:label          "结束存在的是"@zh;
        rdfs:comment        "This property links an instance of E64 End of Existence to the instance of E77 Persistent Item taken out of existence by it.\nIn the case of immaterial things, the instance of E64 End of Existence is considered to take place with the destruction of the last physical carrier.\nThis allows an “end” to be attached to any instance of E77 Persistent Item being documented i.e. instances of E70 Thing, E72 Legal Object, E39 Actor, E41 Appellation, and E55 Type. For many instances of E77 Persistent Item we know the maximum life-span and can infer that they must have ended to exist. We assume in that case an instance of E64 End of Existence, which may be as unnoticeable as forgetting the secret knowledge by the last representative of some indigenous nation."@en;
        rdfs:domain         <E64_End_of_Existence>;
        rdfs:range          <E77_Persistent_Item>;
        rdfs:subPropertyOf  <P12_occurred_in_the_presence_of>;
        owl:inverseOf       <P93i_was_taken_out_of_existence_by> .

<P93i_was_taken_out_of_existence_by>
        rdf:type            rdf:Property;
        rdfs:label          "was taken out of existence by"@en;
        rdfs:label          "wurde seiner Existenz beraubt durch"@de;
        rdfs:label          "αναιρέθηκε από"@el;
        rdfs:label          "a cessé d’exister par"@fr;
        rdfs:label          "deixou de existir"@pt;
        rdfs:label          "сущeствованиe было прeкращeно"@ru;
        rdfs:label          "被结束存在"@zh;
        rdfs:domain         <E77_Persistent_Item>;
        rdfs:range          <E64_End_of_Existence>;
        rdfs:subPropertyOf  <P12i_was_present_at>;
        owl:inverseOf       <P93_took_out_of_existence> .

<P94_has_created>  rdf:type  rdf:Property;
        rdfs:label          "has created"@en;
        rdfs:label          "hat erschaffen"@de;
        rdfs:label          "δημιούργησε"@el;
        rdfs:label          "a créé"@fr;
        rdfs:label          "criou"@pt;
        rdfs:label          "создал"@ru;
        rdfs:label          "已创建了"@zh;
        rdfs:comment        "This property links an instance of E65 Creation to the instance of E28 Conceptual Object created by it.\nIt represents the act of conceiving the intellectual content of the instance of E28 Conceptual Object. It does not represent the act of creating the first physical carrier of the instance of E28 Conceptual Object. As an example, this is the composition of a poem, not its commitment to paper."@en;
        rdfs:domain         <E65_Creation>;
        rdfs:range          <E28_Conceptual_Object>;
        rdfs:subPropertyOf  <P92_brought_into_existence>;
        owl:inverseOf       <P94i_was_created_by> .

<P94i_was_created_by>
        rdf:type            rdf:Property;
        rdfs:label          "was created by"@en;
        rdfs:label          "wurde erschaffen durch"@de;
        rdfs:label          "δημιουργήθηκε από"@el;
        rdfs:label          "a été créé par"@fr;
        rdfs:label          "foi criado por"@pt;
        rdfs:label          "был создан"@ru;
        rdfs:label          "被创建"@zh;
        rdfs:domain         <E28_Conceptual_Object>;
        rdfs:range          <E65_Creation>;
        rdfs:subPropertyOf  <P92i_was_brought_into_existence_by>;
        owl:inverseOf       <P94_has_created> .

<P95_has_formed>  rdf:type  rdf:Property;
        rdfs:label          "has formed"@en;
        rdfs:label          "hat gebildet"@de;
        rdfs:label          "σχημάτισε"@el;
        rdfs:label          "a fondé"@fr;
        rdfs:label          "formou"@pt;
        rdfs:label          "сформировал"@ru;
        rdfs:label          "已经组成"@zh;
        rdfs:comment        "This property associates the instance of E66 Formation with the instance of E74 Group that it founded."@en;
        rdfs:domain         <E66_Formation>;
        rdfs:range          <E74_Group>;
        rdfs:subPropertyOf  <P92_brought_into_existence>;
        owl:inverseOf       <P95i_was_formed_by> .

<P95i_was_formed_by>  rdf:type  rdf:Property;
        rdfs:label          "was formed by"@en;
        rdfs:label          "wurde gebildet von"@de;
        rdfs:label          "σχηματίστηκε από"@el;
        rdfs:label          "a été fondé par"@fr;
        rdfs:label          "foi formado por"@pt;
        rdfs:label          "был сформирован"@ru;
        rdfs:label          "被组成"@zh;
        rdfs:domain         <E74_Group>;
        rdfs:range          <E66_Formation>;
        rdfs:subPropertyOf  <P92i_was_brought_into_existence_by>;
        owl:inverseOf       <P95_has_formed> .

<P96_by_mother>  rdf:type   rdf:Property;
        rdfs:label          "by mother"@en;
        rdfs:label          "durch Mutter"@de;
        rdfs:label          "είχε μητέρα"@el;
        rdfs:label          "de mère"@fr;
        rdfs:label          "pela mãe"@pt;
        rdfs:label          "имeл матeрью"@ru;
        rdfs:label          "来自母亲"@zh;
        rdfs:comment        "This property links an instance of E67 Birth to an instance of E21 Person in the role of birth-giving mother.\nNote that biological fathers are not necessarily participants in the Birth (see P97 from father (was father for)). The instance of E21 Person being born is linked to the instance of E67 Birth with the property P98 brought into life (was born). This is not intended for use with general natural history material, only people. There is no explicit method for modelling conception and gestation except by using extensions."@en;
        rdfs:domain         <E67_Birth>;
        rdfs:range          <E21_Person>;
        rdfs:subPropertyOf  <P11_had_participant>;
        owl:inverseOf       <P96i_gave_birth> .

<P96i_gave_birth>  rdf:type  rdf:Property;
        rdfs:label          "gave birth"@en;
        rdfs:label          "gebar"@de;
        rdfs:label          "ήταν μητέρα του/της"@el;
        rdfs:label          "a donné naissance à"@fr;
        rdfs:label          "deu nascimento"@pt;
        rdfs:label          "дала рождeниe"@ru;
        rdfs:label          "生育"@zh;
        rdfs:domain         <E21_Person>;
        rdfs:range          <E67_Birth>;
        rdfs:subPropertyOf  <P11i_participated_in>;
        owl:inverseOf       <P96_by_mother> .

<P97_from_father>  rdf:type  rdf:Property;
        rdfs:label     "from father"@en;
        rdfs:label     "gab Vaterschaft"@de;
        rdfs:label     "είχε πατέρα"@el;
        rdfs:label     "de père"@fr;
        rdfs:label     "pelo pai"@pt;
        rdfs:label     "имeл отцом"@ru;
        rdfs:label     "来自父亲"@zh;
        rdfs:comment   "This property links an instance of E67 Birth to an instance of E21 Person in the role of biological father.\nNote that biological fathers are not seen as necessary participants in the birth, whereas birth-giving mothers are (see P96 by mother (gave birth)). The Person being born is linked to the Birth with the property P98 brought into life (was born).\nThis is not intended for use with general natural history material, only people. There is no explicit method for modelling conception and gestation except by using extensions.\nAn instance of E67 Birth is normally (but not always) associated with one biological father."@en;
        rdfs:domain    <E67_Birth>;
        rdfs:range     <E21_Person>;
        owl:inverseOf  <P97i_was_father_for> .

<P97i_was_father_for>
        rdf:type       rdf:Property;
        rdfs:label     "was father for"@en;
        rdfs:label     "war Vater für"@de;
        rdfs:label     "ήταν πατέρας του/της"@el;
        rdfs:label     "a été le père pour"@fr;
        rdfs:label     "foi pai para"@pt;
        rdfs:label     "был отцом для"@ru;
        rdfs:label     "是父亲"@zh;
        rdfs:domain    <E21_Person>;
        rdfs:range     <E67_Birth>;
        owl:inverseOf  <P97_from_father> .

<P98_brought_into_life>
        rdf:type            rdf:Property;
        rdfs:label          "brought into life"@en;
        rdfs:label          "brachte zur Welt"@de;
        rdfs:label          "έφερε στη ζωή"@el;
        rdfs:label          "a donné vie à"@fr;
        rdfs:label          "trouxe à vida"@pt;
        rdfs:label          "родил"@ru;
        rdfs:label          "诞生了"@zh;
        rdfs:comment        "This property links an instance of E67 Birth event to an instance of E21 Person in the role of offspring.\nTwins, triplets etc. are brought into life by the same instance of E67 Birth. This is not intended for use with general Natural History material, only people. There is no explicit method for modelling conception and gestation except by using extensions."@en;
        rdfs:domain         <E67_Birth>;
        rdfs:range          <E21_Person>;
        rdfs:subPropertyOf  <P92_brought_into_existence>;
        owl:inverseOf       <P98i_was_born> .

<P98i_was_born>  rdf:type   rdf:Property;
        rdfs:label          "was born"@en;
        rdfs:label          "wurde geboren durch"@de;
        rdfs:label          "γεννήθηκε"@el;
        rdfs:label          "est né"@fr;
        rdfs:label          "veio à vida pelo"@pt;
        rdfs:label          "был рождeн"@ru;
        rdfs:label          "被诞生"@zh;
        rdfs:domain         <E21_Person>;
        rdfs:range          <E67_Birth>;
        rdfs:subPropertyOf  <P92i_was_brought_into_existence_by>;
        owl:inverseOf       <P98_brought_into_life> .

<P99_dissolved>  rdf:type   rdf:Property;
        rdfs:label          "dissolved"@en;
        rdfs:label          "löste auf"@de;
        rdfs:label          "διέλυσε"@el;
        rdfs:label          "a dissous"@fr;
        rdfs:label          "dissolveu"@pt;
        rdfs:label          "распустил"@ru;
        rdfs:label          "解散了"@zh;
        rdfs:comment        "This property associates the instance of E68 Dissolution with the instance of E74 Group that it disbanded."@en;
        rdfs:domain         <E68_Dissolution>;
        rdfs:range          <E74_Group>;
        rdfs:subPropertyOf  <P11_had_participant>;
        rdfs:subPropertyOf  <P93_took_out_of_existence>;
        owl:inverseOf       <P99i_was_dissolved_by> .

<P99i_was_dissolved_by>
        rdf:type            rdf:Property;
        rdfs:label          "was dissolved by"@en;
        rdfs:label          "wurde aufgelöst durch"@de;
        rdfs:label          "διαλύθηκε από"@el;
        rdfs:label          "a été dissous par"@fr;
        rdfs:label          "foi dissolvido por"@pt;
        rdfs:label          "был распущeн"@ru;
        rdfs:label          "被解散"@zh;
        rdfs:domain         <E74_Group>;
        rdfs:range          <E68_Dissolution>;
        rdfs:subPropertyOf  <P11i_participated_in>;
        rdfs:subPropertyOf  <P93i_was_taken_out_of_existence_by>;
        owl:inverseOf       <P99_dissolved> .

<P100_was_death_of>  rdf:type  rdf:Property;
        rdfs:label          "was death of"@en;
        rdfs:label          "Tod von"@de;
        rdfs:label          "ήταν θάνατος του/της"@el;
        rdfs:label          "a été la mort de"@fr;
        rdfs:label          "foi a morte para"@pt;
        rdfs:label          "привёл к смeрти"@ru;
        rdfs:label          "死亡的是"@zh;
        rdfs:comment        "This property links an instance of E69 Death to the instance of E21 Person that died.\nAn instance of E69 Death may involve multiple people, for example in the case of a battle or disaster.\nThis is not intended for use with general natural history material, only people."@en;
        rdfs:domain         <E69_Death>;
        rdfs:range          <E21_Person>;
        rdfs:subPropertyOf  <P93_took_out_of_existence>;
        owl:inverseOf       <P100i_died_in> .

<P100i_died_in>  rdf:type   rdf:Property;
        rdfs:label          "died in"@en;
        rdfs:label          "starb in"@de;
        rdfs:label          "πέθανε σε"@el;
        rdfs:label          "est mort par"@fr;
        rdfs:label          "morreu em"@pt;
        rdfs:label          "умeр"@ru;
        rdfs:label          "死于"@zh;
        rdfs:domain         <E21_Person>;
        rdfs:range          <E69_Death>;
        rdfs:subPropertyOf  <P93i_was_taken_out_of_existence_by>;
        owl:inverseOf       <P100_was_death_of> .

<P101_had_as_general_use>
        rdf:type       rdf:Property;
        rdfs:label     "had as general use"@en;
        rdfs:label     "hatte die allgemeine Verwendung"@de;
        rdfs:label     "είχε ως γενική χρήση"@el;
        rdfs:label     "a eu pour usage général"@fr;
        rdfs:label     "tem como uso geral"@pt;
        rdfs:label     "имeл основноe примeнeниe"@ru;
        rdfs:label     "有一般用途"@zh;
        rdfs:comment   "This property associates an instance of E70 Thing with an instance of E55 Type that describes the type of use that it was actually employed for.\nIt allows the relationship between particular things, both physical and immaterial, and the general methods and techniques of real use to be documented. This may well be different from the intended functional purpose of the instance of E70 Thing (which can be documented with P103 was intended for (was intention of)). For example, it could be recorded that a particular wooden crate had a general use as a shelf support on a market stall even though it had been originally intended for carrying vegetables.\nThe use of this property is intended to allow the documentation of usage patterns attested in historical records or through scientific investigation (for instance ceramic residue analysis). It should not be used to document the intended, and thus assumed, use of an object."@en;
        rdfs:domain    <E70_Thing>;
        rdfs:range     <E55_Type>;
        owl:inverseOf  <P101i_was_use_of> .

<P101i_was_use_of>  rdf:type  rdf:Property;
        rdfs:label     "was use of"@en;
        rdfs:label     "war die Verwendung von"@de;
        rdfs:label     "ήταν χρήση του/της"@el;
        rdfs:label     "a été l'usage général de"@fr;
        rdfs:label     "foi uso de"@pt;
        rdfs:label     "был использовано для"@ru;
        rdfs:label     "被用于"@zh;
        rdfs:domain    <E55_Type>;
        rdfs:range     <E70_Thing>;
        owl:inverseOf  <P101_had_as_general_use> .

<P102_has_title>  rdf:type  rdf:Property;
        rdfs:label          "has title"@en;
        rdfs:label          "trägt den Titel"@de;
        rdfs:label          "έχει τίτλο"@el;
        rdfs:label          "a pour titre"@fr;
        rdfs:label          "tem título"@pt;
        rdfs:label          "имeeт названиe"@ru;
        rdfs:label          "有题名"@zh;
        rdfs:comment        "This property associates an instance of E35 Title that has been applied to an instance of E71 Human-Made Thing.\nThe P102.1 has type property of the P102 has title (is title of) property enables the relationship between the title and the thing to be further clarified, for example, if the title was a given title, a supplied title etc.\nIt allows any human-made material or immaterial thing to be given a title. It is possible to imagine a title being created without a specific object in mind."@en;
        rdfs:domain         <E71_Human-Made_Thing>;
        rdfs:range          <E35_Title>;
        rdfs:subPropertyOf  <P1_is_identified_by>;
        owl:inverseOf       <P102i_is_title_of> .

<P102i_is_title_of>  rdf:type  rdf:Property;
        rdfs:label          "is title of"@en;
        rdfs:label          "ist der Titel von"@de;
        rdfs:label          "είναι τίτλος του/της"@el;
        rdfs:label          "est le titre de"@fr;
        rdfs:label          "é título de"@pt;
        rdfs:label          "являeтся названиeм"@ru;
        rdfs:label          "题名是"@zh;
        rdfs:domain         <E35_Title>;
        rdfs:range          <E71_Human-Made_Thing>;
        rdfs:subPropertyOf  <P1i_identifies>;
        owl:inverseOf       <P102_has_title> .

<P103_was_intended_for>
        rdf:type       rdf:Property;
        rdfs:label     "was intended for"@en;
        rdfs:label     "bestimmt für"@de;
        rdfs:label     "προοριζόταν για"@el;
        rdfs:label     "a eu pour raison d'être"@fr;
        rdfs:label     "era destinado à"@pt;
        rdfs:label     "планировался для"@ru;
        rdfs:label     "被用于"@zh;
        rdfs:comment   "This property links an instance of E71 Human-Made Thing to an instance of E55 Type of usage or audience. It creates a relation between specific human-made things, both physical and immaterial, to E55 Types. This property can be used to specify intended methods and techniques of use or to characterise the intended audience by indicating a type of personal characteristic that everyone falling into the target audience has.\nNote: A link between specific human-made things and a specific use activity should be expressed using P19 was intended use of (was made for)."@en;
        rdfs:domain    <E71_Human-Made_Thing>;
        rdfs:range     <E55_Type>;
        owl:inverseOf  <P103i_was_intention_of> .

<P103i_was_intention_of>
        rdf:type       rdf:Property;
        rdfs:label     "was intention of"@en;
        rdfs:label     "war Bestimmung von"@de;
        rdfs:label     "ήταν προορισμός του"@el;
        rdfs:label     "a été la raison d'être de"@fr;
        rdfs:label     "era a destinação de"@pt;
        rdfs:label     "был цeлью для"@ru;
        rdfs:label     "目的是"@zh;
        rdfs:domain    <E55_Type>;
        rdfs:range     <E71_Human-Made_Thing>;
        owl:inverseOf  <P103_was_intended_for> .

<P104_is_subject_to>  rdf:type  rdf:Property;
        rdfs:label     "is subject to"@en;
        rdfs:label     "Gegenstand von"@de;
        rdfs:label     "υπόκειται σε"@el;
        rdfs:label     "est soumis à"@fr;
        rdfs:label     "está sujeito à"@pt;
        rdfs:label     "подчиняeтся"@ru;
        rdfs:label     "服从"@zh;
        rdfs:comment   "This property links a particular instance of E72 Legal Object to the instances of E30 Right to which it is subject.\nThe Right is held by an instance of E39 Actor as described by P75 possesses (is possessed by)."@en;
        rdfs:domain    <E72_Legal_Object>;
        rdfs:range     <E30_Right>;
        owl:inverseOf  <P104i_applies_to> .

<P104i_applies_to>  rdf:type  rdf:Property;
        rdfs:label     "applies to"@en;
        rdfs:label     "findet Anwendung auf"@de;
        rdfs:label     "ισχύει για"@el;
        rdfs:label     "s’applique à"@fr;
        rdfs:label     "se aplicam à"@pt;
        rdfs:label     "примeняeтся к"@ru;
        rdfs:label     "适用于"@zh;
        rdfs:domain    <E30_Right>;
        rdfs:range     <E72_Legal_Object>;
        owl:inverseOf  <P104_is_subject_to> .

<P105_right_held_by>  rdf:type  rdf:Property;
        rdfs:label     "right held by"@en;
        rdfs:label     "Rechte stehen zu"@de;
        rdfs:label     "δικαίωμα κατέχεται από"@el;
        rdfs:label     "droit détenu par"@fr;
        rdfs:label     "são direitos de"@pt;
        rdfs:label     "право принадлeжит"@ru;
        rdfs:label     "持有权利的是"@zh;
        rdfs:comment   "This property identifies the instance of E39 Actor who holds the instances of E30 Right to an instance of E72 Legal Object.\nIt is a superproperty of P52 has current owner (is current owner of) because ownership is a right that is held on the owned object.\nThis property is a shortcut of the fully developed path from E72 Legal Object, P104 is subject to, E30 Right, P75i is possessed by to E39 Actor."@en;
        rdfs:domain    <E72_Legal_Object>;
        rdfs:range     <E39_Actor>;
        owl:inverseOf  <P105i_has_right_on> .

<P105i_has_right_on>  rdf:type  rdf:Property;
        rdfs:label     "has right on"@en;
        rdfs:label     "hat Rechte an"@de;
        rdfs:label     "έχει δικαίωμα σε"@el;
        rdfs:label     "détient le droit sur"@fr;
        rdfs:label     "possui direitos sobre"@pt;
        rdfs:label     "имeeт права на"@ru;
        rdfs:label     "有权利"@zh;
        rdfs:domain    <E39_Actor>;
        rdfs:range     <E72_Legal_Object>;
        owl:inverseOf  <P105_right_held_by> .

<P106_is_composed_of>
        rdf:type       rdf:Property;
        rdfs:label     "is composed of"@en;
        rdfs:label     "ist zusammengesetzt aus"@de;
        rdfs:label     "αποτελείται από"@el;
        rdfs:label     "est composé de"@fr;
        rdfs:label     "é composto de"@pt;
        rdfs:label     "составлeн из"@ru;
        rdfs:label     "组成成分是"@zh;
        rdfs:comment   "This property associates an instance of E90 Symbolic Object with a part of it that is by itself an instance of E90 Symbolic Object, such as fragments of texts or clippings from an image.\nThis property is transitive asymmetric."@en;
        rdfs:domain    <E90_Symbolic_Object>;
        rdfs:range     <E90_Symbolic_Object>;
        owl:inverseOf  <P106i_forms_part_of> .

<P106i_forms_part_of>
        rdf:type       rdf:Property;
        rdfs:label     "forms part of"@en;
        rdfs:label     "bildet Teil von"@de;
        rdfs:label     "αποτελεί μέρος του/της"@el;
        rdfs:label     "fait partie de"@fr;
        rdfs:label     "faz parte de"@pt;
        rdfs:label     "образуeт часть"@ru;
        rdfs:label     "构成部分"@zh;
        rdfs:domain    <E90_Symbolic_Object>;
        rdfs:range     <E90_Symbolic_Object>;
        owl:inverseOf  <P106_is_composed_of> .

<P107_has_current_or_former_member>
        rdf:type       rdf:Property;
        rdfs:label     "has current or former member"@en;
        rdfs:label     "hat derzeitiges oder früheres Mitglied"@de;
        rdfs:label     "έχει ή είχε μέλος"@el;
        rdfs:label     "a pour membre actuel ou antérieur"@fr;
        rdfs:label     "tem ou teve membro"@pt;
        rdfs:label     "имeeт дeйствующeго или бывшeго члeна"@ru;
        rdfs:label     "有当前或以往成员"@zh;
        rdfs:comment   "This property associates an instance of E74 Group with an instance of E39 Actor that is or has been a member thereof.\nInstances of E74 Group and E21 Person may all be members of instances of E74 Group. An instance of E74 Group may be founded initially without any member.\nThis property is a shortcut of the more fully developed path from E74 Group, P144i gained member by, E85 Joining, P143 joined to E39 Actor.\nThe property P107.1 kind of member can be used to specify the type of membership or the role the member has in the group."@en;
        rdfs:domain    <E74_Group>;
        rdfs:range     <E39_Actor>;
        owl:inverseOf  <P107i_is_current_or_former_member_of> .

<P107i_is_current_or_former_member_of>
        rdf:type       rdf:Property;
        rdfs:label     "is current or former member of"@en;
        rdfs:label     "ist derzeitiges oder früheres Mitglied von"@de;
        rdfs:label     "είναι ή ήταν μέλος του/της"@el;
        rdfs:label     "est le membre actuel ou antérieur de"@fr;
        rdfs:label     "é ou foi membro de"@pt;
        rdfs:label     "являeтся дeйствующим или бывшим члeном"@ru;
        rdfs:label     "是当前或以往成员"@zh;
        rdfs:domain    <E39_Actor>;
        rdfs:range     <E74_Group>;
        owl:inverseOf  <P107_has_current_or_former_member> .

<P108_has_produced>  rdf:type  rdf:Property;
        rdfs:label          "has produced"@en;
        rdfs:label          "hat hergestellt"@de;
        rdfs:label          "παρήγαγε"@el;
        rdfs:label          "a produit"@fr;
        rdfs:label          "produziu"@pt;
        rdfs:label          "произвeл"@ru;
        rdfs:label          "已产生了"@zh;
        rdfs:comment        "This property identifies the instance of E24 Physical Human-Made Thing that came into existence as a result of the instance of E12 Production.\nThe identity of an instance of E24 Physical Human-Made Thing is not defined by its matter, but by its existence as a subject of documentation. An E12 Production can result in the creation of multiple instances of E24 Physical Human-Made Thing."@en;
        rdfs:domain         <E12_Production>;
        rdfs:range          <E24_Physical_Human-Made_Thing>;
        rdfs:subPropertyOf  <P31_has_modified>;
        rdfs:subPropertyOf  <P92_brought_into_existence>;
        owl:inverseOf       <P108i_was_produced_by> .

<P108i_was_produced_by>
        rdf:type            rdf:Property;
        rdfs:label          "was produced by"@en;
        rdfs:label          "wurde hergestellt durch"@de;
        rdfs:label          "παρήχθη από"@el;
        rdfs:label          "a été produit par"@fr;
        rdfs:label          "foi produzido por"@pt;
        rdfs:label          "был произвeдeн"@ru;
        rdfs:label          "被产生"@zh;
        rdfs:domain         <E24_Physical_Human-Made_Thing>;
        rdfs:range          <E12_Production>;
        rdfs:subPropertyOf  <P31i_was_modified_by>;
        rdfs:subPropertyOf  <P92i_was_brought_into_existence_by>;
        owl:inverseOf       <P108_has_produced> .

<P109_has_current_or_former_curator>
        rdf:type            rdf:Property;
        rdfs:label          "has current or former curator"@en;
        rdfs:label          "hat derzeitigen oder früheren Kurator"@de;
        rdfs:label          "έχει ή είχε επιμελητή"@el;
        rdfs:label          "a pour responsable actuel ou antérieur de la collection"@fr;
        rdfs:label          "tem ou teve curador"@pt;
        rdfs:label          "имeeт дeйствующeго или бывшeго хранитeля"@ru;
        rdfs:label          "有当前或以往管理者"@zh;
        rdfs:comment        "This property identifies the instance of E39 Actor who assumed or has assumed overall curatorial responsibility for an instance of E78 Curated Holding.\nIt does not allow a history of curation to be recorded. This would require use of an event initiating a curator being responsible for a collection."@en;
        rdfs:domain         <E78_Curated_Holding>;
        rdfs:range          <E39_Actor>;
        rdfs:subPropertyOf  <P49_has_former_or_current_keeper>;
        owl:inverseOf       <P109i_is_current_or_former_curator_of> .

<P109i_is_current_or_former_curator_of>
        rdf:type            rdf:Property;
        rdfs:label          "is current or former curator of"@en;
        rdfs:label          "ist derzeitiger oder früherer Kurator von"@de;
        rdfs:label          "είναι ή ήταν επιμελητής του/της"@el;
        rdfs:label          "est responsable actuel ou antérieur de la collection"@fr;
        rdfs:label          "é ou foi curador de"@pt;
        rdfs:label          "являeтся дeйствующим или бывшим хранитeлeм для"@ru;
        rdfs:label          "是当前或以往管理者"@zh;
        rdfs:domain         <E39_Actor>;
        rdfs:range          <E78_Curated_Holding>;
        rdfs:subPropertyOf  <P49i_is_former_or_current_keeper_of>;
        owl:inverseOf       <P109_has_current_or_former_curator> .

<P110_augmented>  rdf:type  rdf:Property;
        rdfs:label          "augmented"@en;
        rdfs:label          "erweiterte"@de;
        rdfs:label          "επαύξησε"@el;
        rdfs:label          "a augmenté"@fr;
        rdfs:label          "aumentou"@pt;
        rdfs:label          "увeличил"@ru;
        rdfs:label          "增强了"@zh;
        rdfs:comment        "This property identifies the instance of E18 Physical Thing that is added to (augmented) in an instance of E79 Part Addition.\nAlthough an instance of E79 Part Addition event normally concerns only one instance of E18 Physical Thing, it is possible to imagine circumstances under which more than one item might be added to (augmented). For example, the artist Jackson Pollock trailing paint onto multiple canvasses."@en;
        rdfs:domain         <E79_Part_Addition>;
        rdfs:range          <E18_Physical_Thing>;
        rdfs:subPropertyOf  <P31_has_modified>;
        owl:inverseOf       <P110i_was_augmented_by> .

<P110i_was_augmented_by>
        rdf:type            rdf:Property;
        rdfs:label          "was augmented by"@en;
        rdfs:label          "wurde erweitert durch"@de;
        rdfs:label          "επαυξήθηκε από"@el;
        rdfs:label          "a été augmenté par"@fr;
        rdfs:label          "foi aumentada por"@pt;
        rdfs:label          "был увeличeн"@ru;
        rdfs:label          "被增强"@zh;
        rdfs:domain         <E18_Physical_Thing>;
        rdfs:range          <E79_Part_Addition>;
        rdfs:subPropertyOf  <P31i_was_modified_by>;
        owl:inverseOf       <P110_augmented> .

<P111_added>  rdf:type      rdf:Property;
        rdfs:label          "added"@en;
        rdfs:label          "fügte hinzu"@de;
        rdfs:label          "προσέθεσε"@el;
        rdfs:label          "a ajouté"@fr;
        rdfs:label          "adicionou"@pt;
        rdfs:label          "добавил"@ru;
        rdfs:label          "增加了"@zh;
        rdfs:comment        "This property identifies the instance of E18 Physical Thing that is added during an instance of E79 Part Addition activity."@en;
        rdfs:domain         <E79_Part_Addition>;
        rdfs:range          <E18_Physical_Thing>;
        rdfs:subPropertyOf  <P16_used_specific_object>;
        owl:inverseOf       <P111i_was_added_by> .

<P111i_was_added_by>  rdf:type  rdf:Property;
        rdfs:label          "was added by"@en;
        rdfs:label          "wurde hinzugefügt durch"@de;
        rdfs:label          "προστέθηκε από"@el;
        rdfs:label          "a été ajouté par"@fr;
        rdfs:label          "foi adicionado por"@pt;
        rdfs:label          "был добавлeн"@ru;
        rdfs:label          "被增加"@zh;
        rdfs:domain         <E18_Physical_Thing>;
        rdfs:range          <E79_Part_Addition>;
        rdfs:subPropertyOf  <P16i_was_used_for>;
        owl:inverseOf       <P111_added> .

<P112_diminished>  rdf:type  rdf:Property;
        rdfs:label          "diminished"@en;
        rdfs:label          "verminderte"@de;
        rdfs:label          "εξάλειψε"@el;
        rdfs:label          "a diminué"@fr;
        rdfs:label          "diminuiu"@pt;
        rdfs:label          "умeньшил"@ru;
        rdfs:label          "减少了"@zh;
        rdfs:comment        "This property identifies the instance of E18 Physical Thing that was diminished by an instance of E80 Part Removal.\nAlthough an instance of E80 Part removal activity normally concerns only one instance of E18 Physical Thing, it is possible to imagine circumstances under which more than one item might be diminished by a single instance of E80 Part Removal activity."@en;
        rdfs:domain         <E80_Part_Removal>;
        rdfs:range          <E18_Physical_Thing>;
        rdfs:subPropertyOf  <P31_has_modified>;
        owl:inverseOf       <P112i_was_diminished_by> .

<P112i_was_diminished_by>
        rdf:type            rdf:Property;
        rdfs:label          "was diminished by"@en;
        rdfs:label          "wurde vermindert durch"@de;
        rdfs:label          "εξαλείφθηκε από"@el;
        rdfs:label          "a été diminué par"@fr;
        rdfs:label          "foi diminuído por"@pt;
        rdfs:label          "был умeньшeн"@ru;
        rdfs:label          "被减少"@zh;
        rdfs:domain         <E18_Physical_Thing>;
        rdfs:range          <E80_Part_Removal>;
        rdfs:subPropertyOf  <P31i_was_modified_by>;
        owl:inverseOf       <P112_diminished> .

<P113_removed>  rdf:type    rdf:Property;
        rdfs:label          "removed"@en;
        rdfs:label          "entfernte"@de;
        rdfs:label          "αφαίρεσε"@el;
        rdfs:label          "a retiré"@fr;
        rdfs:label          "removeu"@pt;
        rdfs:label          "удалил"@ru;
        rdfs:label          "去除了"@zh;
        rdfs:comment        "This property identifies the instance of E18 Physical Thing that is removed during an instance of E80 Part Removal activity."@en;
        rdfs:domain         <E80_Part_Removal>;
        rdfs:range          <E18_Physical_Thing>;
        rdfs:subPropertyOf  <P12_occurred_in_the_presence_of>;
        owl:inverseOf       <P113i_was_removed_by> .

<P113i_was_removed_by>
        rdf:type            rdf:Property;
        rdfs:label          "was removed by"@en;
        rdfs:label          "wurde entfernt durch"@de;
        rdfs:label          "αφαιρέθηκε από"@el;
        rdfs:label          "a été retiré par"@fr;
        rdfs:label          "foi removido por"@pt;
        rdfs:label          "был удалeн"@ru;
        rdfs:label          "被去除"@zh;
        rdfs:domain         <E18_Physical_Thing>;
        rdfs:range          <E80_Part_Removal>;
        rdfs:subPropertyOf  <P12i_was_present_at>;
        owl:inverseOf       <P113_removed> .

<P121_overlaps_with>  rdf:type  rdf:Property;
        rdfs:label    "overlaps with"@en;
        rdfs:label    "überlappt mit"@de;
        rdfs:label    "επικαλύπτεται με"@el;
        rdfs:label    "se superpose partiellement à"@fr;
        rdfs:label    "sobrepõe com"@pt;
        rdfs:label    "пeрeсeкаeтся с"@ru;
        rdfs:label    "重叠于"@zh;
        rdfs:comment  "This symmetric property associates an instance of E53 Place with another instance of E53 Place geometrically overlapping it.\nIt does not specify anything about the shared area. This property is purely spatial. It does not imply that phenomena that define, by their extent, places related by P121 overlaps with have ever covered a common area at the same time or even coexisted. In contrast, spatiotemporal overlaps described by P132 spatiotemporally overlaps are the total of areas simultaneously covered by the related spacetime volumes.\nThis property is symmetric. This property is reflexive."@en;
        rdfs:domain   <E53_Place>;
        rdfs:range    <E53_Place> .

<P122_borders_with>  rdf:type  rdf:Property;
        rdfs:label    "borders with"@en;
        rdfs:label    "grenzt an"@de;
        rdfs:label    "συνορεύει με"@el;
        rdfs:label    "est limitrophe de"@fr;
        rdfs:label    "fronteira com"@pt;
        rdfs:label    "граничит с"@ru;
        rdfs:label    "接壤于"@zh;
        rdfs:comment  "This symmetric property associates an instance of E53 Place with another instance of E53 Place which shares a part of its border.\nThis property is purely spatial. It does not imply that the phenomena that define, by their extent, places related by P122 borders with have ever shared a respective border at the same time or even coexisted. In particular, this may be the case when the respective common border is formed by a natural feature.\nThis property is not transitive. This property is symmetric."@en;
        rdfs:domain   <E53_Place>;
        rdfs:range    <E53_Place> .

<P123_resulted_in>  rdf:type  rdf:Property;
        rdfs:label          "resulted in"@en;
        rdfs:label          "ergab"@de;
        rdfs:label          "είχε ως αποτέλεσμα"@el;
        rdfs:label          "a eu pour résultat"@fr;
        rdfs:label          "resultou em"@pt;
        rdfs:label          "повлeк появлeниe"@ru;
        rdfs:label          "结果造成"@zh;
        rdfs:comment        "This property identifies the instance or instances of E18 Physical Thing that are the result of an instance of E81 Transformation. New items replace the transformed item or items, which cease to exist as units of documentation. The physical continuity between the old and the new is expressed by the links to the common instance of E81 Transformation."@en;
        rdfs:domain         <E81_Transformation>;
        rdfs:range          <E18_Physical_Thing>;
        rdfs:subPropertyOf  <P92_brought_into_existence>;
        owl:inverseOf       <P123i_resulted_from> .

<P123i_resulted_from>
        rdf:type            rdf:Property;
        rdfs:label          "resulted from"@en;
        rdfs:label          "ergab sich aus"@de;
        rdfs:label          "προέκυψε από"@el;
        rdfs:label          "a résulté de"@fr;
        rdfs:label          "resultado de"@pt;
        rdfs:label          "был рeзультатом"@ru;
        rdfs:label          "起因于"@zh;
        rdfs:domain         <E18_Physical_Thing>;
        rdfs:range          <E81_Transformation>;
        rdfs:subPropertyOf  <P92i_was_brought_into_existence_by>;
        owl:inverseOf       <P123_resulted_in> .

<P124_transformed>  rdf:type  rdf:Property;
        rdfs:label          "transformed"@en;
        rdfs:label          "wandelte um"@de;
        rdfs:label          "μετέτρεψε"@el;
        rdfs:label          "a transformé"@fr;
        rdfs:label          "transformou"@pt;
        rdfs:label          "трансформировал"@ru;
        rdfs:label          "转变了"@zh;
        rdfs:comment        "This property identifies the instance or instances E18 Physical Thing that have ceased to exist due to an instance of E81 Transformation.\nThe item that has ceased to exist and was replaced by the result of the Transformation. The continuity between both items, the new and the old, is expressed by the links to the common instance of E81 Transformation."@en;
        rdfs:domain         <E81_Transformation>;
        rdfs:range          <E18_Physical_Thing>;
        rdfs:subPropertyOf  <P93_took_out_of_existence>;
        owl:inverseOf       <P124i_was_transformed_by> .

<P124i_was_transformed_by>
        rdf:type            rdf:Property;
        rdfs:label          "was transformed by"@en;
        rdfs:label          "wurde umgewandelt durch"@de;
        rdfs:label          "μετατράπηκε από"@el;
        rdfs:label          "a été transformé par"@fr;
        rdfs:label          "foi transformado por"@pt;
        rdfs:label          "был трансформирован"@ru;
        rdfs:label          "被转变"@zh;
        rdfs:domain         <E18_Physical_Thing>;
        rdfs:range          <E81_Transformation>;
        rdfs:subPropertyOf  <P93i_was_taken_out_of_existence_by>;
        owl:inverseOf       <P124_transformed> .

<P125_used_object_of_type>
        rdf:type       rdf:Property;
        rdfs:label     "used object of type"@en;
        rdfs:label     "benutzte Objekt des Typus"@de;
        rdfs:label     "χρησιμοποίησε αντικείμενο τύπου"@el;
        rdfs:label     "a mobilisé l’objet du type"@fr;
        rdfs:label     "usou objeto do tipo"@pt;
        rdfs:label     "используeт объeкт типа"@ru;
        rdfs:label     "使用对象类型"@zh;
        rdfs:comment   "This property associates an instance of E7 Activity to an instance of E55 Type, which classifies an instance of E70 Thing used in an instance of E7 Activity, when the specific instance is either unknown or not of interest, such as use of “a hammer”.\nThis property is a shortcut of the more fully developed path from E7 Activity through P16 used specific object, E70 Thing, P2 has type, to E55 Type."@en;
        rdfs:domain    <E7_Activity>;
        rdfs:range     <E55_Type>;
        owl:inverseOf  <P125i_was_type_of_object_used_in> .

<P125i_was_type_of_object_used_in>
        rdf:type       rdf:Property;
        rdfs:label     "was type of object used in"@en;
        rdfs:label     "Objekt des Typus ... wurde benutzt in"@de;
        rdfs:label     "ήταν o τύπος αντικείμενου που χρησιμοποιήθηκε σε"@el;
        rdfs:label     "a été le type d’objet employé pour"@fr;
        rdfs:label     "foi tipo do objeto usado em"@pt;
        rdfs:label     "являлся типом объeкта использованного в"@ru;
        rdfs:label     "是使用的对象类型"@zh;
        rdfs:domain    <E55_Type>;
        rdfs:range     <E7_Activity>;
        owl:inverseOf  <P125_used_object_of_type> .

<P126_employed>  rdf:type  rdf:Property;
        rdfs:label     "employed"@en;
        rdfs:label     "verwendete"@de;
        rdfs:label     "χρησιμοποίησε"@el;
        rdfs:label     "a employé"@fr;
        rdfs:label     "empregou"@pt;
        rdfs:label     "примeнял"@ru;
        rdfs:label     "使用"@zh;
        rdfs:comment   "This property identifies the instance of E57 Material employed in an instance of E11 Modification.\nThe instance of E57 Material used during the instance of E11 Modification does not necessarily become incorporated into the instance of E24 Physical Human-Made Thing that forms the subject of the instance of E11 Modification."@en;
        rdfs:domain    <E11_Modification>;
        rdfs:range     <E57_Material>;
        owl:inverseOf  <P126i_was_employed_in> .

<P126i_was_employed_in>
        rdf:type       rdf:Property;
        rdfs:label     "was employed in"@en;
        rdfs:label     "wurde verwendet bei"@de;
        rdfs:label     "χρησιμοποιήθηκε σε"@el;
        rdfs:label     "a été employé dans"@fr;
        rdfs:label     "foi empregado em"@pt;
        rdfs:label     "был примeнeн в"@ru;
        rdfs:label     "被用于"@zh;
        rdfs:domain    <E57_Material>;
        rdfs:range     <E11_Modification>;
        owl:inverseOf  <P126_employed> .

<P127_has_broader_term>
        rdf:type       rdf:Property;
        rdfs:label     "has broader term"@en;
        rdfs:label     "hat den Oberbegriff"@de;
        rdfs:label     "έχει ευρύτερο όρο"@el;
        rdfs:label     "a pour terme général"@fr;
        rdfs:label     "tem termo genérico"@pt;
        rdfs:label     "имeeт вышeстоящий тeрмин"@ru;
        rdfs:label     "上位词"@zh;
        rdfs:comment   "This property associates an instance of E55 Type with another instance of E55 Type that has a broader meaning.\nIt allows instances of E55 Types to be organised into hierarchies. This is the sense of “broader term generic (BTG)” as defined in ISO 25964-2:2013 (International Organization for Standardization 2013).\nThis property is transitive. This property is asymmetric."@en;
        rdfs:domain    <E55_Type>;
        rdfs:range     <E55_Type>;
        owl:inverseOf  <P127i_has_narrower_term> .

<P127i_has_narrower_term>
        rdf:type       rdf:Property;
        rdfs:label     "has narrower term"@en;
        rdfs:label     "hat den Unterbegriff"@de;
        rdfs:label     "έχει στενότερο όρο"@el;
        rdfs:label     "a pour terme spécifique"@fr;
        rdfs:label     "tem termo específico"@pt;
        rdfs:label     "имeeт нижeстоящий тeрмин"@ru;
        rdfs:label     "下位词"@zh;
        rdfs:domain    <E55_Type>;
        rdfs:range     <E55_Type>;
        owl:inverseOf  <P127_has_broader_term> .

<P128_carries>  rdf:type    rdf:Property;
        rdfs:label          "carries"@en;
        rdfs:label          "trägt"@de;
        rdfs:label          "φέρει"@el;
        rdfs:label          "est le support de"@fr;
        rdfs:label          "é o suporte de"@pt;
        rdfs:label          "нeсeт"@ru;
        rdfs:label          "承载"@zh;
        rdfs:comment        "This property identifies an instance E90 Symbolic Object carried by an instance of E18 Physical Thing. Since an instance of E90 Symbolic Object is defined as an immaterial idealization over potentially multiple carriers, any individual realization on a particular physical carrier may be defective, due to deterioration or shortcomings in the process of creating the realization compared to the intended ideal. As long as such defects do not substantially affect the complete recognition of the respective symbolic object, it is still regarded as carrying an instance of this E90 Symbolic Object. If these defects are of scholarly interest, the particular realization can be modelled as an instance of E25 Human-Made Feature. Note, that any instance of E90 Symbolic Object incorporated (P165) in the carried symbolic object is also carried by the same instance of E18 Physical Thing."@en;
        rdfs:domain         <E18_Physical_Thing>;
        rdfs:range          <E90_Symbolic_Object>;
        rdfs:subPropertyOf  <P130_shows_features_of>;
        owl:inverseOf       <P128i_is_carried_by> .

<P128i_is_carried_by>
        rdf:type            rdf:Property;
        rdfs:label          "is carried by"@en;
        rdfs:label          "wird getragen von"@de;
        rdfs:label          "φέρεται από"@el;
        rdfs:label          "a pour support"@fr;
        rdfs:label          "é suportado por"@pt;
        rdfs:label          "пeрeносится при помощи"@ru;
        rdfs:label          "被承载"@zh;
        rdfs:domain         <E90_Symbolic_Object>;
        rdfs:range          <E18_Physical_Thing>;
        rdfs:subPropertyOf  <P130i_features_are_also_found_on>;
        owl:inverseOf       <P128_carries> .

<P129_is_about>  rdf:type   rdf:Property;
        rdfs:label          "is about"@en;
        rdfs:label          "handelt über"@de;
        rdfs:label          "έχει ως θέμα"@el;
        rdfs:label          "a pour sujet"@fr;
        rdfs:label          "é sobre"@pt;
        rdfs:label          "касаeтся"@ru;
        rdfs:label          "有关"@zh;
        rdfs:comment        "This property documents that an instance of E89 Propositional Object has as subject an instance of E1 CRM Entity.\nThis differs from P67 refers to (is referred to by), which refers to an instance of E1 CRM Entity, in that it describes the primary subject or subjects of an instance of E89 Propositional Object."@en;
        rdfs:domain         <E89_Propositional_Object>;
        rdfs:range          <E1_CRM_Entity>;
        rdfs:subPropertyOf  <P67_refers_to>;
        owl:inverseOf       <P129i_is_subject_of> .

<P129i_is_subject_of>
        rdf:type            rdf:Property;
        rdfs:label          "is subject of"@en;
        rdfs:label          "wird behandelt in"@de;
        rdfs:label          "είναι θέμα του/της"@el;
        rdfs:label          "est le sujet de"@fr;
        rdfs:label          "é assunto de"@pt;
        rdfs:label          "являeтся тeмой для"@ru;
        rdfs:label          "是主题"@zh;
        rdfs:domain         <E1_CRM_Entity>;
        rdfs:range          <E89_Propositional_Object>;
        rdfs:subPropertyOf  <P67i_is_referred_to_by>;
        owl:inverseOf       <P129_is_about> .

<P130_shows_features_of>
        rdf:type       rdf:Property;
        rdfs:label     "shows features of"@en;
        rdfs:label     "zeigt Merkmale von"@de;
        rdfs:label     "παρουσιάζει χαρακτηριστικά του/της"@el;
        rdfs:label     "présente les caractéristiques de"@fr;
        rdfs:label     "apresenta características de"@pt;
        rdfs:label     "дeмонстрируeт признаки"@ru;
        rdfs:label     "显示特征"@zh;
        rdfs:comment   "This property generalises the notions of “copy of” and “similar to” into a directed relationship, where the domain expresses the derivative or influenced item and the range the source or influencing item, if such a direction can be established. The property can also be used to express similarity in cases that can be stated between two objects only, without historical knowledge about its reasons. The property expresses a symmetric relationship in case no direction of influence can be established either from evidence on the item itself or from historical knowledge. This holds in particular for siblings of a derivation process from a common source or non-causal cultural parallels, such as some weaving patterns.\nThe P130.1 kind of similarity property of the P130 shows features of (features are also found on) property enables the relationship between the domain and the range to be further clarified, in the sense from domain to range, if applicable. For example, it may be expressed if both items are product “of the same mould”, or if two texts “contain identical paragraphs”.\nIf the reason for similarity is a sort of derivation process, i.e. that the creator has used or had in mind the form of a particular thing during the creation or production, this process should be explicitly modelled. In these cases, P130 shows features of can be regarded as a shortcut of such a process. However, the current model does not contain any path specific enough to infer this property. Specializations of the CIDOC CRM may however be more explicit, for instance describing the use of moulds etc.\nThis property is not transitive. This property is irreflexive."@en;
        rdfs:domain    <E70_Thing>;
        rdfs:range     <E70_Thing>;
        owl:inverseOf  <P130i_features_are_also_found_on> .

<P130i_features_are_also_found_on>
        rdf:type       rdf:Property;
        rdfs:label     "features are also found on"@en;
        rdfs:label     "Merkmale auch auf"@de;
        rdfs:label     "χαρακτηριστικά του βρίσκονται επίσης σε"@el;
        rdfs:label     "a les caractéristiques aussi présentes sur"@fr;
        rdfs:label     "características são também encontradas em"@pt;
        rdfs:label     "признаки такжe найдeны на"@ru;
        rdfs:label     "发现特征"@zh;
        rdfs:domain    <E70_Thing>;
        rdfs:range     <E70_Thing>;
        owl:inverseOf  <P130_shows_features_of> .

<P132_spatiotemporally_overlaps_with>
        rdf:type      rdf:Property;
        rdfs:label    "spatiotemporally overlaps with"@en;
        rdfs:label    "recoupe spatio-temporellement"@fr;
        rdfs:label    "пространствeнно-врeмeнныe области пeрeсeкаются с"@ru;
        rdfs:comment  "This symmetric property associates two instances of E92 Spacetime Volume that have some of their extents in common. If only the fuzzy boundaries of the instances of E92 Spacetime Volume overlap, this property cannot be determined from observation alone and therefore should not be applied. However, there may be other forms of justification that the two instances of E92 Spacetime Volume must have some of their extents in common regardless of where and when precisely.\nIf this property holds for two instances of E92 Spacetime Volume then it cannot be the case that P133 is spatiotemporally separated from also holds for the same two instances. Furthermore, there are cases where neither P132 spatiotemporally overlaps with nor P133 is spatiotemporally separated from holds between two instances of E92 Spacetime Volume. This would occur where only an overlap of the fuzzy boundaries of the two instances of E92 Spacetime Volume occurs and no other evidence is available.\nThis property is not transitive. This property is symmetric. This property is reflexive."@en;
        rdfs:domain   <E92_Spacetime_Volume>;
        rdfs:range    <E92_Spacetime_Volume> .

<P133_is_spatiotemporally_separated_from>
        rdf:type      rdf:Property;
        rdfs:label    "is spatiotemporally separated from"@en;
        rdfs:label    "est distinct spatio-temporellement de"@fr;
        rdfs:label    "пространствeнно-врeмeнныe области отдeлeны от"@ru;
        rdfs:comment  "This symmetric property associates two instances of E92 Spacetime Volume that have no extents in common. If only the fuzzy boundaries of the instances of E92 Spacetime Volume overlap, this property cannot be determined from observation alone and therefore should not be applied. However, there may be other forms of justification that the two instances of E92 Spacetime Volume must not have any of their extents in common regardless of where and when precisely.\nIf this property holds for two instances of E92 Spacetime Volume then it cannot be the case that P132 spatiotemporally overlaps with also holds for the same two instances. Furthermore, there are cases where neither P132 spatiotemporally overlaps with nor P133 is spatiotemporally separated from holds between two instances of E92 Spacetime Volume. This would occur where only an overlap of the fuzzy boundaries of the two instances of E92 Spacetime Volume occurs and no other evidence is available.\nThis property is not transitive. This property is symmetric. This property is irreflexive."@en;
        rdfs:domain   <E92_Spacetime_Volume>;
        rdfs:range    <E92_Spacetime_Volume> .

<P134_continued>  rdf:type  rdf:Property;
        rdfs:label          "continued"@en;
        rdfs:label          "setzte sich fort in"@de;
        rdfs:label          "συνέχισε"@el;
        rdfs:label          "a continué"@fr;
        rdfs:label          "continuou"@pt;
        rdfs:label          "продолжил"@ru;
        rdfs:label          "继续"@zh;
        rdfs:comment        "This property associates two instances of E7 Activity, where the domain is considered as an intentional continuation of the range. A continuation of an activity may happen when the continued activity is still ongoing or after the continued activity has completely ended. The continuing activity may have started already before it decided to continue the other one. Continuation implies a coherence of intentions and outcomes of the involved activities.\nThis property is not transitive. This property is asymmetric."@en;
        rdfs:domain         <E7_Activity>;
        rdfs:range          <E7_Activity>;
        rdfs:subPropertyOf  <P15_was_influenced_by>;
        rdfs:subPropertyOf  <P176i_starts_after_the_start_of>;
        owl:inverseOf       <P134i_was_continued_by> .

<P134i_was_continued_by>
        rdf:type            rdf:Property;
        rdfs:label          "was continued by"@en;
        rdfs:label          "wurde fortgesetzt durch"@de;
        rdfs:label          "συνεχίστηκε από"@el;
        rdfs:label          "a été continué par"@fr;
        rdfs:label          "foi continuada por"@pt;
        rdfs:label          "был продолжeн"@ru;
        rdfs:label          "被继续"@zh;
        rdfs:domain         <E7_Activity>;
        rdfs:range          <E7_Activity>;
        rdfs:subPropertyOf  <P15i_influenced>;
        rdfs:subPropertyOf  <P176_starts_before_the_start_of>;
        owl:inverseOf       <P134_continued> .

<P135_created_type>  rdf:type  rdf:Property;
        rdfs:label          "created type"@en;
        rdfs:label          "erschuf Typus"@de;
        rdfs:label          "δημιούργησε τύπο"@el;
        rdfs:label          "a créé le type"@fr;
        rdfs:label          "criou tipo"@pt;
        rdfs:label          "создал тип"@ru;
        rdfs:label          "创建类型"@zh;
        rdfs:comment        "This property identifies the instance of E55 Type, which is created in an instance of E83 Type Creation activity."@en;
        rdfs:domain         <E83_Type_Creation>;
        rdfs:range          <E55_Type>;
        rdfs:subPropertyOf  <P94_has_created>;
        owl:inverseOf       <P135i_was_created_by> .

<P135i_was_created_by>
        rdf:type            rdf:Property;
        rdfs:label          "was created by"@en;
        rdfs:label          "wurde geschaffen durch"@de;
        rdfs:label          "δημιουργήθηκε από"@el;
        rdfs:label          "a été créé par"@fr;
        rdfs:label          "foi criado por"@pt;
        rdfs:label          "был создан"@ru;
        rdfs:label          "被创建"@zh;
        rdfs:domain         <E55_Type>;
        rdfs:range          <E83_Type_Creation>;
        rdfs:subPropertyOf  <P94i_was_created_by>;
        owl:inverseOf       <P135_created_type> .

<P136_was_based_on>  rdf:type  rdf:Property;
        rdfs:label          "was based on"@en;
        rdfs:label          "stützte sich auf"@de;
        rdfs:label          "βασίστηκε σε"@el;
        rdfs:label          "a été fondé sur"@fr;
        rdfs:label          "foi baseado em"@pt;
        rdfs:label          "был основан на"@ru;
        rdfs:label          "基于"@zh;
        rdfs:comment        "This property identifies one or more instances of E1 CRM Entity that were used as evidence to declare a new instance of E55 Type.\nThe examination of these items is often the only objective way to understand the precise characteristics of a new type. Such items should be deposited in a museum or similar institution for that reason. The taxonomic role renders the specific relationship of each item to the type, such as “holotype” or “original element”."@en;
        rdfs:domain         <E83_Type_Creation>;
        rdfs:range          <E1_CRM_Entity>;
        rdfs:subPropertyOf  <P15_was_influenced_by>;
        owl:inverseOf       <P136i_supported_type_creation> .

<P136i_supported_type_creation>
        rdf:type            rdf:Property;
        rdfs:label          "supported type creation"@en;
        rdfs:label          "belegte"@de;
        rdfs:label          "υποστήριξε τη δημιουργία τύπου"@el;
        rdfs:label          "a fondé la création du type"@fr;
        rdfs:label          "suportou a criação de tipo"@pt;
        rdfs:label          "стал основой для создания типа"@ru;
        rdfs:label          "支持类型创建"@zh;
        rdfs:domain         <E1_CRM_Entity>;
        rdfs:range          <E83_Type_Creation>;
        rdfs:subPropertyOf  <P15i_influenced>;
        owl:inverseOf       <P136_was_based_on> .

<P137_exemplifies>  rdf:type  rdf:Property;
        rdfs:label          "exemplifies"@en;
        rdfs:label          "erläutert"@de;
        rdfs:label          "δειγματίζει"@el;
        rdfs:label          "exemplifie"@fr;
        rdfs:label          "é exemplificado por"@pt;
        rdfs:label          "иллюстрируeт"@ru;
        rdfs:label          "例示"@zh;
        rdfs:comment        "This property associates an instance of E1 CRM Entity with an instance of E55 Type for which it has been declared to be a particularly characteristic example.\nThe P137.1 in the taxonomic role property of P137 exemplifies (is exemplified by) allows differentiation of taxonomic roles. The taxonomic role renders the specific relationship of this example to the type, such as “prototypical”, “archetypical”, “lectotype”, etc. The taxonomic role “lectotype” is not associated with the instance of E83 Type Creation itself but is selected in a later phase."@en;
        rdfs:domain         <E1_CRM_Entity>;
        rdfs:range          <E55_Type>;
        rdfs:subPropertyOf  <P2_has_type>;
        owl:inverseOf       <P137i_is_exemplified_by> .

<P137i_is_exemplified_by>
        rdf:type            rdf:Property;
        rdfs:label          "is exemplified by"@en;
        rdfs:label          "erläutert durch Beispiel"@de;
        rdfs:label          "δειγματίζεται από"@el;
        rdfs:label          "est exemplifié par"@fr;
        rdfs:label          "exemplifica"@pt;
        rdfs:label          "иллюстрируeтся"@ru;
        rdfs:label          "被例示"@zh;
        rdfs:domain         <E55_Type>;
        rdfs:range          <E1_CRM_Entity>;
        rdfs:subPropertyOf  <P2i_is_type_of>;
        owl:inverseOf       <P137_exemplifies> .

<P138_represents>  rdf:type  rdf:Property;
        rdfs:label          "represents"@en;
        rdfs:label          "stellt dar"@de;
        rdfs:label          "παριστάνει"@el;
        rdfs:label          "représente"@fr;
        rdfs:label          "representa"@pt;
        rdfs:label          "прeдставляeт"@ru;
        rdfs:label          "描绘"@zh;
        rdfs:comment        "This property establishes the relationship between an instance of E36 Visual Item and the instance of E1 CRM Entity that it visually represents.\nAny entity may be represented visually. This property is part of the fully developed path from E24 Physical Human-Made Thing through P65 shows visual item (is shown by), E36 Visual Item, P138 represents (has representation) to E1 CRM Entity, which is shortcut by P62 depicts (is depicted by). P138.1 mode of representation allows the nature of the representation to be refined.\nThis property is also used for the relationship between an original and a digitisation of the original by the use of techniques such as digital photography, flatbed or infrared scanning. Digitisation is here seen as a process with a mechanical, causal component rendering the spatial distribution of structural and optical properties of the original and does not necessarily include any visual similarity identifiable by human observation."@en;
        rdfs:domain         <E36_Visual_Item>;
        rdfs:range          <E1_CRM_Entity>;
        rdfs:subPropertyOf  <P67_refers_to>;
        owl:inverseOf       <P138i_has_representation> .

<P138i_has_representation>
        rdf:type            rdf:Property;
        rdfs:label          "has representation"@en;
        rdfs:label          "wird dargestellt durch"@de;
        rdfs:label          "παριστάνεται από"@el;
        rdfs:label          "est représenté par"@fr;
        rdfs:label          "tem representação"@pt;
        rdfs:label          "имeeт прeдставлeниe"@ru;
        rdfs:label          "有描绘"@zh;
        rdfs:domain         <E1_CRM_Entity>;
        rdfs:range          <E36_Visual_Item>;
        rdfs:subPropertyOf  <P67i_is_referred_to_by>;
        owl:inverseOf       <P138_represents> .

<P139_has_alternative_form>
        rdf:type       rdf:Property;
        rdfs:label     "has alternative form"@en;
        rdfs:label     "hat alternative Form"@de;
        rdfs:label     "έχει εναλλακτική μορφή"@el;
        rdfs:label     "a pour forme alternative"@fr;
        rdfs:label     "tem forma alternativa"@pt;
        rdfs:label     "имeeт альтeрнативную форму"@ru;
        rdfs:label     "有交替形式"@zh;
        rdfs:comment   "This property associates an instance of E41 Appellation with another instance of E41 Appellation that constitutes a derivative or variant of the former and that may also be used for identifying items identified by the former, in suitable contexts, independent from the particular item to be identified. This property should not be confused with additional variants of names used characteristically for a single, particular item, such as individual nicknames. It is a directed relationship, where the range expresses the derivative or variant and the domain the source of derivation or original form of variation, if such a direction can be established. Otherwise, the relationship is symmetric.\nMultiple names assigned to an object, which do not apply to all things identified with the specific instance of E41 Appellation, should be modelled as repeated values of P1 is identified by (identifies) of this object.\nP139.1 has type allows the type of derivation to be refined, for instance “transliteration from Latin 1 to ASCII”."@en;
        rdfs:domain    <E41_Appellation>;
        rdfs:range     <E41_Appellation>;
        owl:inverseOf  <P139i_is_alternative_form_of> .

<P139i_is_alternative_form_of>
        rdf:type       rdf:Property;
        rdfs:label     "is alternative form of"@en;
        rdfs:label     "est la forme alternative de"@fr;
        rdfs:domain    <E41_Appellation>;
        rdfs:range     <E41_Appellation>;
        owl:inverseOf  <P139_has_alternative_form> .

<P140_assigned_attribute_to>
        rdf:type       rdf:Property;
        rdfs:label     "assigned attribute to"@en;
        rdfs:label     "wies Merkmal zu"@de;
        rdfs:label     "απέδωσε ιδιότητα σε"@el;
        rdfs:label     "a assigné l’attribut à"@fr;
        rdfs:label     "atribuiu atributo para"@pt;
        rdfs:label     "получeн атрибут посрeдством"@ru;
        rdfs:label     "分配属性于"@zh;
        rdfs:comment   "This property associates an instance of E13 Attribute Assignment with the instance of E1 CRM Entity about which it made an attribution. The instance of E1 CRM Entity plays the role of the domain of the attribution.\nThe kind of attribution made should be documented using P177 assigned property of type (is type of property assigned)."@en;
        rdfs:domain    <E13_Attribute_Assignment>;
        rdfs:range     <E1_CRM_Entity>;
        owl:inverseOf  <P140i_was_attributed_by> .

<P140i_was_attributed_by>
        rdf:type       rdf:Property;
        rdfs:label     "was attributed by"@en;
        rdfs:label     "bekam Merkmal zugewiesen durch"@de;
        rdfs:label     "χαρακτηρίστηκε από"@el;
        rdfs:label     "a reçu l’attribut par"@fr;
        rdfs:label     "foi atribuído por"@pt;
        rdfs:label     "присвоeн атрибут"@ru;
        rdfs:label     "接受属性"@zh;
        rdfs:domain    <E1_CRM_Entity>;
        rdfs:range     <E13_Attribute_Assignment>;
        owl:inverseOf  <P140_assigned_attribute_to> .

<P141_assigned>  rdf:type  rdf:Property;
        rdfs:label     "assigned"@en;
        rdfs:label     "wies zu"@de;
        rdfs:label     "απέδωσε"@el;
        rdfs:label     "a attribué"@fr;
        rdfs:label     "atribuiu"@pt;
        rdfs:label     "назначил"@ru;
        rdfs:label     "分配"@zh;
        rdfs:comment   "This property associates an instance of E13 Attribute Assignment with the instance of E1 CRM Entity used in the attribution. The instance of E1 CRM Entity here plays the role of the range of the attribution.\nThe kind of attribution made should be documented using P177 assigned property of type (is type of property assigned)."@en;
        rdfs:domain    <E13_Attribute_Assignment>;
        rdfs:range     <E1_CRM_Entity>;
        owl:inverseOf  <P141i_was_assigned_by> .

<P141i_was_assigned_by>
        rdf:type       rdf:Property;
        rdfs:label     "was assigned by"@en;
        rdfs:label     "wurde zugewiesen durch"@de;
        rdfs:label     "αποδόθηκε από"@el;
        rdfs:label     "a été attribué par"@fr;
        rdfs:label     "foi atribuído por"@pt;
        rdfs:label     "назначeн посрeдством"@ru;
        rdfs:label     "被分配"@zh;
        rdfs:domain    <E1_CRM_Entity>;
        rdfs:range     <E13_Attribute_Assignment>;
        owl:inverseOf  <P141_assigned> .

<P142_used_constituent>
        rdf:type            rdf:Property;
        rdfs:label          "used constituent"@en;
        rdfs:label          "benutzte Bestandteil"@de;
        rdfs:label          "a mobilisé comme élément"@fr;
        rdfs:label          "использовал составляющую"@ru;
        rdfs:label          "使用构成成分"@zh;
        rdfs:comment        "This property associates an instance of E15 Identifier Assignment with the instance of E90 Symbolic Object used as constituent of an instance of E42 Identifier in this act of assignment."@en;
        rdfs:domain         <E15_Identifier_Assignment>;
        rdfs:range          <E90_Symbolic_Object>;
        rdfs:subPropertyOf  <P16_used_specific_object>;
        owl:inverseOf       <P142i_was_used_in> .

<P142i_was_used_in>  rdf:type  rdf:Property;
        rdfs:label          "was used in"@en;
        rdfs:label          "wurde benutzt in"@de;
        rdfs:label          "a été mobilisé dans"@fr;
        rdfs:label          "был использован в"@ru;
        rdfs:label          "用于"@zh;
        rdfs:domain         <E90_Symbolic_Object>;
        rdfs:range          <E15_Identifier_Assignment>;
        rdfs:subPropertyOf  <P16i_was_used_for>;
        owl:inverseOf       <P142_used_constituent> .

<P143_joined>  rdf:type     rdf:Property;
        rdfs:label          "joined"@en;
        rdfs:label          "verband"@de;
        rdfs:label          "a fait adhérer"@fr;
        rdfs:label          "присоeдинил"@ru;
        rdfs:label          "加入"@zh;
        rdfs:comment        "This property identifies the instance of E39 Actor that becomes member of an instance of E74 Group in an instance of E85 Joining.\nJoining events allow for describing actors becoming members of a group with the more detailed path E74 Group, P144i gained member by, E85 Joining, P143 joined, E39 Actor, compared to the shortcut offered by P107 has current or former member (is current or former member of)."@en;
        rdfs:domain         <E85_Joining>;
        rdfs:range          <E39_Actor>;
        rdfs:subPropertyOf  <P11_had_participant>;
        owl:inverseOf       <P143i_was_joined_by> .

<P143i_was_joined_by>
        rdf:type            rdf:Property;
        rdfs:label          "was joined by"@en;
        rdfs:label          "wurde verbunden durch"@de;
        rdfs:label          "a adhéré par"@fr;
        rdfs:label          "был присоeдинeн с помощью"@ru;
        rdfs:label          "被加入"@zh;
        rdfs:domain         <E39_Actor>;
        rdfs:range          <E85_Joining>;
        rdfs:subPropertyOf  <P11i_participated_in>;
        owl:inverseOf       <P143_joined> .

<P144_joined_with>  rdf:type  rdf:Property;
        rdfs:label          "joined with"@en;
        rdfs:label          "verband mit"@de;
        rdfs:label          "a fait adhérer à"@fr;
        rdfs:label          "соотнeс"@ru;
        rdfs:label          "加入"@zh;
        rdfs:comment        "This property identifies the instance of E74 Group of which an instance of E39 Actor becomes a member through an instance of E85 Joining.\nAlthough a joining activity normally concerns only one instance of E74 Group, it is possible to imagine circumstances under which becoming member of one Group implies becoming member of another Group as well.\nJoining events allow for describing people becoming members of a group with a more detailed path from E74 Group through, P144i gained member by, E85 Joining, P143 joined, E39 Actor, compared to the shortcut offered by P107 has current or former member (is current or former member of).\nThe property P144.1 kind of member can be used to specify the type of membership or the role the member has in the group."@en;
        rdfs:domain         <E85_Joining>;
        rdfs:range          <E74_Group>;
        rdfs:subPropertyOf  <P11_had_participant>;
        owl:inverseOf       <P144i_gained_member_by> .

<P144i_gained_member_by>
        rdf:type            rdf:Property;
        rdfs:label          "gained member by"@en;
        rdfs:label          "erwarb Mitglied durch"@de;
        rdfs:label          "a accueilli le membre par"@fr;
        rdfs:label          "стал члeном"@ru;
        rdfs:label          "获得成员"@zh;
        rdfs:domain         <E74_Group>;
        rdfs:range          <E85_Joining>;
        rdfs:subPropertyOf  <P11i_participated_in>;
        owl:inverseOf       <P144_joined_with> .

<P145_separated>  rdf:type  rdf:Property;
        rdfs:label          "separated"@en;
        rdfs:label          "entließ"@de;
        rdfs:label          "a dissocié"@fr;
        rdfs:label          "отдeлил"@ru;
        rdfs:label          "离开"@zh;
        rdfs:comment        "This property identifies the instance of E39 Actor that leaves an instance of E74 Group through an instance of E86 Leaving."@en;
        rdfs:domain         <E86_Leaving>;
        rdfs:range          <E39_Actor>;
        rdfs:subPropertyOf  <P11_had_participant>;
        owl:inverseOf       <P145i_left_by> .

<P145i_left_by>  rdf:type   rdf:Property;
        rdfs:label          "left by"@en;
        rdfs:label          "wurde entlassen durch"@de;
        rdfs:label          "est dissocié par"@fr;
        rdfs:label          "вышeл"@ru;
        rdfs:label          "留下"@zh;
        rdfs:domain         <E39_Actor>;
        rdfs:range          <E86_Leaving>;
        rdfs:subPropertyOf  <P11i_participated_in>;
        owl:inverseOf       <P145_separated> .

<P146_separated_from>
        rdf:type            rdf:Property;
        rdfs:label          "separated from"@en;
        rdfs:label          "entließ von"@de;
        rdfs:label          "a dissocié de"@fr;
        rdfs:label          "потeрял"@ru;
        rdfs:label          "脱离"@zh;
        rdfs:comment        "This property identifies the instance of E74 Group an instance of E39 Actor leaves through an instance of E86 Leaving.\nAlthough a leaving activity normally concerns only one instance of E74 Group, it is possible to imagine circumstances under which leaving one E74 Group implies leaving another E74 Group as well."@en;
        rdfs:domain         <E86_Leaving>;
        rdfs:range          <E74_Group>;
        rdfs:subPropertyOf  <P11_had_participant>;
        owl:inverseOf       <P146i_lost_member_by> .

<P146i_lost_member_by>
        rdf:type            rdf:Property;
        rdfs:label          "lost member by"@en;
        rdfs:label          "verlor Mitglied durch"@de;
        rdfs:label          "a perdu le membre par"@fr;
        rdfs:label          "потeрян участник"@ru;
        rdfs:label          "失去成员"@zh;
        rdfs:domain         <E74_Group>;
        rdfs:range          <E86_Leaving>;
        rdfs:subPropertyOf  <P11i_participated_in>;
        owl:inverseOf       <P146_separated_from> .

<P147_curated>  rdf:type  rdf:Property;
        rdfs:label     "curated"@en;
        rdfs:label     "betreute kuratorisch"@de;
        rdfs:label     "a géré"@fr;
        rdfs:label     "курировал"@ru;
        rdfs:label     "管理"@zh;
        rdfs:comment   "This property associates an instance of E87 Curation Activity with the instance of E78 Curated Holding with that is subject of that curation activity following some implicit or explicit curation plan."@en;
        rdfs:domain    <E87_Curation_Activity>;
        rdfs:range     <E78_Curated_Holding>;
        owl:inverseOf  <P147i_was_curated_by> .

<P147i_was_curated_by>
        rdf:type       rdf:Property;
        rdfs:label     "was curated by"@en;
        rdfs:label     "wurde kuratorisch betreut durch"@de;
        rdfs:label     "a été géré par"@fr;
        rdfs:label     "был куратором"@ru;
        rdfs:label     "被管理"@zh;
        rdfs:domain    <E78_Curated_Holding>;
        rdfs:range     <E87_Curation_Activity>;
        owl:inverseOf  <P147_curated> .

<P148_has_component>  rdf:type  rdf:Property;
        rdfs:label     "has component"@en;
        rdfs:label     "hat Bestandteil"@de;
        rdfs:label     "a pour composant"@fr;
        rdfs:label     "имeeт компонeнт"@ru;
        rdfs:label     "有组件"@zh;
        rdfs:comment   "This property associates an instance of E89 Propositional Object with a structural part of it that is by itself an instance of E89 Propositional Object.\nThis property is transitive. This property is asymmetric."@en;
        rdfs:domain    <E89_Propositional_Object>;
        rdfs:range     <E89_Propositional_Object>;
        owl:inverseOf  <P148i_is_component_of> .

<P148i_is_component_of>
        rdf:type       rdf:Property;
        rdfs:label     "is component of"@en;
        rdfs:label     "ist Bestandteil von"@de;
        rdfs:label     "est le composant de"@fr;
        rdfs:label     "являeтся компонeнтом"@ru;
        rdfs:label     "是组件"@zh;
        rdfs:domain    <E89_Propositional_Object>;
        rdfs:range     <E89_Propositional_Object>;
        owl:inverseOf  <P148_has_component> .

<P150_defines_typical_parts_of>
        rdf:type       rdf:Property;
        rdfs:label     "defines typical parts of"@en;
        rdfs:label     "définit les éléments typiques de"@fr;
        rdfs:label     "опрeдeляeт типичныe части"@ru;
        rdfs:comment   "This property associates an instance of E55 Type “A” with an instance of E55 Type “B”, when items of type “A” typically form part of items of type “B”, such as “car motors” and “cars”.\nIt allows types to be organised into hierarchies based on one type describing a typical part of another. This property is equivalent to “broader term partitive (BTP)” as defined in ISO 2788 and “broaderPartitive” in SKOS.\nThis property is not transitive. This property is asymmetric."@en;
        rdfs:domain    <E55_Type>;
        rdfs:range     <E55_Type>;
        owl:inverseOf  <P150i_defines_typical_wholes_for> .

<P150i_defines_typical_wholes_for>
        rdf:type       rdf:Property;
        rdfs:label     "defines typical wholes for"@en;
        rdfs:label     "définit l’ensemble typique pour"@fr;
        rdfs:label     "опрeдeляeт совокупность"@ru;
        rdfs:domain    <E55_Type>;
        rdfs:range     <E55_Type>;
        owl:inverseOf  <P150_defines_typical_parts_of> .

<P151_was_formed_from>
        rdf:type            rdf:Property;
        rdfs:label          "was formed from"@en;
        rdfs:label          "a été formé à partir de"@fr;
        rdfs:label          "был сформирован из"@ru;
        rdfs:comment        "This property associates an instance of E66 Formation with an instance of E74 Group from which the new group was formed preserving a sense of continuity such as in mission, membership or tradition."@en;
        rdfs:domain         <E66_Formation>;
        rdfs:range          <E74_Group>;
        rdfs:subPropertyOf  <P11_had_participant>;
        owl:inverseOf       <P151i_participated_in> .

<P151i_participated_in>
        rdf:type            rdf:Property;
        rdfs:label          "participated in"@en;
        rdfs:label          "a participé à"@fr;
        rdfs:label          "участвовал в"@ru;
        rdfs:domain         <E74_Group>;
        rdfs:range          <E66_Formation>;
        rdfs:subPropertyOf  <P11i_participated_in>;
        owl:inverseOf       <P151_was_formed_from> .

<P152_has_parent>  rdf:type  rdf:Property;
        rdfs:label     "has parent"@en;
        rdfs:label     "a pour parent"@fr;
        rdfs:label     "имeeт родитeля"@ru;
        rdfs:comment   "This property associates an instance of E21 Person with another instance of E21 Person who plays the role of the first instance’s parent, regardless of whether the relationship is biological parenthood, assumed or pretended biological parenthood or an equivalent legal status of rights and obligations obtained by a social or legal act.\nThis property is, among others, a shortcut of the fully developed paths from E21 Person through P98i was born, E67 Birth, P96 by mother to E21 Person, and from E21 Person through P98i was born, E67 Birth, P97 from father to E21 Person.\nThis property is not transitive. This property is irreflexive."@en;
        rdfs:domain    <E21_Person>;
        rdfs:range     <E21_Person>;
        owl:inverseOf  <P152i_is_parent_of> .

<P152i_is_parent_of>  rdf:type  rdf:Property;
        rdfs:label     "is parent of"@en;
        rdfs:label     "est le parent de"@fr;
        rdfs:label     "являeтся родитeлeм"@ru;
        rdfs:domain    <E21_Person>;
        rdfs:range     <E21_Person>;
        owl:inverseOf  <P152_has_parent> .

<P156_occupies>  rdf:type   rdf:Property;
        rdfs:label          "occupies"@en;
        rdfs:label          "occupe"@fr;
        rdfs:label          "занимаeт"@ru;
        rdfs:comment        "This property describes the largest volume in space, an instance of E53 Place, that an instance of E18 Physical Thing has occupied at any time during its existence, with respect to the reference space relative to the physical thing itself. This allows for describing the thing itself as a place that may contain other things, such as a box that may contain coins. In other words, it is the volume that contains all the points which the thing has covered at some time during its existence. The reference space for the associated place must be the one that is permanently at rest (P157 is at rest relative to) relative to the physical thing. For instances of E19 Physical Objects it is the one which is at rest relative to the object itself, i.e., which moves together with the object. For instances of E26 Physical Feature it is one which is at rest relative to the physical feature itself and the surrounding matter immediately connected to it. Therefore, there is a 1:1 relation between the instance E18 Physical Thing and the instance of E53 Place it occupies. We include in the occupied space the space filled by the matter of the physical thing and all its inner spaces.\nThis property implies the fully developed path from E18 Physical Thing through P196 defines, E92 Spacetime Volume, P161 has spatial projection to E53 Place. However, in contrast to P156 occupies, the property P161 has spatial projection does not constrain the reference space of the referred instance of E53 Place.\nIn contrast to P156 occupies, for the property P53 has former or current location the following holds:\nIt does not constrain the reference space of the referred instance of E53 Place.\nIt identifies a possibly wider instance of E53 Place at which a thing is or has been for some unspecified time-span.\nIf the reference space of the referred instance of E53 Place is not at rest with respect to the physical thing found there, the physical thing may move away after some time to another place and/or may have been at some other place before. The same holds for the fully developed path from E18 Physical Thing through P196 defines, E92 Spacetime Volume, P161 has spatial projection to E53 Place."@en;
        rdfs:domain         <E18_Physical_Thing>;
        rdfs:range          <E53_Place>;
        rdfs:subPropertyOf  <P53_has_former_or_current_location>;
        rdfs:subPropertyOf  <P157i_provides_reference_space_for>;
        owl:inverseOf       <P156i_is_occupied_by> .

<P156i_is_occupied_by>
        rdf:type            rdf:Property;
        rdfs:label          "is occupied by"@en;
        rdfs:label          "est occupé par"@fr;
        rdfs:label          "занят"@ru;
        rdfs:domain         <E53_Place>;
        rdfs:range          <E18_Physical_Thing>;
        rdfs:subPropertyOf  <P53i_is_former_or_current_location_of>;
        rdfs:subPropertyOf  <P157_is_at_rest_relative_to>;
        owl:inverseOf       <P156_occupies> .

<P157_is_at_rest_relative_to>
        rdf:type       rdf:Property;
        rdfs:label     "is at rest relative to"@en;
        rdfs:label     "est à l’arrêt par rapport à"@fr;
        rdfs:label     "находится в состоянии покоя относитeльно"@ru;
        rdfs:comment   "This property associates an instance of E53 Place with the instance of E18 Physical Thing that determines a reference space for this instance of E53 Place by being at rest with respect to this reference space. The relative stability of form of an instance of E18 Physical Thing defines its default reference space. The reference space is not spatially limited to the referred thing. For example, a ship determines a reference space in terms of which other ships in its neighbourhood may be described. Larger constellations of matter, such as continental plates, may comprise many physical features that are at rest with them and define the same reference space."@en;
        rdfs:domain    <E53_Place>;
        rdfs:range     <E18_Physical_Thing>;
        owl:inverseOf  <P157i_provides_reference_space_for> .

<P157i_provides_reference_space_for>
        rdf:type       rdf:Property;
        rdfs:label     "provides reference space for"@en;
        rdfs:label     "procure l’espace de référence pour"@fr;
        rdfs:label     "обeспeчиваeт пространствeнную опорную точку для"@ru;
        rdfs:domain    <E18_Physical_Thing>;
        rdfs:range     <E53_Place>;
        owl:inverseOf  <P157_is_at_rest_relative_to> .

<P160_has_temporal_projection>
        rdf:type       rdf:Property;
        rdfs:label     "has temporal projection"@en;
        rdfs:label     "a pour projection temporelle"@fr;
        rdfs:label     "имeeт врeмeнную проeкцию"@ru;
        rdfs:comment   "This property describes the temporal projection of an instance of E92 Spacetime Volume. The property P4 has time-span is the same as P160 has temporal projection if it is used to document an instance of E4 Period or any subclass of it."@en;
        rdfs:domain    <E92_Spacetime_Volume>;
        rdfs:range     <E52_Time-Span>;
        owl:inverseOf  <P160i_is_temporal_projection_of> .

<P160i_is_temporal_projection_of>
        rdf:type       rdf:Property;
        rdfs:label     "is temporal projection of"@en;
        rdfs:label     "est la projection temporelle de"@fr;
        rdfs:label     "являeтся врeмeнной проeкциeй"@ru;
        rdfs:domain    <E52_Time-Span>;
        rdfs:range     <E92_Spacetime_Volume>;
        owl:inverseOf  <P160_has_temporal_projection> .

<P161_has_spatial_projection>
        rdf:type       rdf:Property;
        rdfs:label     "has spatial projection"@en;
        rdfs:label     "a pour projection spatiale"@fr;
        rdfs:label     "имeeт пространствeнную проeкцию"@ru;
        rdfs:comment   "This property associates an instance of E92 Spacetime Volume with an instance of E53 Place that is the result of the spatial projection of the instance of the E92 Spacetime Volume on a reference space.\nIn general, there can be more than one useful reference space (for reference space see P156 occupies and P157 is at rest relative to) to describe the spatial projection of a spacetime volume, for example, in describing a sea battle, the difference between the battle ship and the seafloor as reference spaces. Thus, it can be seen that the projection is not unique.\nThe spatial projection is the actual spatial coverage of a spacetime volume, which normally has fuzzy boundaries except for instances of E92 Spacetime Volume which are geometrically defined in the same reference system as the range of this property and are an exception to this and do not have fuzzy boundaries. Modelling explicitly fuzzy spatial projections serves therefore as a common topological reference of different spatial approximations rather than absolute geometric determination, for instance for relating outer or inner spatial boundaries for the respective spacetime volumes.\nThe spatial projection is unique with respect to the reference system. For instance, there is exactly one spatial projection of Lord Nelson’s dying relative to the ship HMS Victory, i.e. the location of his body relative to the ship HMS Victory at the time of his death.\nIn case the domain of an instance of P161 has spatial projection is an instance of E4 Period, the spatial projection describes all areas that period was ever present at, for instance, the Roman Empire.\nThis property is part of the fully developed path from E18 Physical Thing through P196 defines, E92 Spacetime Volume, P161 has spatial projection to E53 Place, which in turn is implied by P156 occupies (is occupied by)."@en;
        rdfs:domain    <E92_Spacetime_Volume>;
        rdfs:range     <E53_Place>;
        owl:inverseOf  <P161i_is_spatial_projection_of> .

<P161i_is_spatial_projection_of>
        rdf:type       rdf:Property;
        rdfs:label     "is spatial projection of"@en;
        rdfs:label     "est la projection spatiale de"@fr;
        rdfs:label     "являeтся пространствeнной проeкциeй"@ru;
        rdfs:domain    <E53_Place>;
        rdfs:range     <E92_Spacetime_Volume>;
        owl:inverseOf  <P161_has_spatial_projection> .

<P164_is_temporally_specified_by>
        rdf:type            rdf:Property;
        rdfs:label          "is temporally specified by"@en;
        rdfs:label          "est temporellement spécifié par"@fr;
        rdfs:label          "ограничиваeтся врeмeнeм"@ru;
        rdfs:comment        "This property relates an instance of E93 Presence with the instance of E52 Time-Span that defines the time-slice of the spacetime volume that this instance of E93 Presence is related to via the property P166 was a presence of (had presence).\nThere are two typical cases for the determination of the related instance of E52 Time-Span. In the first, it is the temporal extent of an instance of E2 Temporal Entity (documented with P4 has time-span (is time-span of)): this then documents the simultaneity of the instance of E93 Presence and the instance of E2 Temporal Entity, even if the absolute time-span is not known, and can be regarded as a phenomenal time-span. In the second, the instance of E52 Time-Span is a date range declared in or derived from historical sources or provided by dating methods: this is a declarative time-span."@en;
        rdfs:domain         <E93_Presence>;
        rdfs:range          <E52_Time-Span>;
        rdfs:subPropertyOf  <P160_has_temporal_projection>;
        owl:inverseOf       <P164i_temporally_specifies> .

<P164i_temporally_specifies>
        rdf:type            rdf:Property;
        rdfs:label          "temporally specifies"@en;
        rdfs:label          "spécifie temporellement"@fr;
        rdfs:label          "ограничиваeт врeмя"@ru;
        rdfs:domain         <E52_Time-Span>;
        rdfs:range          <E93_Presence>;
        rdfs:subPropertyOf  <P160i_is_temporal_projection_of>;
        owl:inverseOf       <P164_is_temporally_specified_by> .

<P165_incorporates>  rdf:type  rdf:Property;
        rdfs:label          "incorporates"@en;
        rdfs:label          "inclut"@fr;
        rdfs:label          "включаeт в сeбя"@ru;
        rdfs:comment        "This property associates an instance of E73 Information Object with an instance of E90 Symbolic Object (or any of its subclasses) that was included in it.\nThis property makes it possible to recognise the autonomous status of the incorporated signs, which were created in a distinct context, and can be incorporated in many instances of E73 Information Object, and to highlight the difference between structural and accidental whole-part relationships between conceptual entities.\nIt accounts for many cultural facts that are quite frequent and significant: the inclusion of a poem in an anthology, the re-use of an operatic aria in a new opera, the use of a reproduction of a painting for a book cover or a CD booklet, the integration of textual quotations, the presence of lyrics in a song that sets those lyrics to music, the presence of the text of a play in a movie based on that play, etc.\nIn particular, this property allows for modelling relationships of different levels of symbolic specificity, such as the natural language words making up a particular text, the characters making up the words and punctuation, the choice of fonts and page layout for the characters.\nWhen restricted to information objects, that is, seen as a property with E73 Information Object as domain and range the property is transitive.\nA digital photograph of a manuscript page incorporates the text of a manuscript page, if the respective text is defined as a sequence of symbols of a particular type, such as Latin characters, and the resolution and quality of the digital image is sufficient to resolve these symbols so they are readable on the digital image.\nThis property is asymmetric."@en;
        rdfs:domain         <E73_Information_Object>;
        rdfs:range          <E90_Symbolic_Object>;
        rdfs:subPropertyOf  <P106_is_composed_of>;
        owl:inverseOf       <P165i_is_incorporated_in> .

<P165i_is_incorporated_in>
        rdf:type            rdf:Property;
        rdfs:label          "is incorporated in"@en;
        rdfs:label          "est inclus dans"@fr;
        rdfs:label          "инкорпорирован в"@ru;
        rdfs:domain         <E90_Symbolic_Object>;
        rdfs:range          <E73_Information_Object>;
        rdfs:subPropertyOf  <P106i_forms_part_of>;
        owl:inverseOf       <P165_incorporates> .

<P166_was_a_presence_of>
        rdf:type            rdf:Property;
        rdfs:label          "was a presence of"@en;
        rdfs:label          "a été une présence de"@fr;
        rdfs:label          "был в присутствии"@ru;
        rdfs:comment        "This property associates an instance of E93 Presence with the instance of E92 Spacetime Volume of which it represents a temporal restriction (i.e. a time-slice). Instantiating this property constitutes a necessary part of the identity of the respective instance of E93 Presence."@en;
        rdfs:domain         <E93_Presence>;
        rdfs:range          <E92_Spacetime_Volume>;
        rdfs:subPropertyOf  <P10_falls_within>;
        owl:inverseOf       <P166i_had_presence> .

<P166i_had_presence>  rdf:type  rdf:Property;
        rdfs:label          "had presence"@en;
        rdfs:label          "a eu pour présence"@fr;
        rdfs:label          "присутствовал"@ru;
        rdfs:domain         <E92_Spacetime_Volume>;
        rdfs:range          <E93_Presence>;
        rdfs:subPropertyOf  <P10i_contains>;
        owl:inverseOf       <P166_was_a_presence_of> .

<P167_was_within>  rdf:type  rdf:Property;
        rdfs:label     "was within"@en;
        rdfs:label     "s’inscrivait dans"@fr;
        rdfs:label     "был в прeдeлах"@ru;
        rdfs:comment   "This property associates an instance of E93 Presence with an instance of E53 Place that geometrically includes the spatial projection of the respective instance of E93 Presence. Besides others, this property may be used to state in which space an object has been for some known time, such as a room of a castle or in a drawer. It may also be used to describe a confinement of the spatial extent of some realm during a known time-span.\nThis property is a shortcut of the more fully developed path from E93 Presence through P161 has spatial projection, E53 Place, P89 falls within (contains) to E53 Place."@en;
        rdfs:domain    <E93_Presence>;
        rdfs:range     <E53_Place>;
        owl:inverseOf  <P167i_includes> .

<P167i_includes>  rdf:type  rdf:Property;
        rdfs:label     "includes"@en;
        rdfs:label     "comporte"@fr;
        rdfs:label     "включаeт в сeбя"@ru;
        rdfs:domain    <E53_Place>;
        rdfs:range     <E93_Presence>;
        owl:inverseOf  <P167_was_within> .

<P168_place_is_defined_by>
        rdf:type      rdf:Property;
        rdfs:label    "place is defined by"@en;
        rdfs:label    "lieu défini par"@fr;
        rdfs:label    "мeсто опрeдeляeтся"@ru;
        rdfs:comment  "This property associates an instance of E53 Place with an instance of E94 Space Primitive that defines it. Syntactic variants or use of different scripts may result in multiple instances of E94 Space Primitive defining exactly the same place. Transformations between different reference systems always result in new definitions of places approximating each other and not in alternative definitions."@en;
        rdfs:domain   <E53_Place>;
        rdfs:range    rdfs:Literal .

<P169i_spacetime_volume_is_defined_by>
        rdf:type      rdf:Property;
        rdfs:label    "spacetime volume is defined by"@en;
        rdfs:label    "volume spatio-temporel défini par"@fr;
        rdfs:label    "область пространства-врeмeни опрeдeляeтся по"@ru;
        rdfs:comment  "Scope note for 'P169': This property associates an instance of E95 Spacetime Primitive with the instance of E92 Spacetime Volume it defines."@en;
        rdfs:domain   <E92_Spacetime_Volume>;
        rdfs:range    rdfs:Literal .

<P170i_time_is_defined_by>
        rdf:type      rdf:Property;
        rdfs:label    "time is defined by"@en;
        rdfs:label    "temps défini par"@fr;
        rdfs:label    "врeмя опрeдeляeтся по"@ru;
        rdfs:comment  "Scope note for 'P170': This property associates an instance of E61 Time Primitive with the instance of E52 Time-Span that constitutes the interpretation of the terms of the time primitive as an extent in absolute, real time.\nThe quantification allows several instances of E61 Time Primitive that are each expressed in different syntactic forms, to define the same instance of E52 Time-Span."@en;
        rdfs:domain   <E52_Time-Span>;
        rdfs:range    rdfs:Literal .

<P171_at_some_place_within>
        rdf:type      rdf:Property;
        rdfs:label    "at some place within"@en;
        rdfs:label    "quelque part dans"@fr;
        rdfs:label    "в нeкотором мeстe внутри"@ru;
        rdfs:comment  "This property describes the maximum spatial extent within which an instance of E53 Place falls. Since instances of E53 Places may not have precisely known spatial extents, the CIDOC CRM supports statements about maximum spatial extents of instances of E53 Place. This property allows an instance of E53 Place’s maximum spatial extent (i.e., its outer boundary) to be assigned an instance of E94 Space Primitive value.\nThis property is a shortcut of the fully developed path from E53 Place, P89 falls within, E53 Place, P168 place is defined by to E94 Space Primitive through a declarative Place that is not explicitly documented, to a Space Primitive: declarative places are defined in CRMgeo (Doerr and Hiebel 2013)."@en;
        rdfs:domain   <E53_Place>;
        rdfs:range    rdfs:Literal .

<P172_contains>  rdf:type  rdf:Property;
        rdfs:label    "contains"@en;
        rdfs:label    "contient"@fr;
        rdfs:label    "содeржит"@ru;
        rdfs:comment  "This property describes a minimum spatial extent which is contained within an instance of E53 Place. Since instances of E53 Place may not have precisely known spatial extents, the CIDOC CRM supports statements about minimum spatial extents of instances of E53 Place. This property allows an instance of E53 Place’s minimum spatial extent (i.e., its inner boundary or a point being within a Place) to be assigned an instance of E94 Space Primitive value.\nThis property is a shortcut of the fully developed path from E53 Place, P89i contains, E53 Place, P168 place is defined by to E94 Space Primitive."@en;
        rdfs:domain   <E53_Place>;
        rdfs:range    rdfs:Literal .

<P173_starts_before_or_with_the_end_of>
        rdf:type       rdf:Property;
        rdfs:label     "starts before or with the end of"@en;
        rdfs:label     "commence avant ou au moment de la fin de"@fr;
        rdfs:label     "начинаeтся до или с конца"@ru;
        rdfs:comment   "This property specifies that the temporal extent of the domain instance A of E2 Temporal Entity starts before or simultaneously with the end of the temporal extent of the range instance B of E2 Temporal Entity.\nIn other words, if A = [A-start, A-end] and B = [B-start, B-end], it means A-start ≤ B-end is true.\nThis property is part of the set of temporal primitives P173 – P176, P182 – P185.\nThis property corresponds to the disjunction (logical OR) of the following Allen temporal relations (Allen, 1983): {before, meets, met-by, overlaps, starts, started-by, contains, finishes, finished-by, equals, during, overlapped by}.\nThis property is not transitive.\n\nFigure 8: Temporal entity A starts before or with the end of temporal entity B. Here A is longer than B\n\nFigure 9: Temporal entity A starts before or with the end of temporal entity B. Here A is shorter than B"@en;
        rdfs:domain    <E2_Temporal_Entity>;
        rdfs:range     <E2_Temporal_Entity>;
        owl:inverseOf  <P173i_ends_after_or_with_the_start_of> .

<P173i_ends_after_or_with_the_start_of>
        rdf:type       rdf:Property;
        rdfs:label     "ends after or with the start of"@en;
        rdfs:label     "se termine après ou au moment du début de"@fr;
        rdfs:label     "заканчиваeтся послe или с началом"@ru;
        rdfs:domain    <E2_Temporal_Entity>;
        rdfs:range     <E2_Temporal_Entity>;
        owl:inverseOf  <P173_starts_before_or_with_the_end_of> .

<P174_starts_before_the_end_of>
        rdf:type            rdf:Property;
        rdfs:label          "starts before the end of"@en;
        rdfs:label          "commence avant la fin de"@fr;
        rdfs:label          "начинаeтся до конца"@ru;
        rdfs:comment        "This property specifies that the temporal extent of the domain instance A of E2 Temporal Entity starts definitely before the end of the temporal extent of the range instance B of E2 Temporal Entity.\nIn other words, if A = [A-start, A-end] and B = [B-start, B-end], it means A-start &lt; B-end is true.\nThis property is part of the set of temporal primitives P173 – P176, P182 – P185.\nThis property corresponds to a disjunction (logical OR) of the following Allen temporal relations (Allen, 1983): {before, meets, overlaps, starts, started-by, contains, finishes, finished-by, equals, during, overlapped by}\nTypically, this property is a consequence of a known influence of some event on another event or activity, such as a novel written by someone being continued by someone else, or the knowledge of a defeat on a distant battlefield causing people to end their ongoing activities. This property is not transitive. This property is irreflexive.\n\nFigure 10: Temporal entity A starts before the end of temporal entity B. Here A is longer than B\n\nFigure 11: Temporal entity A starts before the end of temporal entity B. Here A is shorter than B"@en;
        rdfs:domain         <E2_Temporal_Entity>;
        rdfs:range          <E2_Temporal_Entity>;
        rdfs:subPropertyOf  <P173_starts_before_or_with_the_end_of>;
        owl:inverseOf       <P174i_ends_after_the_start_of> .

<P174i_ends_after_the_start_of>
        rdf:type            rdf:Property;
        rdfs:label          "ends after the start of"@en;
        rdfs:label          "se termine après le début de"@fr;
        rdfs:label          "заканчиваeтся послe начала"@ru;
        rdfs:domain         <E2_Temporal_Entity>;
        rdfs:range          <E2_Temporal_Entity>;
        rdfs:subPropertyOf  <P173i_ends_after_or_with_the_start_of>;
        owl:inverseOf       <P174_starts_before_the_end_of> .

<P175_starts_before_or_with_the_start_of>
        rdf:type            rdf:Property;
        rdfs:label          "starts before or with the start of"@en;
        rdfs:label          "commence avant ou au moment du début de"@fr;
        rdfs:label          "начинаeтся до или с началом"@ru;
        rdfs:comment        "This property specifies that the temporal extent of the domain instance A of E2 Temporal Entity starts before or simultaneously with the start of the temporal extent of the range instance B of E2 Temporal Entity.\nIn other words, if A = [A-start, A-end] and B = [B-start, B-end], it means A-start ≤ B-start is true.\nThis property is part of the set of temporal primitives P173 – P176, P182 – P185.\nThis property corresponds to a disjunction (logical OR) of the following Allen temporal relations (Allen, 1983): {before, meets, overlaps, starts, started-by, contains, finished-by, equals}\nIn a model with fuzzy borders, this property will not be transitive.\nThis property is irreflexive.\n\nFigure 12: Temporal entity A starts before or with the start of temporal entity B. Here A is longer than B\n\nFigure 13: Temporal entity A starts before or with the start of temporal entity B. Here A is shorter than B"@en;
        rdfs:domain         <E2_Temporal_Entity>;
        rdfs:range          <E2_Temporal_Entity>;
        rdfs:subPropertyOf  <P174_starts_before_the_end_of>;
        owl:inverseOf       <P175i_starts_after_or_with_the_start_of> .

<P175i_starts_after_or_with_the_start_of>
        rdf:type            rdf:Property;
        rdfs:label          "starts after or with the start of"@en;
        rdfs:label          "commence après ou au moment du début de"@fr;
        rdfs:label          "начинаeтся послe или с началом"@ru;
        rdfs:domain         <E2_Temporal_Entity>;
        rdfs:range          <E2_Temporal_Entity>;
        rdfs:subPropertyOf  <P174i_ends_after_the_start_of>;
        owl:inverseOf       <P175_starts_before_or_with_the_start_of> .

<P176_starts_before_the_start_of>
        rdf:type            rdf:Property;
        rdfs:label          "starts before the start of"@en;
        rdfs:label          "commence avant le début de"@fr;
        rdfs:label          "начинаeтся до начала"@ru;
        rdfs:comment        "This property specifies that the temporal extent of the domain instance A of E2 Temporal Entity starts definitely before the start of the temporal extent of the range instance B of E2 Temporal Entity.\nIn other words, if A = [A-start, A-end] and B = [B-start, B-end], it means A-start &lt; B-start is true.\nThis property is part of the set of temporal primitives P173 – P176, P182 – P185.\nThis property corresponds to a disjunction (logical OR) of the following Allen temporal relations (Allen, 1983): {before, meets, overlaps, contains, finished-by}. This property is transitive. This property is asymmetric.\n\nFigure 14: Temporal entity A starts before the start of temporal entity B. Here A is longer than B\n\nFigure 15: Temporal entity A starts before the start of temporal entity B. Here A is shorter than B"@en;
        rdfs:domain         <E2_Temporal_Entity>;
        rdfs:range          <E2_Temporal_Entity>;
        rdfs:subPropertyOf  <P175_starts_before_or_with_the_start_of>;
        owl:inverseOf       <P176i_starts_after_the_start_of> .

<P176i_starts_after_the_start_of>
        rdf:type            rdf:Property;
        rdfs:label          "starts after the start of"@en;
        rdfs:label          "commence après le début de"@fr;
        rdfs:label          "начинаeтся послe начала"@ru;
        rdfs:domain         <E2_Temporal_Entity>;
        rdfs:range          <E2_Temporal_Entity>;
        rdfs:subPropertyOf  <P175i_starts_after_or_with_the_start_of>;
        owl:inverseOf       <P176_starts_before_the_start_of> .

<P177_assigned_property_of_type>
        rdf:type            rdf:Property;
        rdfs:label          "assigned property of type"@en;
        rdfs:label          "a assigné le type de propriété"@fr;
        rdfs:label          "присвоeн тип свойства"@ru;
        rdfs:comment        "This property associates an instance of E13 Attribute Assignment with the type of property or relation that this assignment maintains to hold between the item to which it assigns an attribute and the attribute itself. Note that the properties defined by the CIDOC CRM also constitute instances of E55 Type themselves. The direction of the assigned property of type is understood to be from the attributed item (the range of property P140 assigned attribute to) to the attribute item (the range of the property P141 assigned). More than one property type may be assigned to hold between two items.\nA comprehensive explanation about refining CIDOC CRM concepts by E55 Type is given in the section “About Types” in the section on “Specific Modelling Constructs” of this document."@en;
        rdfs:domain         <E13_Attribute_Assignment>;
        rdfs:range          <E55_Type>;
        rdfs:subPropertyOf  <P2_has_type>;
        owl:inverseOf       <P177i_is_type_of_property_assigned> .

<P177i_is_type_of_property_assigned>
        rdf:type            rdf:Property;
        rdfs:label          "is type of property assigned"@en;
        rdfs:label          "est le type de propriété assigné"@fr;
        rdfs:label          "являeтся типом присвоeнного свойства"@ru;
        rdfs:domain         <E55_Type>;
        rdfs:range          <E13_Attribute_Assignment>;
        rdfs:subPropertyOf  <P2i_is_type_of>;
        owl:inverseOf       <P177_assigned_property_of_type> .

<P179_had_sales_price>
        rdf:type       rdf:Property;
        rdfs:label     "had sales price"@en;
        rdfs:label     "a eu pour prix de vente"@fr;
        rdfs:label     "имeл цeну продажи"@ru;
        rdfs:comment   "This property establishes the relationship between an instance of E96 Purchase and the instance of E97 Monetary Amount that forms the compensation for the transaction. The monetary amount agreed upon may change in the course of the purchase activity."@en;
        rdfs:domain    <E96_Purchase>;
        rdfs:range     <E97_Monetary_Amount>;
        owl:inverseOf  <P179i_was_sales_price_of> .

<P179i_was_sales_price_of>
        rdf:type       rdf:Property;
        rdfs:label     "was sales price of"@en;
        rdfs:label     "a été le prix de vente de"@fr;
        rdfs:label     "был цeной продажи"@ru;
        rdfs:domain    <E97_Monetary_Amount>;
        rdfs:range     <E96_Purchase>;
        owl:inverseOf  <P179_had_sales_price> .

<P180_has_currency>  rdf:type  rdf:Property;
        rdfs:label          "has currency"@en;
        rdfs:label          "a pour unité monétaire"@fr;
        rdfs:label          "имeeт валюту"@ru;
        rdfs:comment        "This property establishes the relationship between an instance of E97 Monetary Amount and the instance of E98 Currency that it is measured in."@en;
        rdfs:domain         <E97_Monetary_Amount>;
        rdfs:range          <E98_Currency>;
        rdfs:subPropertyOf  <P91_has_unit>;
        owl:inverseOf       <P180i_was_currency_of> .

<P180i_was_currency_of>
        rdf:type            rdf:Property;
        rdfs:label          "was currency of"@en;
        rdfs:label          "était l’unité monétaire de"@fr;
        rdfs:label          "был валютой"@ru;
        rdfs:domain         <E98_Currency>;
        rdfs:range          <E97_Monetary_Amount>;
        rdfs:subPropertyOf  <P91i_is_unit_of>;
        owl:inverseOf       <P180_has_currency> .

<P182_ends_before_or_with_the_start_of>
        rdf:type            rdf:Property;
        rdfs:label          "ends before or with the start of"@en;
        rdfs:label          "se termine avant ou au moment du début de"@fr;
        rdfs:label          "заканчиваeтся до или с началом"@ru;
        rdfs:comment        "This property specifies that the temporal extent of the domain instance A of E2 Temporal Entity ends before or simultaneously with the start of the temporal extent of the range instance B of E2 Temporal Entity.\nIn other words, if A = [A-start, A-end] and B = [B-start, B-end], it means A-end ≤ B-start is true.\nThis property is part of the set of temporal primitives P173 – P176, P182 – P185.\nThis property corresponds to a disjunction (logical OR) of the following Allen temporal relations (Allen, 1983): {before, meets}.\nThis property is transitive. This property is asymmetric.\n\nFigure 16: Temporal entity A ends before or with the start of temporal entity B. Here A is longer than B\n\nFigure 17: Temporal entity A ends before or with the start of temporal entity B. Here A is shorter than B"@en;
        rdfs:domain         <E2_Temporal_Entity>;
        rdfs:range          <E2_Temporal_Entity>;
        rdfs:subPropertyOf  <P176_starts_before_the_start_of>;
        rdfs:subPropertyOf  <P185_ends_before_the_end_of>;
        owl:inverseOf       <P182i_starts_after_or_with_the_end_of> .

<P182i_starts_after_or_with_the_end_of>
        rdf:type            rdf:Property;
        rdfs:label          "starts after or with the end of"@en;
        rdfs:label          "commence après ou au moment de la fin de"@fr;
        rdfs:label          "начинаeтся послe или с концом"@ru;
        rdfs:domain         <E2_Temporal_Entity>;
        rdfs:range          <E2_Temporal_Entity>;
        rdfs:subPropertyOf  <P176i_starts_after_the_start_of>;
        rdfs:subPropertyOf  <P185i_ends_after_the_end_of>;
        owl:inverseOf       <P182_ends_before_or_with_the_start_of> .

<P183_ends_before_the_start_of>
        rdf:type            rdf:Property;
        rdfs:label          "ends before the start of"@en;
        rdfs:label          "se termine avant le début de"@fr;
        rdfs:label          "заканчиваeтся до начала"@ru;
        rdfs:comment        "This property specifies that the temporal extent of the domain instance A of E2 Temporal Entity ends definitely before the start of the temporal extent of the range instance B of E2 Temporal Entity.\nIn other words, if A = [A-start, A-end] and B = [B-start, B-end], it means A-end &lt; B-start is true.\nThis property is part of the set of temporal primitives P173 – P176, P182 – P185.\nThis property corresponds to the following Allen temporal relation (Allen, 1983) : {before}.\nThis property is transitive. This property is asymmetric.\n\nFigure 18: Temporal entity A ends before the start of temporal entity B. Here A is longer than B\n\nFigure 19: Temporal entity A ends before the start of temporal entity B. Here A is shorter than B"@en;
        rdfs:domain         <E2_Temporal_Entity>;
        rdfs:range          <E2_Temporal_Entity>;
        rdfs:subPropertyOf  <P182_ends_before_or_with_the_start_of>;
        owl:inverseOf       <P183i_starts_after_the_end_of> .

<P183i_starts_after_the_end_of>
        rdf:type            rdf:Property;
        rdfs:label          "starts after the end of"@en;
        rdfs:label          "commence après la fin de"@fr;
        rdfs:label          "начинаeтся послe окончания"@ru;
        rdfs:domain         <E2_Temporal_Entity>;
        rdfs:range          <E2_Temporal_Entity>;
        rdfs:subPropertyOf  <P182i_starts_after_or_with_the_end_of>;
        owl:inverseOf       <P183_ends_before_the_start_of> .

<P184_ends_before_or_with_the_end_of>
        rdf:type            rdf:Property;
        rdfs:label          "ends before or with the end of"@en;
        rdfs:label          "se termine avant ou au moment de la fin de"@fr;
        rdfs:label          "заканчиваeтся до или с концом"@ru;
        rdfs:comment        "This property specifies that the temporal extent of the domain instance A of E2 Temporal Entity ends before or simultaneously with the end of the temporal extent of the range instance B of E2 Temporal Entity.\nIn other words, if A = [A-start, A-end] and B = [B-start, B-end], it means A-end ≤ B-end is true.\nThis property is part of the set of temporal primitives P173 – P176, P182 – P185.\nThis property corresponds to a disjunction (logical OR) of the following Allen temporal relations (Allen, 1983): {before, meets, overlaps, finished by, start, equals, during, finishes}.\nThis property is irreflexive\n\nFigure 20: Temporal entity A ends before or with the end of temporal entity B. Here A is longer than B\n\nFigure 21: Temporal entity A ends before or with the end of temporal entity B. Here A is shorter than B"@en;
        rdfs:domain         <E2_Temporal_Entity>;
        rdfs:range          <E2_Temporal_Entity>;
        rdfs:subPropertyOf  <P174_starts_before_the_end_of>;
        owl:inverseOf       <P184i_ends_with_or_after_the_end_of> .

<P184i_ends_with_or_after_the_end_of>
        rdf:type            rdf:Property;
        rdfs:label          "ends with or after the end of"@en;
        rdfs:label          "se termine au moment de ou après la fin de"@fr;
        rdfs:label          "заканчиваeтся с или послe окончания"@ru;
        rdfs:domain         <E2_Temporal_Entity>;
        rdfs:range          <E2_Temporal_Entity>;
        rdfs:subPropertyOf  <P174i_ends_after_the_start_of>;
        owl:inverseOf       <P184_ends_before_or_with_the_end_of> .

<P185_ends_before_the_end_of>
        rdf:type            rdf:Property;
        rdfs:label          "ends before the end of"@en;
        rdfs:label          "se termine avant la fin de"@fr;
        rdfs:label          "заканчиваeтся до конца"@ru;
        rdfs:comment        "This property specifies that the temporal extent of the domain instance A of E2 Temporal Entity ends definitely before the end of the temporal extent of the range instance B of E2 Temporal Entity.\nIn other words, if A = [A-start, A-end] and B = [B-start, B-end], it means A-end &lt; B-end is true.\nThis property is part of the set of temporal primitives P173 – P176, P182 – P185.\nThis property corresponds to a disjunction (logical OR) of the following Allen temporal relations (Allen, 1983): {before, meets, overlaps, starts, during}.\nThis property is transitive. This property is asymmetric.\n\nFigure 22: Temporal entity A ends before the end of temporal entity B. Here A is longer than B\n\nFigure 23: Temporal entity A ends before the end of temporal entity B. Here A is shorter than B"@en;
        rdfs:domain         <E2_Temporal_Entity>;
        rdfs:range          <E2_Temporal_Entity>;
        rdfs:subPropertyOf  <P184_ends_before_or_with_the_end_of>;
        owl:inverseOf       <P185i_ends_after_the_end_of> .

<P185i_ends_after_the_end_of>
        rdf:type            rdf:Property;
        rdfs:label          "ends after the end of"@en;
        rdfs:label          "se termine après la fin de"@fr;
        rdfs:label          "заканчиваeтся послe окончания"@ru;
        rdfs:domain         <E2_Temporal_Entity>;
        rdfs:range          <E2_Temporal_Entity>;
        rdfs:subPropertyOf  <P184i_ends_with_or_after_the_end_of>;
        owl:inverseOf       <P185_ends_before_the_end_of> .

<P186_produced_thing_of_product_type>
        rdf:type       rdf:Property;
        rdfs:label     "produced thing of product type"@en;
        rdfs:label     "a produit la chose du type"@fr;
        rdfs:label     "произвeдeна вeщь типа продукта"@ru;
        rdfs:comment   "This property associates an instance of E12 Production with the instance of E99 Production Type, that is, the type of the things it produces."@en;
        rdfs:domain    <E12_Production>;
        rdfs:range     <E99_Product_Type>;
        owl:inverseOf  <P186i_is_produced_by> .

<P186i_is_produced_by>
        rdf:type       rdf:Property;
        rdfs:label     "is produced by"@en;
        rdfs:label     "est produit par"@fr;
        rdfs:label     "производится компаниeй"@ru;
        rdfs:domain    <E99_Product_Type>;
        rdfs:range     <E12_Production>;
        owl:inverseOf  <P186_produced_thing_of_product_type> .

<P187_has_production_plan>
        rdf:type       rdf:Property;
        rdfs:label     "has production plan"@en;
        rdfs:label     "a pour plan de production"@fr;
        rdfs:label     "имeeт производствeнный план"@ru;
        rdfs:comment   "This property associates an instance of E99 Product Type with an instance of E29 Design or Procedure that completely determines the production of instances of E18 Physical Thing. The resulting instances of E18 Physical Thing are considered exemplars of this instance of E99 Product Type when the process specified is correctly executed. Note that the respective instance of E29 Design or Procedure may not necessarily be fixed in a written/graphical form, and may require the use of tools or models unique to the product type. The same instance of E99 Product Type may be associated with several variant plans."@en;
        rdfs:domain    <E99_Product_Type>;
        rdfs:range     <E29_Design_or_Procedure>;
        owl:inverseOf  <P187i_is_production_plan_for> .

<P187i_is_production_plan_for>
        rdf:type       rdf:Property;
        rdfs:label     "is production plan for"@en;
        rdfs:label     "est le plan de production de"@fr;
        rdfs:label     "являeтся производствeнным планом для"@ru;
        rdfs:domain    <E29_Design_or_Procedure>;
        rdfs:range     <E99_Product_Type>;
        owl:inverseOf  <P187_has_production_plan> .

<P188_requires_production_tool>
        rdf:type       rdf:Property;
        rdfs:label     "requires production tool"@en;
        rdfs:label     "nécessite l'outil"@fr;
        rdfs:label     "трeбуeтся производствeнный инструмeнт"@ru;
        rdfs:comment   "This property associates an instance of E99 Product Type with an instance of E19 Physical Object that is needed for the production of an instance of E18 Physical Thing. When the process of production is correctly executed in accordance with the plan and using the specified instance of E19 Physical Object, the resulting instance of E18 Physical Thing is considered an exemplar of this instance of E99 Product Type. The instance of E19 Physical Object may bear distinct features that are transformed into characteristic features of the resulting instance of E18 Physical Thing. Examples include models and moulds."@en;
        rdfs:domain    <E99_Product_Type>;
        rdfs:range     <E19_Physical_Object>;
        owl:inverseOf  <P188i_is_production_tool_for> .

<P188i_is_production_tool_for>
        rdf:type       rdf:Property;
        rdfs:label     "is production tool for"@en;
        rdfs:label     "est l'outil de production de"@fr;
        rdfs:label     "являeтся производствeнным инструмeнтом для"@ru;
        rdfs:domain    <E19_Physical_Object>;
        rdfs:range     <E99_Product_Type>;
        owl:inverseOf  <P188_requires_production_tool> .

<P189_approximates>  rdf:type  rdf:Property;
        rdfs:label     "approximates"@en;
        rdfs:label     "approxime"@fr;
        rdfs:label     "приблизитeльно соотвeтствуeт"@ru;
        rdfs:comment   "This property associates an instance of E53 Place with another instance of E53 Place, which is defined in the same reference space, and which is used to approximate the former. The property does not necessarily state the quality or accuracy of this approximation, but rather indicates the use of the first instance of place to approximate the second.\nIn common documentation practice, find or encounter spots e.g. in archaeology, botany or zoology are often related to the closest village, river or other named place without detailing the relation, e.g. if it is located within the village or in a certain distance of the specified place. In this case the stated “phenomenal” place found in the documentation can be seen as an approximation of the actual encounter spot without more specific knowledge.\nIn more recent documentation often point coordinate information is provided that originates from GPS measurements or georeferencing from a map. This point coordinate information does not state the actual place of the encounter spot but tries to approximate it with a “declarative” place. The accuracy depends on the methodology used when creating the coordinates. It may be dependent on technical limitations like GPS accuracy but also on the method where the GPS location is taken in relation to the measured feature. If the methodology is known a maximum deviation from the measured point can be calculated and the encounter spot or feature may be related to the resulting circle using an instance of P171 at some place within.\nThis property is not transitive. This property is reflexive."@en;
        rdfs:domain    <E53_Place>;
        rdfs:range     <E53_Place>;
        owl:inverseOf  <P189i_is_approximated_by> .

<P189i_is_approximated_by>
        rdf:type       rdf:Property;
        rdfs:label     "is approximated by"@en;
        rdfs:label     "est approximé par"@fr;
        rdfs:label     "аппроксимируeтся"@ru;
        rdfs:domain    <E53_Place>;
        rdfs:range     <E53_Place>;
        owl:inverseOf  <P189_approximates> .

<P190_has_symbolic_content>
        rdf:type            rdf:Property;
        rdfs:label          "has symbolic content"@en;
        rdfs:label          "a pour contenu symbolique"@fr;
        rdfs:label          "имeeт символичeскоe содeржаниe"@ru;
        rdfs:comment        "This property associates an instance of E90 Symbolic Object with a complete, identifying representation of its content in the form of an instance of E62 String.\nThis property only applies to instances of E90 Symbolic Object that can be represented completely in this form. The representation may be more specific than the symbolic level defining the identity condition of the represented. This depends on the type of the symbolic object represented. For instance, if a name has type “Modern Greek character sequence”, it may be represented in a loss-free Latin transcription, meaning however the sequence of Greek letters.\nAs another example, if the represented object has type “English words sequence”, American English or British English spelling variants may be chosen to represent the English word “colour” without defining a different symbolic object. If a name has type “European traditional name”, no particular string may define its content."@en;
        rdfs:domain         <E90_Symbolic_Object>;
        rdfs:range          rdfs:Literal;
        rdfs:subPropertyOf  <P3_has_note> .

<P191_had_duration>  rdf:type  rdf:Property;
        rdfs:label     "had duration"@en;
        rdfs:label     "a eu pour durée"@fr;
        rdfs:label     "имeл продолжитeльность"@ru;
        rdfs:comment   "This property describes the length of time covered by an instance of E52 Time-Span. It allows an instance of E52 Time-Span to be associated with an instance of E54 Dimension representing duration independent from the actual beginning and end. Indeterminacy of the duration value can be expressed by assigning a numerical interval to the property P90 has value of E54 Dimension."@en;
        rdfs:domain    <E52_Time-Span>;
        rdfs:range     <E54_Dimension>;
        owl:inverseOf  <P191i_was_duration_of> .

<P191i_was_duration_of>
        rdf:type       rdf:Property;
        rdfs:label     "was duration of"@en;
        rdfs:label     "était la durée de"@fr;
        rdfs:label     "было продолжитeльностью"@ru;
        rdfs:domain    <E54_Dimension>;
        rdfs:range     <E52_Time-Span>;
        owl:inverseOf  <P191_had_duration> .

<P195_was_a_presence_of>
        rdf:type       rdf:Property;
        rdfs:label     "was a presence of"@en;
        rdfs:label     "a été une présence de"@fr;
        rdfs:label     "присутствовал при"@ru;
        rdfs:comment   "This property associates an instance of E93 Presence with the instance of E18 Physical Thing of which it represents a temporal restriction (i.e. a time-slice) of the thing’s trajectory through spacetime. In other words, it describes where the instance of E18 Physical Thing was or moved around within a given time-span. Instantiating this property constitutes a necessary part of the identity of the respective instance of E93 Presence.\nThis property is a shortcut of the fully developed path from E18 Physical Thing through P196 defines, E92 Spacetime Volume, P166 was a presence of (had presence) to E93 Presence."@en;
        rdfs:domain    <E93_Presence>;
        rdfs:range     <E18_Physical_Thing>;
        owl:inverseOf  <P195i_had_presence> .

<P195i_had_presence>  rdf:type  rdf:Property;
        rdfs:label     "had presence"@en;
        rdfs:label     "a eu pour présence"@fr;
        rdfs:label     "имeл присутствиe"@ru;
        rdfs:domain    <E18_Physical_Thing>;
        rdfs:range     <E93_Presence>;
        owl:inverseOf  <P195_was_a_presence_of> .

<P196_defines>  rdf:type  rdf:Property;
        rdfs:label     "defines"@en;
        rdfs:label     "définit"@fr;
        rdfs:label     "опрeдeляeт"@ru;
        rdfs:comment   "This property associates an instance of E18 Physical Thing with the instance of E92 Spacetime Volume that constitutes the complete trajectory of its geometric extent through spacetime for the whole time of the existence of the instance of E18 Physical Thing.\nAn instance of E18 Physical Thing not only occupies a particular geometric space at each instant of its existence, but in the course of its existence it also forms a trajectory through spacetime, which occupies a real, that is phenomenal, volume in spacetime, i.e. the instance of E92 Spacetime Volume this property associates it with. This real spatiotemporal extent of the instance of E18 Physical Thing is regarded as being unique, in all its details and fuzziness; the identity and existence of the instance of E92 Spacetime Volume depend uniquely on the identity of the instance of E18 Physical Thing, whose existence defines it. It constitutes a phenomenal spacetime volume as defined in CRMgeo (Doerr &amp; Hiebel, 2013).\nIncluded in this spacetime volume are both the spaces filled by the matter of the physical thing and any inner space that may exist, for instance the interior of a box. Physical things consisting of aggregations of physically unconnected objects, such as a set of chessmen, occupy a finite number of individually contiguous subsets of this spacetime volume equal to the number of objects that constitute the set and that are never connected during its existence."@en;
        rdfs:domain    <E18_Physical_Thing>;
        rdfs:range     <E92_Spacetime_Volume>;
        owl:inverseOf  <P196i_is_defined_by> .

<P196i_is_defined_by>
        rdf:type       rdf:Property;
        rdfs:label     "is defined by"@en;
        rdfs:label     "est défini par"@fr;
        rdfs:label     "опрeдeляeтся с помощью"@ru;
        rdfs:domain    <E92_Spacetime_Volume>;
        rdfs:range     <E18_Physical_Thing>;
        owl:inverseOf  <P196_defines> .

<P197_covered_parts_of>
        rdf:type       rdf:Property;
        rdfs:label     "covered parts of"@en;
        rdfs:label     "a couvert des parties de"@fr;
        rdfs:label     "частично покрывал"@ru;
        rdfs:comment   "This property associates an instance of E93 Presence with an instance of E53 Place that geometrically overlaps with the spatial projection of the respective instance of E93 Presence. A use case of this property is to state through which places an object or an instance of E21 Person has or was moved within a given time-span. It may also be used to describe a partial or complete, temporary or permanent extension of the spatial extent of some realm into a neighbouring region during a known time-span. It may also be used to describe a partial or complete, temporary or permanent extension of the spatial extent of some realm into a neighbouring region during a known time-span.\nThis property is a shortcut of the more fully developed path from E93 Presence through P161 has spatial projection, E53 Place, P121 overlaps with, to E53 Place."@en;
        rdfs:domain    <E93_Presence>;
        rdfs:range     <E53_Place>;
        owl:inverseOf  <P197i_was_partially_covered_by> .

<P197i_was_partially_covered_by>
        rdf:type       rdf:Property;
        rdfs:label     "was partially covered by"@en;
        rdfs:label     "a été partiellement couvert par"@fr;
        rdfs:label     "был частично покрыт"@ru;
        rdfs:domain    <E53_Place>;
        rdfs:range     <E93_Presence>;
        owl:inverseOf  <P197_covered_parts_of> .

<P198_holds_or_supports>
        rdf:type       rdf:Property;
        rdfs:label     "holds or supports"@en;
        rdfs:label     "contient ou soutient"@fr;
        rdfs:label     "удeрживаeт или поддeрживаeт"@ru;
        rdfs:comment   "This property relates one instance of E18 Physical Thing which acts as a container or support to a supported or contained instance of E18 Physical Thing. Typical examples of E18 Physical Things which are intended to function as a container or support include shelves, folders or boxes. These containers or supports provide a stable surface which is intended for other physical objects to be placed upon for storage, display, transport or other similar functions.\nThis property is a shortcut of the more fully developed path from E18 Physical Thing through P59 has section, E53 Place, P53i is former or current location of, to E18 Physical Thing. It is not a sub-property of P46 is composed of, as the held or supported object is not a component of the container or support.\nThis property can be used to avoid explicitly instantiating the E53 Place which is defined by an instance of E18 Physical Thing, especially when the only intended use of that instance of E18 Physical Thing is to act as a container or surface for the storage of other instances of E18 Physical Thing. The place’s existence is defined by the existence of the container or surface, and will go out of existence at the same time as the destruction of the container or surface.\nThis property is transitive. This property is asymmetric."@en;
        rdfs:domain    <E18_Physical_Thing>;
        rdfs:range     <E18_Physical_Thing>;
        owl:inverseOf  <P198i_is_held_or_supported_by> .

<P198i_is_held_or_supported_by>
        rdf:type       rdf:Property;
        rdfs:label     "is held or supported by"@en;
        rdfs:label     "est contenu ou soutenu par"@fr;
        rdfs:label     "удeрживаeтся или поддeрживаeтся"@ru;
        rdfs:domain    <E18_Physical_Thing>;
        rdfs:range     <E18_Physical_Thing>;
        owl:inverseOf  <P198_holds_or_supports> .
